<?xml version="1.0"?>
<rdf:RDF xmlns="http://purl.obolibrary.org/obo/envo/subsets/biome-hierarchy.owl#"
     xml:base="http://purl.obolibrary.org/obo/envo/subsets/biome-hierarchy.owl"
     xmlns:dc="http://purl.org/dc/elements/1.1/"
     xmlns:obo="http://purl.obolibrary.org/obo/"
     xmlns:owl="http://www.w3.org/2002/07/owl#"
     xmlns:rdf="http://www.w3.org/1999/02/22-rdf-syntax-ns#"
     xmlns:xml="http://www.w3.org/XML/1998/namespace"
     xmlns:xsd="http://www.w3.org/2001/XMLSchema#"
     xmlns:rdfs="http://www.w3.org/2000/01/rdf-schema#"
     xmlns:oboInOwl="http://www.geneontology.org/formats/oboInOwl#">
    <owl:Ontology rdf:about="http://purl.obolibrary.org/obo/envo/subsets/biome-hierarchy.owl">
        <owl:versionIRI rdf:resource="http://purl.obolibrary.org/obo/envo/releases/2025-10-20/subsets/biome-hierarchy.owl"/>
        <owl:versionInfo>subsets/biome-hierarchy.owl 2025-10-20</owl:versionInfo>
    </owl:Ontology>
    


    <!-- 
    ///////////////////////////////////////////////////////////////////////////////////////
    //
    // Annotation properties
    //
    ///////////////////////////////////////////////////////////////////////////////////////
     -->

    


    <!-- http://purl.obolibrary.org/obo/IAO_0000115 -->

    <owl:AnnotationProperty rdf:about="http://purl.obolibrary.org/obo/IAO_0000115">
        <rdfs:label>definition</rdfs:label>
    </owl:AnnotationProperty>
    


    <!-- http://purl.obolibrary.org/obo/IAO_0000116 -->

    <owl:AnnotationProperty rdf:about="http://purl.obolibrary.org/obo/IAO_0000116"/>
    


    <!-- http://purl.org/dc/elements/1.1/creator -->

    <owl:AnnotationProperty rdf:about="http://purl.org/dc/elements/1.1/creator"/>
    


    <!-- http://purl.org/dc/elements/1.1/date -->

    <owl:AnnotationProperty rdf:about="http://purl.org/dc/elements/1.1/date"/>
    


    <!-- http://www.geneontology.org/formats/oboInOwl#created_by -->

    <owl:AnnotationProperty rdf:about="http://www.geneontology.org/formats/oboInOwl#created_by"/>
    


    <!-- http://www.geneontology.org/formats/oboInOwl#creation_date -->

    <owl:AnnotationProperty rdf:about="http://www.geneontology.org/formats/oboInOwl#creation_date"/>
    


    <!-- http://www.geneontology.org/formats/oboInOwl#hasBroadSynonym -->

    <owl:AnnotationProperty rdf:about="http://www.geneontology.org/formats/oboInOwl#hasBroadSynonym"/>
    


    <!-- http://www.geneontology.org/formats/oboInOwl#hasDbXref -->

    <owl:AnnotationProperty rdf:about="http://www.geneontology.org/formats/oboInOwl#hasDbXref"/>
    


    <!-- http://www.geneontology.org/formats/oboInOwl#hasExactSynonym -->

    <owl:AnnotationProperty rdf:about="http://www.geneontology.org/formats/oboInOwl#hasExactSynonym"/>
    


    <!-- http://www.geneontology.org/formats/oboInOwl#hasNarrowSynonym -->

    <owl:AnnotationProperty rdf:about="http://www.geneontology.org/formats/oboInOwl#hasNarrowSynonym"/>
    


    <!-- http://www.geneontology.org/formats/oboInOwl#hasOBONamespace -->

    <owl:AnnotationProperty rdf:about="http://www.geneontology.org/formats/oboInOwl#hasOBONamespace"/>
    


    <!-- http://www.geneontology.org/formats/oboInOwl#hasRelatedSynonym -->

    <owl:AnnotationProperty rdf:about="http://www.geneontology.org/formats/oboInOwl#hasRelatedSynonym"/>
    


    <!-- http://www.geneontology.org/formats/oboInOwl#id -->

    <owl:AnnotationProperty rdf:about="http://www.geneontology.org/formats/oboInOwl#id"/>
    


    <!-- http://www.geneontology.org/formats/oboInOwl#inSubset -->

    <owl:AnnotationProperty rdf:about="http://www.geneontology.org/formats/oboInOwl#inSubset"/>
    


    <!-- 
    ///////////////////////////////////////////////////////////////////////////////////////
    //
    // Classes
    //
    ///////////////////////////////////////////////////////////////////////////////////////
     -->

    


    <!-- http://purl.obolibrary.org/obo/ENVO_00000428 -->

    <owl:Class rdf:about="http://purl.obolibrary.org/obo/ENVO_00000428">
        <obo:IAO_0000115 xml:lang="en">A biome is an ecosystem which is undergoing climactic ecological succession.</obo:IAO_0000115>
        <oboInOwl:hasDbXref>EcoLexicon:biome</oboInOwl:hasDbXref>
        <oboInOwl:hasDbXref>LTER:809</oboInOwl:hasDbXref>
        <oboInOwl:hasExactSynonym>major habitat type</oboInOwl:hasExactSynonym>
        <oboInOwl:hasRelatedSynonym>EcosytemType</oboInOwl:hasRelatedSynonym>
        <rdfs:comment xml:lang="en">In this definition, there is an assumption that no major perturbations are occurring or have occurred in a time frame affects the successional dynamics of the ecosystem. A &quot;major&quot; perturbation is one which disrupts the community&apos;s ability to restore its (near) equilibrium. Usually, pioneer or early secondary successional processes would be in effect in such scenarios.</rdfs:comment>
        <rdfs:label>biome</rdfs:label>
    </owl:Class>
    <owl:Axiom>
        <owl:annotatedSource rdf:resource="http://purl.obolibrary.org/obo/ENVO_00000428"/>
        <owl:annotatedProperty rdf:resource="http://purl.obolibrary.org/obo/IAO_0000115"/>
        <owl:annotatedTarget xml:lang="en">A biome is an ecosystem which is undergoing climactic ecological succession.</owl:annotatedTarget>
        <oboInOwl:hasDbXref>DOI:10.1186/2041-1480-4-43</oboInOwl:hasDbXref>
        <oboInOwl:hasDbXref>https://en.wikipedia.org/wiki/Biome</oboInOwl:hasDbXref>
    </owl:Axiom>
    <owl:Axiom>
        <owl:annotatedSource rdf:resource="http://purl.obolibrary.org/obo/ENVO_00000428"/>
        <owl:annotatedProperty rdf:resource="http://www.geneontology.org/formats/oboInOwl#hasDbXref"/>
        <owl:annotatedTarget>LTER:809</owl:annotatedTarget>
        <oboInOwl:hasDbXref>https://vocab.lternet.edu/vocab/vocab/index.php?tema=809&amp;/biomes</oboInOwl:hasDbXref>
    </owl:Axiom>
    <owl:Axiom>
        <owl:annotatedSource rdf:resource="http://purl.obolibrary.org/obo/ENVO_00000428"/>
        <owl:annotatedProperty rdf:resource="http://www.geneontology.org/formats/oboInOwl#hasExactSynonym"/>
        <owl:annotatedTarget>major habitat type</owl:annotatedTarget>
        <oboInOwl:hasDbXref>WWF:Biome</oboInOwl:hasDbXref>
    </owl:Axiom>
    <owl:Axiom>
        <owl:annotatedSource rdf:resource="http://purl.obolibrary.org/obo/ENVO_00000428"/>
        <owl:annotatedProperty rdf:resource="http://www.geneontology.org/formats/oboInOwl#hasRelatedSynonym"/>
        <owl:annotatedTarget>EcosytemType</owl:annotatedTarget>
        <oboInOwl:hasDbXref>NASA:earthrealm</oboInOwl:hasDbXref>
    </owl:Axiom>
    


    <!-- http://purl.obolibrary.org/obo/ENVO_00000446 -->

    <owl:Class rdf:about="http://purl.obolibrary.org/obo/ENVO_00000446">
        <rdfs:subClassOf rdf:resource="http://purl.obolibrary.org/obo/ENVO_00000428"/>
        <obo:IAO_0000115>A biome which is  primarily or completely situated on a landmass.</obo:IAO_0000115>
        <oboInOwl:hasDbXref>LTER:798</oboInOwl:hasDbXref>
        <oboInOwl:hasDbXref>SPIRE:Terrestrial</oboInOwl:hasDbXref>
        <oboInOwl:hasRelatedSynonym>terrestrial realm</oboInOwl:hasRelatedSynonym>
        <rdfs:label>terrestrial biome</rdfs:label>
    </owl:Class>
    <owl:Axiom>
        <owl:annotatedSource rdf:resource="http://purl.obolibrary.org/obo/ENVO_00000446"/>
        <owl:annotatedProperty rdf:resource="http://purl.obolibrary.org/obo/IAO_0000115"/>
        <owl:annotatedTarget>A biome which is  primarily or completely situated on a landmass.</owl:annotatedTarget>
        <oboInOwl:hasDbXref>https://en.wikipedia.org/wiki/Biome#Terrestrial_biomes</oboInOwl:hasDbXref>
    </owl:Axiom>
    


    <!-- http://purl.obolibrary.org/obo/ENVO_00000447 -->

    <owl:Class rdf:about="http://purl.obolibrary.org/obo/ENVO_00000447">
        <rdfs:subClassOf rdf:resource="http://purl.obolibrary.org/obo/ENVO_00002030"/>
        <obo:IAO_0000115>An aquatic biome which is determined by a marine water body.</obo:IAO_0000115>
        <oboInOwl:hasDbXref>SPIRE:Marine</oboInOwl:hasDbXref>
        <oboInOwl:hasRelatedSynonym>marine realm</oboInOwl:hasRelatedSynonym>
        <oboInOwl:inSubset>envoPolar</oboInOwl:inSubset>
        <rdfs:comment>This biome includes open-ocean and unprotected coastal ecosystems, characterized by exposure to wave action, tidal fluctuation, and ocean currents as well as systems that largely resemble these. Water in the marine biome is generally within the salinity range of seawater: 30 to 38 ppt.</rdfs:comment>
        <rdfs:label>marine biome</rdfs:label>
    </owl:Class>
    <owl:Axiom>
        <owl:annotatedSource rdf:resource="http://purl.obolibrary.org/obo/ENVO_00000447"/>
        <owl:annotatedProperty rdf:resource="http://purl.obolibrary.org/obo/IAO_0000115"/>
        <owl:annotatedTarget>An aquatic biome which is determined by a marine water body.</owl:annotatedTarget>
        <oboInOwl:hasDbXref rdf:resource="https://orcid.org/0000-0002-4366-3088"/>
        <oboInOwl:hasDbXref>ISBN:978-0-618-45504-1</oboInOwl:hasDbXref>
        <oboInOwl:hasDbXref>MA:ma</oboInOwl:hasDbXref>
        <oboInOwl:hasDbXref>https://en.wikipedia.org/wiki/Ocean</oboInOwl:hasDbXref>
    </owl:Axiom>
    


    <!-- http://purl.obolibrary.org/obo/ENVO_00000873 -->

    <owl:Class rdf:about="http://purl.obolibrary.org/obo/ENVO_00000873">
        <rdfs:subClassOf rdf:resource="http://purl.obolibrary.org/obo/ENVO_00002030"/>
        <obo:IAO_0000115>An aquatic biome which is determined by a body of freshwater.</obo:IAO_0000115>
        <oboInOwl:hasDbXref>SPIRE:Freshwater</oboInOwl:hasDbXref>
        <oboInOwl:hasRelatedSynonym>freshwater realm</oboInOwl:hasRelatedSynonym>
        <oboInOwl:inSubset>envoPolar</oboInOwl:inSubset>
        <rdfs:label>freshwater biome</rdfs:label>
    </owl:Class>
    <owl:Axiom>
        <owl:annotatedSource rdf:resource="http://purl.obolibrary.org/obo/ENVO_00000873"/>
        <owl:annotatedProperty rdf:resource="http://purl.obolibrary.org/obo/IAO_0000115"/>
        <owl:annotatedTarget>An aquatic biome which is determined by a body of freshwater.</owl:annotatedTarget>
        <oboInOwl:hasDbXref rdf:resource="https://orcid.org/0000-0002-4366-3088"/>
        <oboInOwl:hasDbXref>MA:ma</oboInOwl:hasDbXref>
    </owl:Axiom>
    


    <!-- http://purl.obolibrary.org/obo/ENVO_00000887 -->

    <owl:Class rdf:about="http://purl.obolibrary.org/obo/ENVO_00000887">
        <rdfs:subClassOf rdf:resource="http://purl.obolibrary.org/obo/ENVO_01000253"/>
        <obo:IAO_0000115 xml:lang="en">A freshwater river biome which is determined by a large river.</obo:IAO_0000115>
        <oboInOwl:inSubset>wwfBiome</oboInOwl:inSubset>
        <rdfs:comment>&quot;Large&quot; is ambiguous. For details on &quot;Large rivers&quot; (e.g. the Mekong river) see http://worldwildlife.org/biomes/large-river-ecosystems This class will be replaced with a less ambiguous class.</rdfs:comment>
        <rdfs:label>large river biome</rdfs:label>
    </owl:Class>
    


    <!-- http://purl.obolibrary.org/obo/ENVO_00000888 -->

    <owl:Class rdf:about="http://purl.obolibrary.org/obo/ENVO_00000888">
        <rdfs:subClassOf rdf:resource="http://purl.obolibrary.org/obo/ENVO_01000253"/>
        <obo:IAO_0000115 xml:lang="en">A freshwater river biome which is determined by the headwaters of a large river.</obo:IAO_0000115>
        <oboInOwl:inSubset>wwfBiome</oboInOwl:inSubset>
        <rdfs:comment>&quot;Large&quot; is ambiguous. For details on &quot;Large river headwaters&quot; (e.g. the Upper Amazon headwaters) see http://worldwildlife.org/biomes/large-river-headwater-ecosystems This class will be replaced with a less ambiguous class.</rdfs:comment>
        <rdfs:label>large river headwater biome</rdfs:label>
    </owl:Class>
    


    <!-- http://purl.obolibrary.org/obo/ENVO_00000889 -->

    <owl:Class rdf:about="http://purl.obolibrary.org/obo/ENVO_00000889">
        <rdfs:subClassOf rdf:resource="http://purl.obolibrary.org/obo/ENVO_01000253"/>
        <obo:IAO_0000115 xml:lang="en">A freshwater river biome which is determined by the delta of a large river.</obo:IAO_0000115>
        <oboInOwl:inSubset>wwfBiome</oboInOwl:inSubset>
        <rdfs:comment>&quot;Large&quot; is ambiguous. For details on &quot;Large river deltas&quot; (e.g. the Niger river delta) see http://worldwildlife.org/biomes/large-river-delta-ecosystems This class will be replaced with a less ambiguous class.</rdfs:comment>
        <rdfs:label>large river delta biome</rdfs:label>
    </owl:Class>
    


    <!-- http://purl.obolibrary.org/obo/ENVO_00000890 -->

    <owl:Class rdf:about="http://purl.obolibrary.org/obo/ENVO_00000890">
        <rdfs:subClassOf rdf:resource="http://purl.obolibrary.org/obo/ENVO_01000253"/>
        <obo:IAO_0000115 xml:lang="en">A freshwater river biome which is determined by a small river.</obo:IAO_0000115>
        <oboInOwl:inSubset>wwfBiome</oboInOwl:inSubset>
        <rdfs:comment>&quot;Small&quot; is ambiguous. For details on &quot;Small rivers&quot; (e.g. the Salween river) see http://worldwildlife.org/biomes/small-river-ecosystems. This class will be replaced with a less ambiguous class.</rdfs:comment>
        <rdfs:label>small river biome</rdfs:label>
    </owl:Class>
    


    <!-- http://purl.obolibrary.org/obo/ENVO_00000891 -->

    <owl:Class rdf:about="http://purl.obolibrary.org/obo/ENVO_00000891">
        <rdfs:subClassOf rdf:resource="http://purl.obolibrary.org/obo/ENVO_01000252"/>
        <obo:IAO_0000115 xml:lang="en">A freshwater biome which is determined by a large lake.</obo:IAO_0000115>
        <oboInOwl:inSubset>wwfBiome</oboInOwl:inSubset>
        <rdfs:comment>&quot;Large&quot; is ambiguous. For details on &quot;Large lakes&quot; (e.g. African rift lakes) see http://worldwildlife.org/biomes/large-lake-ecosystems This class will be replaced with a less ambiguous class.</rdfs:comment>
        <rdfs:label>large freshwater lake biome</rdfs:label>
    </owl:Class>
    


    <!-- http://purl.obolibrary.org/obo/ENVO_00000892 -->

    <owl:Class rdf:about="http://purl.obolibrary.org/obo/ENVO_00000892">
        <rdfs:subClassOf rdf:resource="http://purl.obolibrary.org/obo/ENVO_01000252"/>
        <obo:IAO_0000115 xml:lang="en">A freshwater lake biome which is determined by a small lake.</obo:IAO_0000115>
        <oboInOwl:inSubset>wwfBiome</oboInOwl:inSubset>
        <rdfs:comment>&quot;Small&quot; is ambiguous. For details on &quot;Small lakes&quot; (e.g. Cameroon crater lakes)  see http://worldwildlife.org/biomes/small-lake-ecosystems. This class will be replaced with a less ambiguous class.</rdfs:comment>
        <rdfs:label>small freshwater lake biome</rdfs:label>
    </owl:Class>
    


    <!-- http://purl.obolibrary.org/obo/ENVO_00000893 -->

    <owl:Class rdf:about="http://purl.obolibrary.org/obo/ENVO_00000893">
        <rdfs:subClassOf rdf:resource="http://purl.obolibrary.org/obo/ENVO_00000873"/>
        <obo:IAO_0000115>A biome which has little permanent surface water and a low relative abundance of springs.</obo:IAO_0000115>
        <obo:IAO_0000116>The WWF definition is somewhat ambiguous, but workable.</obo:IAO_0000116>
        <oboInOwl:inSubset>wwfBiome</oboInOwl:inSubset>
        <rdfs:label>xeric basin biome</rdfs:label>
    </owl:Class>
    <owl:Axiom>
        <owl:annotatedSource rdf:resource="http://purl.obolibrary.org/obo/ENVO_00000893"/>
        <owl:annotatedProperty rdf:resource="http://purl.obolibrary.org/obo/IAO_0000115"/>
        <owl:annotatedTarget>A biome which has little permanent surface water and a low relative abundance of springs.</owl:annotatedTarget>
        <oboInOwl:hasDbXref>https://www.worldwildlife.org/biomes/xeric-basin-ecosystems</oboInOwl:hasDbXref>
    </owl:Axiom>
    


    <!-- http://purl.obolibrary.org/obo/ENVO_00002030 -->

    <owl:Class rdf:about="http://purl.obolibrary.org/obo/ENVO_00002030">
        <rdfs:subClassOf rdf:resource="http://purl.obolibrary.org/obo/ENVO_00000428"/>
        <obo:IAO_0000115>A biome which is determined by a water body and which has ecological climax communities adapted to life in or on water.</obo:IAO_0000115>
        <oboInOwl:hasDbXref>LTER:41</oboInOwl:hasDbXref>
        <rdfs:label>aquatic biome</rdfs:label>
    </owl:Class>
    


    <!-- http://purl.obolibrary.org/obo/ENVO_01000004 -->

    <owl:Class rdf:about="http://purl.obolibrary.org/obo/ENVO_01000004">
        <rdfs:subClassOf rdf:resource="http://purl.obolibrary.org/obo/ENVO_01000047"/>
        <obo:IAO_0000115>The concentration basin mediterranean sea biome comprises expressions of the mediterranean sea biome that have higher salinity than bordering oceans due to evaporation. Water exchange consists of inflow of the fresher oceanic water in the upper layer and outflow of the saltier mediterranean water in the lower layer of the connecting channel.</obo:IAO_0000115>
        <oboInOwl:created_by>ORCID:0000-0002-4366-3088</oboInOwl:created_by>
        <oboInOwl:creation_date>2010-03-19T09:32:59Z</oboInOwl:creation_date>
        <rdfs:label>concentration basin mediterranean sea biome</rdfs:label>
    </owl:Class>
    <owl:Axiom>
        <owl:annotatedSource rdf:resource="http://purl.obolibrary.org/obo/ENVO_01000004"/>
        <owl:annotatedProperty rdf:resource="http://purl.obolibrary.org/obo/IAO_0000115"/>
        <owl:annotatedTarget>The concentration basin mediterranean sea biome comprises expressions of the mediterranean sea biome that have higher salinity than bordering oceans due to evaporation. Water exchange consists of inflow of the fresher oceanic water in the upper layer and outflow of the saltier mediterranean water in the lower layer of the connecting channel.</owl:annotatedTarget>
        <oboInOwl:hasDbXref>ORCID:0000-0002-4366-3088</oboInOwl:hasDbXref>
        <oboInOwl:hasDbXref>https://en.wikipedia.org/wiki/Mediterranean_sea</oboInOwl:hasDbXref>
    </owl:Axiom>
    


    <!-- http://purl.obolibrary.org/obo/ENVO_01000020 -->

    <owl:Class rdf:about="http://purl.obolibrary.org/obo/ENVO_01000020">
        <rdfs:subClassOf rdf:resource="http://purl.obolibrary.org/obo/ENVO_00000447"/>
        <obo:IAO_0000115>Expressions of the estuarine biome occur at wide lower courses of a rivers where they flow into a sea. Estuaries experience tidal flows and their water is a changing mixture of fresh and salt.</obo:IAO_0000115>
        <oboInOwl:created_by>ORCID:0000-0002-4366-3088</oboInOwl:created_by>
        <oboInOwl:creation_date>2010-03-15T11:17:06Z</oboInOwl:creation_date>
        <oboInOwl:hasDbXref>SPIRE:Estuarine</oboInOwl:hasDbXref>
        <rdfs:label>estuarine biome</rdfs:label>
    </owl:Class>
    <owl:Axiom>
        <owl:annotatedSource rdf:resource="http://purl.obolibrary.org/obo/ENVO_01000020"/>
        <owl:annotatedProperty rdf:resource="http://purl.obolibrary.org/obo/IAO_0000115"/>
        <owl:annotatedTarget>Expressions of the estuarine biome occur at wide lower courses of a rivers where they flow into a sea. Estuaries experience tidal flows and their water is a changing mixture of fresh and salt.</owl:annotatedTarget>
        <oboInOwl:hasDbXref>ISBN:978-92-1-161386-5</oboInOwl:hasDbXref>
        <oboInOwl:hasDbXref>ORCID:0000-0002-4366-3088</oboInOwl:hasDbXref>
    </owl:Axiom>
    


    <!-- http://purl.obolibrary.org/obo/ENVO_01000022 -->

    <owl:Class rdf:about="http://purl.obolibrary.org/obo/ENVO_01000022">
        <rdfs:subClassOf rdf:resource="http://purl.obolibrary.org/obo/ENVO_00000447"/>
        <obo:IAO_0000115>The marine salt marsh biome comprises marshes that are transitional intertidals between land and salty or brackish marine water (e.g.: sloughs, bays, estuaries). It is dominated by halophytic (salt tolerant) herbaceous plants. The daily tidal surges bring in nutrients, which tend to settle in roots of the plants within the salt marsh. The natural chemical activity of salty (or brackish) water and the tendency of algae to bloom in the shallow unshaded water also allow for great biodiversity.</obo:IAO_0000115>
        <oboInOwl:created_by>ORCID:0000-0002-4366-3088</oboInOwl:created_by>
        <oboInOwl:creation_date>2010-03-15T11:17:06Z</oboInOwl:creation_date>
        <oboInOwl:hasOBONamespace>ENVO</oboInOwl:hasOBONamespace>
        <oboInOwl:id>ENVO:01000022</oboInOwl:id>
        <rdfs:label>marine salt marsh biome</rdfs:label>
    </owl:Class>
    <owl:Axiom>
        <owl:annotatedSource rdf:resource="http://purl.obolibrary.org/obo/ENVO_01000022"/>
        <owl:annotatedProperty rdf:resource="http://purl.obolibrary.org/obo/IAO_0000115"/>
        <owl:annotatedTarget>The marine salt marsh biome comprises marshes that are transitional intertidals between land and salty or brackish marine water (e.g.: sloughs, bays, estuaries). It is dominated by halophytic (salt tolerant) herbaceous plants. The daily tidal surges bring in nutrients, which tend to settle in roots of the plants within the salt marsh. The natural chemical activity of salty (or brackish) water and the tendency of algae to bloom in the shallow unshaded water also allow for great biodiversity.</owl:annotatedTarget>
        <oboInOwl:hasDbXref>ORCID:0000-0002-4366-3088</oboInOwl:hasDbXref>
        <oboInOwl:hasDbXref>https://en.wikipedia.org/wiki/Salt_marsh</oboInOwl:hasDbXref>
    </owl:Axiom>
    


    <!-- http://purl.obolibrary.org/obo/ENVO_01000023 -->

    <owl:Class rdf:about="http://purl.obolibrary.org/obo/ENVO_01000023">
        <rdfs:subClassOf rdf:resource="http://purl.obolibrary.org/obo/ENVO_00000447"/>
        <obo:IAO_0000115>The marine pelagic biome (pelagic meaning open sea) is that of the marine water column, from the surface to the greatest depths.</obo:IAO_0000115>
        <oboInOwl:created_by>ORCID:0000-0002-4366-3088</oboInOwl:created_by>
        <oboInOwl:creation_date>2010-03-15T11:17:06Z</oboInOwl:creation_date>
        <oboInOwl:hasOBONamespace>ENVO</oboInOwl:hasOBONamespace>
        <oboInOwl:id>ENVO:01000023</oboInOwl:id>
        <oboInOwl:inSubset>envoPolar</oboInOwl:inSubset>
        <rdfs:label>marine pelagic biome</rdfs:label>
    </owl:Class>
    <owl:Axiom>
        <owl:annotatedSource rdf:resource="http://purl.obolibrary.org/obo/ENVO_01000023"/>
        <owl:annotatedProperty rdf:resource="http://purl.obolibrary.org/obo/IAO_0000115"/>
        <owl:annotatedTarget>The marine pelagic biome (pelagic meaning open sea) is that of the marine water column, from the surface to the greatest depths.</owl:annotatedTarget>
        <oboInOwl:hasDbXref>ISBN:978-0-7506-3384-0</oboInOwl:hasDbXref>
    </owl:Axiom>
    


    <!-- http://purl.obolibrary.org/obo/ENVO_01000024 -->

    <owl:Class rdf:about="http://purl.obolibrary.org/obo/ENVO_01000024">
        <rdfs:subClassOf rdf:resource="http://purl.obolibrary.org/obo/ENVO_00000447"/>
        <obo:IAO_0000115>The marine benthic biome (benthic meaning &apos;bottom&apos;) encompasses the seafloor and includes such areas as shores, littoral or intertidal areas, marine coral reefs, and the deep seabed.</obo:IAO_0000115>
        <oboInOwl:created_by>ORCID:0000-0002-4366-3088</oboInOwl:created_by>
        <oboInOwl:creation_date>2010-03-15T11:17:06Z</oboInOwl:creation_date>
        <oboInOwl:hasDbXref>SPIRE:Benthic</oboInOwl:hasDbXref>
        <oboInOwl:inSubset>envoPolar</oboInOwl:inSubset>
        <rdfs:label>marine benthic biome</rdfs:label>
    </owl:Class>
    <owl:Axiom>
        <owl:annotatedSource rdf:resource="http://purl.obolibrary.org/obo/ENVO_01000024"/>
        <owl:annotatedProperty rdf:resource="http://purl.obolibrary.org/obo/IAO_0000115"/>
        <owl:annotatedTarget>The marine benthic biome (benthic meaning &apos;bottom&apos;) encompasses the seafloor and includes such areas as shores, littoral or intertidal areas, marine coral reefs, and the deep seabed.</owl:annotatedTarget>
        <oboInOwl:hasDbXref>ISBN:978-0-7506-3384-0</oboInOwl:hasDbXref>
        <oboInOwl:hasDbXref>ORCID:0000-0002-4366-3088</oboInOwl:hasDbXref>
    </owl:Axiom>
    


    <!-- http://purl.obolibrary.org/obo/ENVO_01000025 -->

    <owl:Class rdf:about="http://purl.obolibrary.org/obo/ENVO_01000025">
        <rdfs:subClassOf rdf:resource="http://purl.obolibrary.org/obo/ENVO_01000024"/>
        <obo:IAO_0000115>The marine neritic zone biome comprises sea floor from the high tide mark to a continental shelf break. This zone generally extends to 200 m below average sea level.</obo:IAO_0000115>
        <oboInOwl:created_by>ORCID:0000-0002-4366-3088</oboInOwl:created_by>
        <oboInOwl:creation_date>2010-03-15T11:18:40Z</oboInOwl:creation_date>
        <oboInOwl:inSubset>envoPolar</oboInOwl:inSubset>
        <rdfs:label>marine neritic benthic zone biome</rdfs:label>
    </owl:Class>
    <owl:Axiom>
        <owl:annotatedSource rdf:resource="http://purl.obolibrary.org/obo/ENVO_01000025"/>
        <owl:annotatedProperty rdf:resource="http://purl.obolibrary.org/obo/IAO_0000115"/>
        <owl:annotatedTarget>The marine neritic zone biome comprises sea floor from the high tide mark to a continental shelf break. This zone generally extends to 200 m below average sea level.</owl:annotatedTarget>
        <oboInOwl:hasDbXref>ISBN:978-0-444-82619-0</oboInOwl:hasDbXref>
        <oboInOwl:hasDbXref>ISBN:978-0-7506-3384-0</oboInOwl:hasDbXref>
        <oboInOwl:hasDbXref>ORCID:0000-0002-4366-3088</oboInOwl:hasDbXref>
    </owl:Axiom>
    


    <!-- http://purl.obolibrary.org/obo/ENVO_01000026 -->

    <owl:Class rdf:about="http://purl.obolibrary.org/obo/ENVO_01000026">
        <rdfs:subClassOf rdf:resource="http://purl.obolibrary.org/obo/ENVO_01000024"/>
        <obo:IAO_0000115>The marine bathyal zone biome comprises regions of the marine benthic biome between approximately 200 m and 3000 m depth. This zone generally coincides with the continental slope.</obo:IAO_0000115>
        <oboInOwl:created_by>ORCID:0000-0002-4366-3088</oboInOwl:created_by>
        <oboInOwl:creation_date>2010-03-15T11:18:40Z</oboInOwl:creation_date>
        <rdfs:label>marine bathyal zone biome</rdfs:label>
    </owl:Class>
    <owl:Axiom>
        <owl:annotatedSource rdf:resource="http://purl.obolibrary.org/obo/ENVO_01000026"/>
        <owl:annotatedProperty rdf:resource="http://purl.obolibrary.org/obo/IAO_0000115"/>
        <owl:annotatedTarget>The marine bathyal zone biome comprises regions of the marine benthic biome between approximately 200 m and 3000 m depth. This zone generally coincides with the continental slope.</owl:annotatedTarget>
        <oboInOwl:hasDbXref>ISBN:978-0-444-82619-0</oboInOwl:hasDbXref>
        <oboInOwl:hasDbXref>ORCID:0000-0002-4366-3088</oboInOwl:hasDbXref>
    </owl:Axiom>
    


    <!-- http://purl.obolibrary.org/obo/ENVO_01000027 -->

    <owl:Class rdf:about="http://purl.obolibrary.org/obo/ENVO_01000027">
        <rdfs:subClassOf rdf:resource="http://purl.obolibrary.org/obo/ENVO_01000024"/>
        <obo:IAO_0000115>The marine abyssal zone biome comprises regions of the marine benthic biome  between approximately 2500 m and 6000 m depth. This zone generally coincides with the continental rise and the abyssal plain.</obo:IAO_0000115>
        <oboInOwl:created_by>ORCID:0000-0002-4366-3088</oboInOwl:created_by>
        <oboInOwl:creation_date>2010-03-15T11:18:40Z</oboInOwl:creation_date>
        <rdfs:label>marine abyssal zone biome</rdfs:label>
    </owl:Class>
    <owl:Axiom>
        <owl:annotatedSource rdf:resource="http://purl.obolibrary.org/obo/ENVO_01000027"/>
        <owl:annotatedProperty rdf:resource="http://purl.obolibrary.org/obo/IAO_0000115"/>
        <owl:annotatedTarget>The marine abyssal zone biome comprises regions of the marine benthic biome  between approximately 2500 m and 6000 m depth. This zone generally coincides with the continental rise and the abyssal plain.</owl:annotatedTarget>
        <oboInOwl:hasDbXref>ISBN:978-0-444-82619-0</oboInOwl:hasDbXref>
        <oboInOwl:hasDbXref>ORCID:0000-0002-4366-3088</oboInOwl:hasDbXref>
    </owl:Axiom>
    


    <!-- http://purl.obolibrary.org/obo/ENVO_01000028 -->

    <owl:Class rdf:about="http://purl.obolibrary.org/obo/ENVO_01000028">
        <rdfs:subClassOf rdf:resource="http://purl.obolibrary.org/obo/ENVO_01000024"/>
        <obo:IAO_0000115>The marine hadal zone biome describes sea floor deeper than 6000 m such as that of the oceanic trenches.</obo:IAO_0000115>
        <oboInOwl:created_by>ORCID:0000-0002-4366-3088</oboInOwl:created_by>
        <oboInOwl:creation_date>2010-03-15T11:18:40Z</oboInOwl:creation_date>
        <rdfs:label>marine hadal zone biome</rdfs:label>
    </owl:Class>
    <owl:Axiom>
        <owl:annotatedSource rdf:resource="http://purl.obolibrary.org/obo/ENVO_01000028"/>
        <owl:annotatedProperty rdf:resource="http://purl.obolibrary.org/obo/IAO_0000115"/>
        <owl:annotatedTarget>The marine hadal zone biome describes sea floor deeper than 6000 m such as that of the oceanic trenches.</owl:annotatedTarget>
        <oboInOwl:hasDbXref>ISBN:978-0-444-82619-0</oboInOwl:hasDbXref>
        <oboInOwl:hasDbXref>ORCID:0000-0002-4366-3088</oboInOwl:hasDbXref>
    </owl:Axiom>
    


    <!-- http://purl.obolibrary.org/obo/ENVO_01000029 -->

    <owl:Class rdf:about="http://purl.obolibrary.org/obo/ENVO_01000029">
        <rdfs:subClassOf rdf:resource="http://purl.obolibrary.org/obo/ENVO_01000024"/>
        <obo:IAO_0000115>A biome expressed by strips or ridges of rocks, sand, or coral that rises to or near the surface of a body of marine water.</obo:IAO_0000115>
        <oboInOwl:created_by>ORCID:0000-0002-4366-3088</oboInOwl:created_by>
        <oboInOwl:creation_date>2010-03-15T11:18:40Z</oboInOwl:creation_date>
        <rdfs:label>marine reef biome</rdfs:label>
    </owl:Class>
    <owl:Axiom>
        <owl:annotatedSource rdf:resource="http://purl.obolibrary.org/obo/ENVO_01000029"/>
        <owl:annotatedProperty rdf:resource="http://purl.obolibrary.org/obo/IAO_0000115"/>
        <owl:annotatedTarget>A biome expressed by strips or ridges of rocks, sand, or coral that rises to or near the surface of a body of marine water.</owl:annotatedTarget>
        <oboInOwl:hasDbXref>ISBN:978-0-618-45504-1</oboInOwl:hasDbXref>
        <oboInOwl:hasDbXref>ORCID:0000-0002-4366-3088</oboInOwl:hasDbXref>
    </owl:Axiom>
    


    <!-- http://purl.obolibrary.org/obo/ENVO_01000030 -->

    <owl:Class rdf:about="http://purl.obolibrary.org/obo/ENVO_01000030">
        <rdfs:subClassOf rdf:resource="http://purl.obolibrary.org/obo/ENVO_01000024"/>
        <obo:IAO_0000115>The marine hydrothermal vent biome comprises regions of the marine benthic biome where heat generated due to tectonic activity, either at divergent plate boundaries or convergent ocean plates where back-arc spreading occurs, is released or &apos;vented&apos; to the surface. The resultant high temperature water jets are laden with dissolved metals and minerals.</obo:IAO_0000115>
        <oboInOwl:created_by>ORCID:0000-0002-4366-3088</oboInOwl:created_by>
        <oboInOwl:creation_date>2010-03-15T11:18:40Z</oboInOwl:creation_date>
        <rdfs:label>marine hydrothermal vent biome</rdfs:label>
    </owl:Class>
    <owl:Axiom>
        <owl:annotatedSource rdf:resource="http://purl.obolibrary.org/obo/ENVO_01000030"/>
        <owl:annotatedProperty rdf:resource="http://purl.obolibrary.org/obo/IAO_0000115"/>
        <owl:annotatedTarget>The marine hydrothermal vent biome comprises regions of the marine benthic biome where heat generated due to tectonic activity, either at divergent plate boundaries or convergent ocean plates where back-arc spreading occurs, is released or &apos;vented&apos; to the surface. The resultant high temperature water jets are laden with dissolved metals and minerals.</owl:annotatedTarget>
        <oboInOwl:hasDbXref>ISBN:978-0-444-82619-0</oboInOwl:hasDbXref>
        <oboInOwl:hasDbXref>ORCID:0000-0002-4366-3088</oboInOwl:hasDbXref>
    </owl:Axiom>
    


    <!-- http://purl.obolibrary.org/obo/ENVO_01000032 -->

    <owl:Class rdf:about="http://purl.obolibrary.org/obo/ENVO_01000032">
        <rdfs:subClassOf rdf:resource="http://purl.obolibrary.org/obo/ENVO_01000023"/>
        <owl:disjointWith rdf:resource="http://purl.obolibrary.org/obo/ENVO_01000033"/>
        <obo:IAO_0000115>The neritic epipelagic zone biome comprises the marine water column above a continental shelf.</obo:IAO_0000115>
        <oboInOwl:created_by>ORCID:0000-0002-4366-3088</oboInOwl:created_by>
        <oboInOwl:creation_date>2010-03-15T11:19:19Z</oboInOwl:creation_date>
        <oboInOwl:hasOBONamespace>ENVO</oboInOwl:hasOBONamespace>
        <oboInOwl:id>ENVO:01000032</oboInOwl:id>
        <rdfs:label>neritic pelagic zone biome</rdfs:label>
    </owl:Class>
    <owl:Axiom>
        <owl:annotatedSource rdf:resource="http://purl.obolibrary.org/obo/ENVO_01000032"/>
        <owl:annotatedProperty rdf:resource="http://purl.obolibrary.org/obo/IAO_0000115"/>
        <owl:annotatedTarget>The neritic epipelagic zone biome comprises the marine water column above a continental shelf.</owl:annotatedTarget>
        <oboInOwl:hasDbXref>ISBN:978-0-444-82619-0</oboInOwl:hasDbXref>
        <oboInOwl:hasDbXref>ISBN:978-0-7506-3384-0</oboInOwl:hasDbXref>
        <oboInOwl:hasDbXref>ORCID:0000-0002-4366-3088</oboInOwl:hasDbXref>
    </owl:Axiom>
    


    <!-- http://purl.obolibrary.org/obo/ENVO_01000033 -->

    <owl:Class rdf:about="http://purl.obolibrary.org/obo/ENVO_01000033">
        <rdfs:subClassOf rdf:resource="http://purl.obolibrary.org/obo/ENVO_01000023"/>
        <obo:IAO_0000115>The oceanic epipelagic zone biome comprises the marine water column offshore, beyond a continental shelf.</obo:IAO_0000115>
        <oboInOwl:created_by>ORCID:0000-0002-4366-3088</oboInOwl:created_by>
        <oboInOwl:creation_date>2010-03-15T11:19:19Z</oboInOwl:creation_date>
        <oboInOwl:hasOBONamespace>ENVO</oboInOwl:hasOBONamespace>
        <oboInOwl:id>ENVO:01000033</oboInOwl:id>
        <rdfs:label>oceanic pelagic zone biome</rdfs:label>
    </owl:Class>
    <owl:Axiom>
        <owl:annotatedSource rdf:resource="http://purl.obolibrary.org/obo/ENVO_01000033"/>
        <owl:annotatedProperty rdf:resource="http://purl.obolibrary.org/obo/IAO_0000115"/>
        <owl:annotatedTarget>The oceanic epipelagic zone biome comprises the marine water column offshore, beyond a continental shelf.</owl:annotatedTarget>
        <oboInOwl:hasDbXref>ISBN:978-0-444-82619-0</oboInOwl:hasDbXref>
        <oboInOwl:hasDbXref>ISBN:978-0-7506-3384-0</oboInOwl:hasDbXref>
        <oboInOwl:hasDbXref>ORCID:0000-0002-4366-3088</oboInOwl:hasDbXref>
    </owl:Axiom>
    


    <!-- http://purl.obolibrary.org/obo/ENVO_01000034 -->

    <owl:Class rdf:about="http://purl.obolibrary.org/obo/ENVO_01000034">
        <rdfs:subClassOf rdf:resource="http://purl.obolibrary.org/obo/ENVO_01000033"/>
        <obo:IAO_0000115>The oceanic sea surface microlayer (SML) biome comprises the top 1000 micrometers of the marine surface waters occurring offshore, away from a continental shelf. It is the boundary layer where all exchange occurs between the atmosphere and the ocean. The chemical, physical, and biological properties of the SML differ greatly from the sub-surface water just a few centimeters beneath.</obo:IAO_0000115>
        <oboInOwl:created_by>ORCID:0000-0002-4366-3088</oboInOwl:created_by>
        <oboInOwl:creation_date>2010-03-15T11:21:03Z</oboInOwl:creation_date>
        <oboInOwl:hasOBONamespace>ENVO</oboInOwl:hasOBONamespace>
        <oboInOwl:id>ENVO:01000034</oboInOwl:id>
        <rdfs:label>oceanic sea surface microlayer biome</rdfs:label>
    </owl:Class>
    <owl:Axiom>
        <owl:annotatedSource rdf:resource="http://purl.obolibrary.org/obo/ENVO_01000034"/>
        <owl:annotatedProperty rdf:resource="http://purl.obolibrary.org/obo/IAO_0000115"/>
        <owl:annotatedTarget>The oceanic sea surface microlayer (SML) biome comprises the top 1000 micrometers of the marine surface waters occurring offshore, away from a continental shelf. It is the boundary layer where all exchange occurs between the atmosphere and the ocean. The chemical, physical, and biological properties of the SML differ greatly from the sub-surface water just a few centimeters beneath.</owl:annotatedTarget>
        <oboInOwl:hasDbXref>ORCID:0000-0002-4366-3088</oboInOwl:hasDbXref>
        <oboInOwl:hasDbXref>https://en.wikipedia.org/wiki/Sea_surface_microlayer</oboInOwl:hasDbXref>
    </owl:Axiom>
    


    <!-- http://purl.obolibrary.org/obo/ENVO_01000035 -->

    <owl:Class rdf:about="http://purl.obolibrary.org/obo/ENVO_01000035">
        <rdfs:subClassOf rdf:resource="http://purl.obolibrary.org/obo/ENVO_01000033"/>
        <obo:IAO_0000115>The oceanic epipelagic zone biome comprises regions of the marine water column that occur offshore, beyond a continental shelf. This biome extends from the surface of the ocean to a depth of ca. 200-250m. Throughout the zone the light field tends to be asymmetrical vertically, so that the direction and elevation of the sun can still be detected. The oceanic epipelagic zone biome encompasses the euphotic zone and, where and when it occurs, the seasonal thermocline.</obo:IAO_0000115>
        <oboInOwl:created_by>ORCID:0000-0002-4366-3088</oboInOwl:created_by>
        <oboInOwl:creation_date>2010-03-15T11:21:03Z</oboInOwl:creation_date>
        <oboInOwl:hasOBONamespace>ENVO</oboInOwl:hasOBONamespace>
        <oboInOwl:id>ENVO:01000035</oboInOwl:id>
        <rdfs:label>oceanic epipelagic zone biome</rdfs:label>
    </owl:Class>
    <owl:Axiom>
        <owl:annotatedSource rdf:resource="http://purl.obolibrary.org/obo/ENVO_01000035"/>
        <owl:annotatedProperty rdf:resource="http://purl.obolibrary.org/obo/IAO_0000115"/>
        <owl:annotatedTarget>The oceanic epipelagic zone biome comprises regions of the marine water column that occur offshore, beyond a continental shelf. This biome extends from the surface of the ocean to a depth of ca. 200-250m. Throughout the zone the light field tends to be asymmetrical vertically, so that the direction and elevation of the sun can still be detected. The oceanic epipelagic zone biome encompasses the euphotic zone and, where and when it occurs, the seasonal thermocline.</owl:annotatedTarget>
        <oboInOwl:hasDbXref>ISBN:978-0-444-82619-0</oboInOwl:hasDbXref>
        <oboInOwl:hasDbXref>ORCID:0000-0002-4366-3088</oboInOwl:hasDbXref>
    </owl:Axiom>
    


    <!-- http://purl.obolibrary.org/obo/ENVO_01000036 -->

    <owl:Class rdf:about="http://purl.obolibrary.org/obo/ENVO_01000036">
        <rdfs:subClassOf rdf:resource="http://purl.obolibrary.org/obo/ENVO_01000033"/>
        <obo:IAO_0000115>The oceanic mesopelagic zone biome comprises regions of the marine water column that occur offshore, beyond a continental shelf. This biome extends through the water column from approximately 200-1000 m depth - the maximal depth of light penetration in all but the clearest oligotrophic ocean regions. In comparison to the epipelagic zone, dominant forms of pelagic organisms do not change very much; however, there are marked changes in species composition and the proportion of smaller-sized individuals decreases.</obo:IAO_0000115>
        <oboInOwl:created_by>ORCID:0000-0002-4366-3088</oboInOwl:created_by>
        <oboInOwl:creation_date>2010-03-15T11:21:03Z</oboInOwl:creation_date>
        <oboInOwl:hasOBONamespace>ENVO</oboInOwl:hasOBONamespace>
        <oboInOwl:id>ENVO:01000036</oboInOwl:id>
        <rdfs:label>oceanic mesopelagic zone biome</rdfs:label>
    </owl:Class>
    <owl:Axiom>
        <owl:annotatedSource rdf:resource="http://purl.obolibrary.org/obo/ENVO_01000036"/>
        <owl:annotatedProperty rdf:resource="http://purl.obolibrary.org/obo/IAO_0000115"/>
        <owl:annotatedTarget>The oceanic mesopelagic zone biome comprises regions of the marine water column that occur offshore, beyond a continental shelf. This biome extends through the water column from approximately 200-1000 m depth - the maximal depth of light penetration in all but the clearest oligotrophic ocean regions. In comparison to the epipelagic zone, dominant forms of pelagic organisms do not change very much; however, there are marked changes in species composition and the proportion of smaller-sized individuals decreases.</owl:annotatedTarget>
        <oboInOwl:hasDbXref>ISBN:978-0-444-82619-0</oboInOwl:hasDbXref>
        <oboInOwl:hasDbXref>ORCID:0000-0002-4366-3088</oboInOwl:hasDbXref>
    </owl:Axiom>
    


    <!-- http://purl.obolibrary.org/obo/ENVO_01000037 -->

    <owl:Class rdf:about="http://purl.obolibrary.org/obo/ENVO_01000037">
        <rdfs:subClassOf rdf:resource="http://purl.obolibrary.org/obo/ENVO_01000033"/>
        <obo:IAO_0000115>The bathypelagic zone biome comprises the marine water column below approximately 1000 m water depth - the maximum depth to which detectable daylight penetrates in all but the clearest oligotrophic waters - and extends to about 2500 - 2700 m water depth. In the temperate Atlantic, the beginning of the bathypelagic zone biome approximates to the deep oxygen minimum and the base of the permanent thermocline.</obo:IAO_0000115>
        <oboInOwl:created_by>ORCID:0000-0002-4366-3088</oboInOwl:created_by>
        <oboInOwl:creation_date>2010-03-15T11:21:03Z</oboInOwl:creation_date>
        <oboInOwl:hasOBONamespace>ENVO</oboInOwl:hasOBONamespace>
        <oboInOwl:id>ENVO:01000037</oboInOwl:id>
        <rdfs:label>oceanic bathypelagic zone biome</rdfs:label>
    </owl:Class>
    <owl:Axiom>
        <owl:annotatedSource rdf:resource="http://purl.obolibrary.org/obo/ENVO_01000037"/>
        <owl:annotatedProperty rdf:resource="http://purl.obolibrary.org/obo/IAO_0000115"/>
        <owl:annotatedTarget>The bathypelagic zone biome comprises the marine water column below approximately 1000 m water depth - the maximum depth to which detectable daylight penetrates in all but the clearest oligotrophic waters - and extends to about 2500 - 2700 m water depth. In the temperate Atlantic, the beginning of the bathypelagic zone biome approximates to the deep oxygen minimum and the base of the permanent thermocline.</owl:annotatedTarget>
        <oboInOwl:hasDbXref>ISBN:978-0-444-82619-0</oboInOwl:hasDbXref>
        <oboInOwl:hasDbXref>ORCID:0000-0002-4366-3088</oboInOwl:hasDbXref>
    </owl:Axiom>
    


    <!-- http://purl.obolibrary.org/obo/ENVO_01000038 -->

    <owl:Class rdf:about="http://purl.obolibrary.org/obo/ENVO_01000038">
        <rdfs:subClassOf rdf:resource="http://purl.obolibrary.org/obo/ENVO_01000033"/>
        <obo:IAO_0000115>The abyssopelagic zone biome comprises the marine water column below the bathypelagic zone biome at approximately 2500 -2700 m and extends either to the hadal pelagic zone biome (at approximately 6000 m) or to the benthopelagic zone biome within ca. 100 m of the seafloor. The depth of 2700 m may be critical for physiological reasons as the change in hydrostatic pressure across this depth may preclude organism migration.</obo:IAO_0000115>
        <oboInOwl:created_by>ORCID:0000-0002-4366-3088</oboInOwl:created_by>
        <oboInOwl:creation_date>2010-03-15T11:21:03Z</oboInOwl:creation_date>
        <oboInOwl:hasOBONamespace>ENVO</oboInOwl:hasOBONamespace>
        <oboInOwl:id>ENVO:01000038</oboInOwl:id>
        <rdfs:label>oceanic abyssopelagic zone biome</rdfs:label>
    </owl:Class>
    <owl:Axiom>
        <owl:annotatedSource rdf:resource="http://purl.obolibrary.org/obo/ENVO_01000038"/>
        <owl:annotatedProperty rdf:resource="http://purl.obolibrary.org/obo/IAO_0000115"/>
        <owl:annotatedTarget>The abyssopelagic zone biome comprises the marine water column below the bathypelagic zone biome at approximately 2500 -2700 m and extends either to the hadal pelagic zone biome (at approximately 6000 m) or to the benthopelagic zone biome within ca. 100 m of the seafloor. The depth of 2700 m may be critical for physiological reasons as the change in hydrostatic pressure across this depth may preclude organism migration.</owl:annotatedTarget>
        <oboInOwl:hasDbXref>ISBN:978-0-444-82619-0</oboInOwl:hasDbXref>
        <oboInOwl:hasDbXref>ORCID:0000-0002-4366-3088</oboInOwl:hasDbXref>
    </owl:Axiom>
    


    <!-- http://purl.obolibrary.org/obo/ENVO_01000039 -->

    <owl:Class rdf:about="http://purl.obolibrary.org/obo/ENVO_01000039">
        <rdfs:subClassOf rdf:resource="http://purl.obolibrary.org/obo/ENVO_01000033"/>
        <obo:IAO_0000115>The oceanic hadal pelagic zone biome comprises the water column in oceanic trenches occurring at depths between 6000m and 10,000m.</obo:IAO_0000115>
        <oboInOwl:created_by>ORCID:0000-0002-4366-3088</oboInOwl:created_by>
        <oboInOwl:creation_date>2010-03-15T11:21:03Z</oboInOwl:creation_date>
        <oboInOwl:hasOBONamespace>ENVO</oboInOwl:hasOBONamespace>
        <oboInOwl:id>ENVO:01000039</oboInOwl:id>
        <rdfs:label>oceanic hadal pelagic zone biome</rdfs:label>
    </owl:Class>
    <owl:Axiom>
        <owl:annotatedSource rdf:resource="http://purl.obolibrary.org/obo/ENVO_01000039"/>
        <owl:annotatedProperty rdf:resource="http://purl.obolibrary.org/obo/IAO_0000115"/>
        <owl:annotatedTarget>The oceanic hadal pelagic zone biome comprises the water column in oceanic trenches occurring at depths between 6000m and 10,000m.</owl:annotatedTarget>
        <oboInOwl:hasDbXref>ISBN:978-0-444-82619-0</oboInOwl:hasDbXref>
        <oboInOwl:hasDbXref>ORCID:0000-0002-4366-3088</oboInOwl:hasDbXref>
    </owl:Axiom>
    


    <!-- http://purl.obolibrary.org/obo/ENVO_01000040 -->

    <owl:Class rdf:about="http://purl.obolibrary.org/obo/ENVO_01000040">
        <rdfs:subClassOf rdf:resource="http://purl.obolibrary.org/obo/ENVO_01000033"/>
        <obo:IAO_0000115>The benthopelagic zone biome comprises regions of the marine water column which usually coincide with the benthic boundary layer (BBL) - the layer of isothermal and isohaline water contiguous to the sea floor. A general reversal in the declining gradient of pelagic biomass may be observed here, perhaps explained by viable nutrition on the sea floor being resuspended by bottom currents. This zone typically extends 100 m above the seafloor, but may reach upto1000 m during benthic storms.</obo:IAO_0000115>
        <oboInOwl:created_by>ORCID:0000-0002-4366-3088</oboInOwl:created_by>
        <oboInOwl:creation_date>2010-03-15T11:21:03Z</oboInOwl:creation_date>
        <oboInOwl:hasOBONamespace>ENVO</oboInOwl:hasOBONamespace>
        <oboInOwl:id>ENVO:01000040</oboInOwl:id>
        <rdfs:label>oceanic benthopelagic zone biome</rdfs:label>
    </owl:Class>
    <owl:Axiom>
        <owl:annotatedSource rdf:resource="http://purl.obolibrary.org/obo/ENVO_01000040"/>
        <owl:annotatedProperty rdf:resource="http://purl.obolibrary.org/obo/IAO_0000115"/>
        <owl:annotatedTarget>The benthopelagic zone biome comprises regions of the marine water column which usually coincide with the benthic boundary layer (BBL) - the layer of isothermal and isohaline water contiguous to the sea floor. A general reversal in the declining gradient of pelagic biomass may be observed here, perhaps explained by viable nutrition on the sea floor being resuspended by bottom currents. This zone typically extends 100 m above the seafloor, but may reach upto1000 m during benthic storms.</owl:annotatedTarget>
        <oboInOwl:hasDbXref>ISBN:978-0-444-82619-0</oboInOwl:hasDbXref>
        <oboInOwl:hasDbXref>ORCID:0000-0002-4366-3088</oboInOwl:hasDbXref>
    </owl:Axiom>
    


    <!-- http://purl.obolibrary.org/obo/ENVO_01000041 -->

    <owl:Class rdf:about="http://purl.obolibrary.org/obo/ENVO_01000041">
        <rdfs:subClassOf rdf:resource="http://purl.obolibrary.org/obo/ENVO_01000032"/>
        <obo:IAO_0000115>The neritic sea surface microlayer (SML) biome comprises the top 1000 micrometers of marine surface waters occurring above a continental shelf. It is the boundary layer where all exchange occurs between the atmosphere and the ocean. The chemical, physical, and biological properties of the SML differ greatly from the sub-surface water just a few centimeters beneath.</obo:IAO_0000115>
        <oboInOwl:created_by>ORCID:0000-0002-4366-3088</oboInOwl:created_by>
        <oboInOwl:creation_date>2010-03-15T11:22:09Z</oboInOwl:creation_date>
        <oboInOwl:hasOBONamespace>ENVO</oboInOwl:hasOBONamespace>
        <oboInOwl:id>ENVO:01000041</oboInOwl:id>
        <rdfs:label>neritic sea surface microlayer biome</rdfs:label>
    </owl:Class>
    <owl:Axiom>
        <owl:annotatedSource rdf:resource="http://purl.obolibrary.org/obo/ENVO_01000041"/>
        <owl:annotatedProperty rdf:resource="http://purl.obolibrary.org/obo/IAO_0000115"/>
        <owl:annotatedTarget>The neritic sea surface microlayer (SML) biome comprises the top 1000 micrometers of marine surface waters occurring above a continental shelf. It is the boundary layer where all exchange occurs between the atmosphere and the ocean. The chemical, physical, and biological properties of the SML differ greatly from the sub-surface water just a few centimeters beneath.</owl:annotatedTarget>
        <oboInOwl:hasDbXref>ORCID:0000-0002-4366-3088</oboInOwl:hasDbXref>
        <oboInOwl:hasDbXref>https://en.wikipedia.org/wiki/Sea_surface_microlayer</oboInOwl:hasDbXref>
    </owl:Axiom>
    


    <!-- http://purl.obolibrary.org/obo/ENVO_01000042 -->

    <owl:Class rdf:about="http://purl.obolibrary.org/obo/ENVO_01000042">
        <rdfs:subClassOf rdf:resource="http://purl.obolibrary.org/obo/ENVO_01000032"/>
        <obo:IAO_0000115>The neritic epipelagic zone biome comprises the marine water column that occurs above a continental shelf and extends from the surface of the ocean to a depth of ca. 200-250m. Throughout the zone the light field tends to be asymmetrical vertically, so that the direction and elevation of the sun can still be detected. The epipelagic zone encompasses the euphotic zone and, where and when it occurs, the seasonal thermocline.</obo:IAO_0000115>
        <oboInOwl:created_by>ORCID:0000-0002-4366-3088</oboInOwl:created_by>
        <oboInOwl:creation_date>2010-03-15T11:22:09Z</oboInOwl:creation_date>
        <oboInOwl:hasOBONamespace>ENVO</oboInOwl:hasOBONamespace>
        <oboInOwl:id>ENVO:01000042</oboInOwl:id>
        <rdfs:label>neritic epipelagic zone biome</rdfs:label>
    </owl:Class>
    <owl:Axiom>
        <owl:annotatedSource rdf:resource="http://purl.obolibrary.org/obo/ENVO_01000042"/>
        <owl:annotatedProperty rdf:resource="http://purl.obolibrary.org/obo/IAO_0000115"/>
        <owl:annotatedTarget>The neritic epipelagic zone biome comprises the marine water column that occurs above a continental shelf and extends from the surface of the ocean to a depth of ca. 200-250m. Throughout the zone the light field tends to be asymmetrical vertically, so that the direction and elevation of the sun can still be detected. The epipelagic zone encompasses the euphotic zone and, where and when it occurs, the seasonal thermocline.</owl:annotatedTarget>
        <oboInOwl:hasDbXref>ISBN:978-0-444-82619-0</oboInOwl:hasDbXref>
        <oboInOwl:hasDbXref>ORCID:0000-0002-4366-3088</oboInOwl:hasDbXref>
    </owl:Axiom>
    


    <!-- http://purl.obolibrary.org/obo/ENVO_01000043 -->

    <owl:Class rdf:about="http://purl.obolibrary.org/obo/ENVO_01000043">
        <rdfs:subClassOf rdf:resource="http://purl.obolibrary.org/obo/ENVO_01000032"/>
        <obo:IAO_0000115>The neritic mesopelagic zone biome comprises the marine column that occurs above a continental shelf and extends from approximately 200 to 1000 m depth - the maximal depth of light penetration in all but the clearest oligotrophic ocean regions. In comparison to the epipelagic zone, dominant forms of pelagic organisms do not change very much; however, there are marked changes in species composition and the proportion of smaller-sized individuals decreases.</obo:IAO_0000115>
        <oboInOwl:created_by>ORCID:0000-0002-4366-3088</oboInOwl:created_by>
        <oboInOwl:creation_date>2010-03-15T11:22:09Z</oboInOwl:creation_date>
        <rdfs:label>neritic mesopelagic zone biome</rdfs:label>
    </owl:Class>
    <owl:Axiom>
        <owl:annotatedSource rdf:resource="http://purl.obolibrary.org/obo/ENVO_01000043"/>
        <owl:annotatedProperty rdf:resource="http://purl.obolibrary.org/obo/IAO_0000115"/>
        <owl:annotatedTarget>The neritic mesopelagic zone biome comprises the marine column that occurs above a continental shelf and extends from approximately 200 to 1000 m depth - the maximal depth of light penetration in all but the clearest oligotrophic ocean regions. In comparison to the epipelagic zone, dominant forms of pelagic organisms do not change very much; however, there are marked changes in species composition and the proportion of smaller-sized individuals decreases.</owl:annotatedTarget>
        <oboInOwl:hasDbXref>ISBN:978-0-444-82619-0</oboInOwl:hasDbXref>
        <oboInOwl:hasDbXref>ORCID:0000-0002-4366-3088</oboInOwl:hasDbXref>
    </owl:Axiom>
    


    <!-- http://purl.obolibrary.org/obo/ENVO_01000045 -->

    <owl:Class rdf:about="http://purl.obolibrary.org/obo/ENVO_01000045">
        <rdfs:subClassOf rdf:resource="http://purl.obolibrary.org/obo/ENVO_00000447"/>
        <obo:IAO_0000115>The epeiric sea (also known as an epicontinental sea) biome comprises a shallow seas that extend over part of a continent. Epeiric seas are usually associated with the marine transgressions of the geologic  past, which have variously been due to either global eustatic sea level changes, local tectonic deformation, or both, and are occasionally semi-cyclic.</obo:IAO_0000115>
        <oboInOwl:created_by>ORCID:0000-0002-4366-3088</oboInOwl:created_by>
        <oboInOwl:creation_date>2010-03-15T11:23:23Z</oboInOwl:creation_date>
        <oboInOwl:hasExactSynonym>epicontinental sea biome</oboInOwl:hasExactSynonym>
        <rdfs:label>epeiric sea biome</rdfs:label>
    </owl:Class>
    <owl:Axiom>
        <owl:annotatedSource rdf:resource="http://purl.obolibrary.org/obo/ENVO_01000045"/>
        <owl:annotatedProperty rdf:resource="http://purl.obolibrary.org/obo/IAO_0000115"/>
        <owl:annotatedTarget>The epeiric sea (also known as an epicontinental sea) biome comprises a shallow seas that extend over part of a continent. Epeiric seas are usually associated with the marine transgressions of the geologic  past, which have variously been due to either global eustatic sea level changes, local tectonic deformation, or both, and are occasionally semi-cyclic.</owl:annotatedTarget>
        <oboInOwl:hasDbXref>ORCID:0000-0002-4366-3088</oboInOwl:hasDbXref>
        <oboInOwl:hasDbXref>https://en.wikipedia.org/wiki/Epeiric_sea</oboInOwl:hasDbXref>
    </owl:Axiom>
    <owl:Axiom>
        <owl:annotatedSource rdf:resource="http://purl.obolibrary.org/obo/ENVO_01000045"/>
        <owl:annotatedProperty rdf:resource="http://www.geneontology.org/formats/oboInOwl#hasExactSynonym"/>
        <owl:annotatedTarget>epicontinental sea biome</owl:annotatedTarget>
        <oboInOwl:hasDbXref>https://en.wikipedia.org/wiki/Epeiric_sea</oboInOwl:hasDbXref>
    </owl:Axiom>
    


    <!-- http://purl.obolibrary.org/obo/ENVO_01000046 -->

    <owl:Class rdf:about="http://purl.obolibrary.org/obo/ENVO_01000046">
        <rdfs:subClassOf rdf:resource="http://purl.obolibrary.org/obo/ENVO_00000447"/>
        <obo:IAO_0000115>The marginal sea biome comprises parts of an ocean partially enclosed by land such as islands, archipelagos, or peninsulas. Unlike mediterranean seas, marginal seas have ocean currents caused by ocean winds. Many marginal seas are enclosed by island arcs that were formed from the subduction of one oceanic plate beneath another.</obo:IAO_0000115>
        <oboInOwl:created_by>ORCID:0000-0002-4366-3088</oboInOwl:created_by>
        <oboInOwl:creation_date>2010-03-15T11:23:23Z</oboInOwl:creation_date>
        <rdfs:label>marginal sea biome</rdfs:label>
    </owl:Class>
    <owl:Axiom>
        <owl:annotatedSource rdf:resource="http://purl.obolibrary.org/obo/ENVO_01000046"/>
        <owl:annotatedProperty rdf:resource="http://purl.obolibrary.org/obo/IAO_0000115"/>
        <owl:annotatedTarget>The marginal sea biome comprises parts of an ocean partially enclosed by land such as islands, archipelagos, or peninsulas. Unlike mediterranean seas, marginal seas have ocean currents caused by ocean winds. Many marginal seas are enclosed by island arcs that were formed from the subduction of one oceanic plate beneath another.</owl:annotatedTarget>
        <oboInOwl:hasDbXref>ORCID:0000-0002-4366-3088</oboInOwl:hasDbXref>
        <oboInOwl:hasDbXref>https://en.wikipedia.org/wiki/Marginal_sea</oboInOwl:hasDbXref>
    </owl:Axiom>
    


    <!-- http://purl.obolibrary.org/obo/ENVO_01000047 -->

    <owl:Class rdf:about="http://purl.obolibrary.org/obo/ENVO_01000047">
        <rdfs:subClassOf rdf:resource="http://purl.obolibrary.org/obo/ENVO_00000447"/>
        <rdfs:subClassOf rdf:resource="http://purl.obolibrary.org/obo/ENVO_01001833"/>
        <obo:IAO_0000115>The mediterranean sea biome comprises mostly enclosed seas that have limited exchange of deep water with outer oceans and where the water circulation is dominated by salinity and temperature differences rather than winds.</obo:IAO_0000115>
        <oboInOwl:created_by>ORCID:0000-0002-4366-3088</oboInOwl:created_by>
        <oboInOwl:creation_date>2010-03-15T11:23:23Z</oboInOwl:creation_date>
        <rdfs:label>mediterranean sea biome</rdfs:label>
    </owl:Class>
    <owl:Axiom>
        <owl:annotatedSource rdf:resource="http://purl.obolibrary.org/obo/ENVO_01000047"/>
        <owl:annotatedProperty rdf:resource="http://purl.obolibrary.org/obo/IAO_0000115"/>
        <owl:annotatedTarget>The mediterranean sea biome comprises mostly enclosed seas that have limited exchange of deep water with outer oceans and where the water circulation is dominated by salinity and temperature differences rather than winds.</owl:annotatedTarget>
        <oboInOwl:hasDbXref>ORCID:0000-0002-4366-3088</oboInOwl:hasDbXref>
        <oboInOwl:hasDbXref>https://en.wikipedia.org/wiki/Mediterranean_sea</oboInOwl:hasDbXref>
    </owl:Axiom>
    


    <!-- http://purl.obolibrary.org/obo/ENVO_01000048 -->

    <owl:Class rdf:about="http://purl.obolibrary.org/obo/ENVO_01000048">
        <rdfs:subClassOf rdf:resource="http://purl.obolibrary.org/obo/ENVO_00000447"/>
        <obo:IAO_0000115>A marine biome which is determined by an ocean.</obo:IAO_0000115>
        <oboInOwl:created_by>ORCID:0000-0002-4366-3088</oboInOwl:created_by>
        <oboInOwl:creation_date>2010-03-15T11:23:23Z</oboInOwl:creation_date>
        <oboInOwl:inSubset>envoPolar</oboInOwl:inSubset>
        <rdfs:comment>Ocean biomes are determined by major bodies of saline water, principal components of the hydrosphere. Approximately 71% of the Earth&apos;s surface is covered by ocean, a continuous body of water that is customarily divided into several principal oceans and smaller seas. More than half of this area is over 3,000 metres (9,800 ft) deep. Average oceanic salinity is around 35 parts per thousand (ppt) (3.5%), and nearly all seawater has a salinity in the range of 30 to 38 ppt.</rdfs:comment>
        <rdfs:label>ocean biome</rdfs:label>
    </owl:Class>
    <owl:Axiom>
        <owl:annotatedSource rdf:resource="http://purl.obolibrary.org/obo/ENVO_01000048"/>
        <owl:annotatedProperty rdf:resource="http://purl.obolibrary.org/obo/IAO_0000115"/>
        <owl:annotatedTarget>A marine biome which is determined by an ocean.</owl:annotatedTarget>
        <oboInOwl:hasDbXref>ORCID:0000-0002-4366-3088</oboInOwl:hasDbXref>
        <oboInOwl:hasDbXref>https://en.wikipedia.org/wiki/Ocean</oboInOwl:hasDbXref>
    </owl:Axiom>
    


    <!-- http://purl.obolibrary.org/obo/ENVO_01000049 -->

    <owl:Class rdf:about="http://purl.obolibrary.org/obo/ENVO_01000049">
        <rdfs:subClassOf rdf:resource="http://purl.obolibrary.org/obo/ENVO_01000029"/>
        <obo:IAO_0000115>The marine coral reef biome comprises constructional wave-resistant entities which are primarily built by corals and are often cemented together. The growth of these structures is aided by zooxanthellae, algae that are symbiotic with the reef-building corals.</obo:IAO_0000115>
        <oboInOwl:created_by>ORCID:0000-0002-4366-3088</oboInOwl:created_by>
        <oboInOwl:creation_date>2010-03-15T11:27:06Z</oboInOwl:creation_date>
        <oboInOwl:hasOBONamespace>ENVO</oboInOwl:hasOBONamespace>
        <oboInOwl:id>ENVO:01000049</oboInOwl:id>
        <rdfs:label>marine coral reef biome</rdfs:label>
    </owl:Class>
    <owl:Axiom>
        <owl:annotatedSource rdf:resource="http://purl.obolibrary.org/obo/ENVO_01000049"/>
        <owl:annotatedProperty rdf:resource="http://purl.obolibrary.org/obo/IAO_0000115"/>
        <owl:annotatedTarget>The marine coral reef biome comprises constructional wave-resistant entities which are primarily built by corals and are often cemented together. The growth of these structures is aided by zooxanthellae, algae that are symbiotic with the reef-building corals.</owl:annotatedTarget>
        <oboInOwl:hasDbXref>ISBN:978-0-7506-3384-0</oboInOwl:hasDbXref>
        <oboInOwl:hasDbXref>ORCID:0000-0002-4366-3088</oboInOwl:hasDbXref>
    </owl:Axiom>
    


    <!-- http://purl.obolibrary.org/obo/ENVO_01000050 -->

    <owl:Class rdf:about="http://purl.obolibrary.org/obo/ENVO_01000050">
        <rdfs:subClassOf rdf:resource="http://purl.obolibrary.org/obo/ENVO_01000029"/>
        <obo:IAO_0000115>The marine rocky subtidal reef biome comprises regions of the marine reef biome composed mainly of rock and which harbour abundant communities of algae and invertebrates. These reefs are often very patchy, with alterations of rocks dominated by rich invertebrate assemblages and turf-forming calcareous red algae.</obo:IAO_0000115>
        <oboInOwl:created_by>ORCID:0000-0002-4366-3088</oboInOwl:created_by>
        <oboInOwl:creation_date>2010-03-15T11:27:06Z</oboInOwl:creation_date>
        <oboInOwl:hasOBONamespace>ENVO</oboInOwl:hasOBONamespace>
        <oboInOwl:id>ENVO:01000050</oboInOwl:id>
        <rdfs:label>marine subtidal rocky reef biome</rdfs:label>
    </owl:Class>
    <owl:Axiom>
        <owl:annotatedSource rdf:resource="http://purl.obolibrary.org/obo/ENVO_01000050"/>
        <owl:annotatedProperty rdf:resource="http://purl.obolibrary.org/obo/IAO_0000115"/>
        <owl:annotatedTarget>The marine rocky subtidal reef biome comprises regions of the marine reef biome composed mainly of rock and which harbour abundant communities of algae and invertebrates. These reefs are often very patchy, with alterations of rocks dominated by rich invertebrate assemblages and turf-forming calcareous red algae.</owl:annotatedTarget>
        <oboInOwl:hasDbXref>ISBN:978-0-7506-3384-0</oboInOwl:hasDbXref>
        <oboInOwl:hasDbXref>ORCID:0000-0002-4366-3088</oboInOwl:hasDbXref>
    </owl:Axiom>
    


    <!-- http://purl.obolibrary.org/obo/ENVO_01000051 -->

    <owl:Class rdf:about="http://purl.obolibrary.org/obo/ENVO_01000051">
        <rdfs:subClassOf rdf:resource="http://purl.obolibrary.org/obo/ENVO_01000030"/>
        <obo:IAO_0000115>A marine black smoker biome comprises regions of the marine hydrothermal vent biome characterised by a black vent plume. This black plume is a consequence of dissolved metals and minerals forming complexes with sulphide and indicates polymetallic sulphide mineral deposits beneath the surface.</obo:IAO_0000115>
        <oboInOwl:created_by>ORCID:0000-0002-4366-3088</oboInOwl:created_by>
        <oboInOwl:creation_date>2010-03-15T11:29:37Z</oboInOwl:creation_date>
        <oboInOwl:hasOBONamespace>ENVO</oboInOwl:hasOBONamespace>
        <oboInOwl:id>ENVO:01000051</oboInOwl:id>
        <rdfs:label>marine black smoker biome</rdfs:label>
    </owl:Class>
    <owl:Axiom>
        <owl:annotatedSource rdf:resource="http://purl.obolibrary.org/obo/ENVO_01000051"/>
        <owl:annotatedProperty rdf:resource="http://purl.obolibrary.org/obo/IAO_0000115"/>
        <owl:annotatedTarget>A marine black smoker biome comprises regions of the marine hydrothermal vent biome characterised by a black vent plume. This black plume is a consequence of dissolved metals and minerals forming complexes with sulphide and indicates polymetallic sulphide mineral deposits beneath the surface.</owl:annotatedTarget>
        <oboInOwl:hasDbXref>ISBN:978-0-444-82619-0</oboInOwl:hasDbXref>
        <oboInOwl:hasDbXref>ORCID:0000-0002-4366-3088</oboInOwl:hasDbXref>
    </owl:Axiom>
    


    <!-- http://purl.obolibrary.org/obo/ENVO_01000052 -->

    <owl:Class rdf:about="http://purl.obolibrary.org/obo/ENVO_01000052">
        <rdfs:subClassOf rdf:resource="http://purl.obolibrary.org/obo/ENVO_01000030"/>
        <obo:IAO_0000115>A marine white smoker biome comprises regions of the marine hydrothermal vent biome characterised by lightly hued plumes, typically containing barium, calcium, and silicon. These vents tend to have lower temperature plumes when compared to black smoker environments.</obo:IAO_0000115>
        <oboInOwl:created_by>ORCID:0000-0002-4366-3088</oboInOwl:created_by>
        <oboInOwl:creation_date>2010-03-15T11:29:37Z</oboInOwl:creation_date>
        <oboInOwl:hasOBONamespace>ENVO</oboInOwl:hasOBONamespace>
        <oboInOwl:id>ENVO:01000052</oboInOwl:id>
        <rdfs:label>marine white smoker biome</rdfs:label>
    </owl:Class>
    <owl:Axiom>
        <owl:annotatedSource rdf:resource="http://purl.obolibrary.org/obo/ENVO_01000052"/>
        <owl:annotatedProperty rdf:resource="http://purl.obolibrary.org/obo/IAO_0000115"/>
        <owl:annotatedTarget>A marine white smoker biome comprises regions of the marine hydrothermal vent biome characterised by lightly hued plumes, typically containing barium, calcium, and silicon. These vents tend to have lower temperature plumes when compared to black smoker environments.</owl:annotatedTarget>
        <oboInOwl:hasDbXref>ORCID:0000-0002-4366-3088</oboInOwl:hasDbXref>
        <oboInOwl:hasDbXref>https://en.wikipedia.org/wiki/Hydrothermal_vent</oboInOwl:hasDbXref>
    </owl:Axiom>
    


    <!-- http://purl.obolibrary.org/obo/ENVO_01000053 -->

    <owl:Class rdf:about="http://purl.obolibrary.org/obo/ENVO_01000053">
        <rdfs:subClassOf rdf:resource="http://purl.obolibrary.org/obo/ENVO_01000030"/>
        <obo:IAO_0000115>A marine ultramafic hydrothermal vent biome comprises regions of themarine  hydrothermal vent biome hosted on ultramafic (also referred to as ultrabasic) rocks. Ultramafic rocks are igneous and meta-igneous rocks with very low silica content (less than 45%), generally &gt;18% MgO, high FeO, low potassium, and are composed of usually greater than 90% mafic minerals  (dark colored, high magnesium and iron content). The Earth&apos;s mantle is composed of ultramafic rocks.</obo:IAO_0000115>
        <oboInOwl:created_by>ORCID:0000-0002-4366-3088</oboInOwl:created_by>
        <oboInOwl:creation_date>2010-03-15T11:29:37Z</oboInOwl:creation_date>
        <oboInOwl:hasOBONamespace>ENVO</oboInOwl:hasOBONamespace>
        <oboInOwl:id>ENVO:01000053</oboInOwl:id>
        <rdfs:label>marine ultramafic hydrothermal vent biome</rdfs:label>
    </owl:Class>
    <owl:Axiom>
        <owl:annotatedSource rdf:resource="http://purl.obolibrary.org/obo/ENVO_01000053"/>
        <owl:annotatedProperty rdf:resource="http://purl.obolibrary.org/obo/IAO_0000115"/>
        <owl:annotatedTarget>A marine ultramafic hydrothermal vent biome comprises regions of themarine  hydrothermal vent biome hosted on ultramafic (also referred to as ultrabasic) rocks. Ultramafic rocks are igneous and meta-igneous rocks with very low silica content (less than 45%), generally &gt;18% MgO, high FeO, low potassium, and are composed of usually greater than 90% mafic minerals  (dark colored, high magnesium and iron content). The Earth&apos;s mantle is composed of ultramafic rocks.</owl:annotatedTarget>
        <oboInOwl:hasDbXref>ISBN:978-0-444-82619-0</oboInOwl:hasDbXref>
        <oboInOwl:hasDbXref>ORCID:0000-0002-4366-3088</oboInOwl:hasDbXref>
        <oboInOwl:hasDbXref>https://en.wikipedia.org/wiki/Ultramafic</oboInOwl:hasDbXref>
    </owl:Axiom>
    


    <!-- http://purl.obolibrary.org/obo/ENVO_01000054 -->

    <owl:Class rdf:about="http://purl.obolibrary.org/obo/ENVO_01000054">
        <rdfs:subClassOf rdf:resource="http://purl.obolibrary.org/obo/ENVO_01000030"/>
        <obo:IAO_0000115>A marine basaltic hydrothermal vent biome comprises regions of the marine hydrothermal vent biome hosted on basaltic rocks. Basalt generally has a composition of 45 to 55 wt % SiO2, 2 to 6 wt % total alkalis, 0.5 to 2.0 wt % TiO2, 5 to 14 wt % FeO and 14 wt % or more Al2O3. Contents of CaO are commonly near 10 wt %, those of MgO commonly in the range 5 to 12 wt %.</obo:IAO_0000115>
        <oboInOwl:created_by>ORCID:0000-0002-4366-3088</oboInOwl:created_by>
        <oboInOwl:creation_date>2010-03-15T11:29:37Z</oboInOwl:creation_date>
        <oboInOwl:hasOBONamespace>ENVO</oboInOwl:hasOBONamespace>
        <oboInOwl:id>ENVO:01000054</oboInOwl:id>
        <rdfs:label>marine basaltic hydrothermal vent biome</rdfs:label>
    </owl:Class>
    <owl:Axiom>
        <owl:annotatedSource rdf:resource="http://purl.obolibrary.org/obo/ENVO_01000054"/>
        <owl:annotatedProperty rdf:resource="http://purl.obolibrary.org/obo/IAO_0000115"/>
        <owl:annotatedTarget>A marine basaltic hydrothermal vent biome comprises regions of the marine hydrothermal vent biome hosted on basaltic rocks. Basalt generally has a composition of 45 to 55 wt % SiO2, 2 to 6 wt % total alkalis, 0.5 to 2.0 wt % TiO2, 5 to 14 wt % FeO and 14 wt % or more Al2O3. Contents of CaO are commonly near 10 wt %, those of MgO commonly in the range 5 to 12 wt %.</owl:annotatedTarget>
        <oboInOwl:hasDbXref>ISBN:978-0-444-82619-0</oboInOwl:hasDbXref>
        <oboInOwl:hasDbXref>ORCID:0000-0002-4366-3088</oboInOwl:hasDbXref>
        <oboInOwl:hasDbXref>https://en.wikipedia.org/wiki/Basalt</oboInOwl:hasDbXref>
    </owl:Axiom>
    


    <!-- http://purl.obolibrary.org/obo/ENVO_01000123 -->

    <owl:Class rdf:about="http://purl.obolibrary.org/obo/ENVO_01000123">
        <rdfs:subClassOf rdf:resource="http://purl.obolibrary.org/obo/ENVO_01000029"/>
        <obo:IAO_0000115>The marine sponge reef biome comprises marine reefs primarily built by marine sponges. The primary frame-building sponges are all members of the order Hexactinosa. They are found only in glacier-scoured troughs of low-angle continental shelf. The seafloor is stable and consists of rock, coarse gravel, and large boulders.</obo:IAO_0000115>
        <oboInOwl:created_by>ORCID:0000-0002-4366-3088</oboInOwl:created_by>
        <oboInOwl:creation_date>2010-03-17T04:43:05Z</oboInOwl:creation_date>
        <oboInOwl:hasOBONamespace>ENVO</oboInOwl:hasOBONamespace>
        <oboInOwl:id>ENVO:01000123</oboInOwl:id>
        <rdfs:label>marine sponge reef biome</rdfs:label>
    </owl:Class>
    <owl:Axiom>
        <owl:annotatedSource rdf:resource="http://purl.obolibrary.org/obo/ENVO_01000123"/>
        <owl:annotatedProperty rdf:resource="http://purl.obolibrary.org/obo/IAO_0000115"/>
        <owl:annotatedTarget>The marine sponge reef biome comprises marine reefs primarily built by marine sponges. The primary frame-building sponges are all members of the order Hexactinosa. They are found only in glacier-scoured troughs of low-angle continental shelf. The seafloor is stable and consists of rock, coarse gravel, and large boulders.</owl:annotatedTarget>
        <oboInOwl:hasDbXref>ORCID:0000-0002-4366-3088</oboInOwl:hasDbXref>
        <oboInOwl:hasDbXref>https://en.wikipedia.org/wiki/Sponge_reef</oboInOwl:hasDbXref>
    </owl:Axiom>
    


    <!-- http://purl.obolibrary.org/obo/ENVO_01000127 -->

    <owl:Class rdf:about="http://purl.obolibrary.org/obo/ENVO_01000127">
        <rdfs:subClassOf rdf:resource="http://purl.obolibrary.org/obo/ENVO_01000024"/>
        <obo:IAO_0000115>A marine benthic biome which is determined by a cold seep.</obo:IAO_0000115>
        <oboInOwl:created_by rdf:resource="https://orcid.org/0000-0002-4366-3088"/>
        <oboInOwl:creation_date>2010-03-19T08:33:56Z</oboInOwl:creation_date>
        <rdfs:comment>The marine cold seep biome comprises regions of the marine benthic biome where seepage of methane, hydrogen sulphide, hydrocarbon rich fluids and other fluids occurs.</rdfs:comment>
        <rdfs:label>marine cold seep biome</rdfs:label>
    </owl:Class>
    <owl:Axiom>
        <owl:annotatedSource rdf:resource="http://purl.obolibrary.org/obo/ENVO_01000127"/>
        <owl:annotatedProperty rdf:resource="http://purl.obolibrary.org/obo/IAO_0000115"/>
        <owl:annotatedTarget>A marine benthic biome which is determined by a cold seep.</owl:annotatedTarget>
        <oboInOwl:hasDbXref rdf:resource="https://orcid.org/0000-0002-4366-3088"/>
        <oboInOwl:hasDbXref>https://en.wikipedia.org/wiki/Cold_seep</oboInOwl:hasDbXref>
    </owl:Axiom>
    


    <!-- http://purl.obolibrary.org/obo/ENVO_01000128 -->

    <owl:Class rdf:about="http://purl.obolibrary.org/obo/ENVO_01000128">
        <rdfs:subClassOf rdf:resource="http://purl.obolibrary.org/obo/ENVO_01000047"/>
        <obo:IAO_0000115>The dilution basin mediterranean sea biome comprises expressions of the mediterranean sea biome with lower salinity than the surrounding ocean due to freshwater gains such as rainfall and rivers. Water exchange consists of outflow of the fresher mediterranean water in the upper layer and inflow of the saltier oceanic water in the lower layer of the channel. Renewal of deep water may not be sufficient to supply oxygen to the bottom.</obo:IAO_0000115>
        <oboInOwl:created_by>ORCID:0000-0002-4366-3088</oboInOwl:created_by>
        <oboInOwl:creation_date>2010-03-19T09:32:59Z</oboInOwl:creation_date>
        <rdfs:label>dilution basin mediterranean sea biome</rdfs:label>
    </owl:Class>
    <owl:Axiom>
        <owl:annotatedSource rdf:resource="http://purl.obolibrary.org/obo/ENVO_01000128"/>
        <owl:annotatedProperty rdf:resource="http://purl.obolibrary.org/obo/IAO_0000115"/>
        <owl:annotatedTarget>The dilution basin mediterranean sea biome comprises expressions of the mediterranean sea biome with lower salinity than the surrounding ocean due to freshwater gains such as rainfall and rivers. Water exchange consists of outflow of the fresher mediterranean water in the upper layer and inflow of the saltier oceanic water in the lower layer of the channel. Renewal of deep water may not be sufficient to supply oxygen to the bottom.</owl:annotatedTarget>
        <oboInOwl:hasDbXref>ORCID:0000-0002-4366-3088</oboInOwl:hasDbXref>
        <oboInOwl:hasDbXref>https://en.wikipedia.org/wiki/Mediterranean_sea</oboInOwl:hasDbXref>
    </owl:Axiom>
    


    <!-- http://purl.obolibrary.org/obo/ENVO_01000174 -->

    <owl:Class rdf:about="http://purl.obolibrary.org/obo/ENVO_01000174">
        <rdfs:subClassOf rdf:resource="http://purl.obolibrary.org/obo/ENVO_00000446"/>
        <obo:IAO_0000115 xml:lang="en">A forest ecosystem which is undergoing climactic ecological succession.</obo:IAO_0000115>
        <oboInOwl:created_by>ORCID:0000-0002-4366-3088</oboInOwl:created_by>
        <oboInOwl:creation_date>2013-04-07T14:26:46Z</oboInOwl:creation_date>
        <oboInOwl:hasDbXref>LTER:212</oboInOwl:hasDbXref>
        <oboInOwl:hasDbXref>SPIRE:Forest</oboInOwl:hasDbXref>
        <rdfs:label>forest biome</rdfs:label>
    </owl:Class>
    


    <!-- http://purl.obolibrary.org/obo/ENVO_01000175 -->

    <owl:Class rdf:about="http://purl.obolibrary.org/obo/ENVO_01000175">
        <rdfs:subClassOf rdf:resource="http://purl.obolibrary.org/obo/ENVO_00000446"/>
        <obo:IAO_0000115>A woodland biome is a terrestrial biome which includes, across its entire spatial extent, woody plants spaced sufficiently far apart to allow light penetration to support communities of herbaceous plants or shrubs living closer to the woodland floor.</obo:IAO_0000115>
        <oboInOwl:created_by>ORCID:0000-0002-4366-3088</oboInOwl:created_by>
        <oboInOwl:creation_date>2013-04-07T14:26:46Z</oboInOwl:creation_date>
        <rdfs:comment>Preliminary definition.</rdfs:comment>
        <rdfs:label>woodland biome</rdfs:label>
    </owl:Class>
    


    <!-- http://purl.obolibrary.org/obo/ENVO_01000176 -->

    <owl:Class rdf:about="http://purl.obolibrary.org/obo/ENVO_01000176">
        <rdfs:subClassOf rdf:resource="http://purl.obolibrary.org/obo/ENVO_00000446"/>
        <obo:IAO_0000115>A shrubland biome is a terrestrial biome which includes, across its entire spatial extent, dense groups of shrubs.</obo:IAO_0000115>
        <oboInOwl:created_by>ORCID:0000-0002-4366-3088</oboInOwl:created_by>
        <oboInOwl:creation_date>2013-04-07T14:26:46Z</oboInOwl:creation_date>
        <rdfs:comment>Preliminary definition.</rdfs:comment>
        <rdfs:label>shrubland biome</rdfs:label>
    </owl:Class>
    


    <!-- http://purl.obolibrary.org/obo/ENVO_01000177 -->

    <owl:Class rdf:about="http://purl.obolibrary.org/obo/ENVO_01000177">
        <rdfs:subClassOf rdf:resource="http://purl.obolibrary.org/obo/ENVO_00000446"/>
        <obo:IAO_0000115>A grassland ecosystem in which dominant ecological communities have reached their climax successional state.</obo:IAO_0000115>
        <oboInOwl:created_by>ORCID:0000-0002-4366-3088</oboInOwl:created_by>
        <oboInOwl:creation_date>2013-04-07T14:26:46Z</oboInOwl:creation_date>
        <oboInOwl:hasDbXref>SPIRE:Savannah_or_grassland</oboInOwl:hasDbXref>
        <rdfs:label>grassland biome</rdfs:label>
    </owl:Class>
    


    <!-- http://purl.obolibrary.org/obo/ENVO_01000178 -->

    <owl:Class rdf:about="http://purl.obolibrary.org/obo/ENVO_01000178">
        <rdfs:subClassOf rdf:resource="http://purl.obolibrary.org/obo/ENVO_01000175"/>
        <obo:IAO_0000115 xml:lang="en">A woodland biome which has seasonal water availability and includes trees spaced sufficiently far apart to allow an unbroken layer of grass, sedge (Cyperaceae) or  rush (Juncaceae) communities to live.</obo:IAO_0000115>
        <oboInOwl:created_by>ORCID:0000-0002-4366-3088</oboInOwl:created_by>
        <oboInOwl:creation_date>2013-04-07T14:26:46Z</oboInOwl:creation_date>
        <oboInOwl:hasDbXref>SPIRE:Savannah_or_grassland</oboInOwl:hasDbXref>
        <rdfs:label>savanna biome</rdfs:label>
    </owl:Class>
    


    <!-- http://purl.obolibrary.org/obo/ENVO_01000179 -->

    <owl:Class rdf:about="http://purl.obolibrary.org/obo/ENVO_01000179">
        <rdfs:subClassOf rdf:resource="http://purl.obolibrary.org/obo/ENVO_00000428"/>
        <obo:IAO_0000115 xml:lang="en">A desert ecosystem which is undergoing climactic ecological succession.</obo:IAO_0000115>
        <oboInOwl:created_by>ORCID:0000-0002-4366-3088</oboInOwl:created_by>
        <oboInOwl:creation_date>2013-04-07T14:26:46Z</oboInOwl:creation_date>
        <oboInOwl:hasDbXref>SPIRE:Desert_or_dune</oboInOwl:hasDbXref>
        <oboInOwl:inSubset>wwfBiome</oboInOwl:inSubset>
        <rdfs:label>desert biome</rdfs:label>
    </owl:Class>
    


    <!-- http://purl.obolibrary.org/obo/ENVO_01000180 -->

    <owl:Class rdf:about="http://purl.obolibrary.org/obo/ENVO_01000180">
        <rdfs:subClassOf rdf:resource="http://purl.obolibrary.org/obo/ENVO_00000446"/>
        <obo:IAO_0000115 xml:lang="en">A tundra ecosystem which is undergoing climactic ecological succession.</obo:IAO_0000115>
        <oboInOwl:created_by>ORCID:0000-0002-4366-3088</oboInOwl:created_by>
        <oboInOwl:creation_date>2013-04-07T14:26:46Z</oboInOwl:creation_date>
        <oboInOwl:hasDbXref>SPIRE:Tundra</oboInOwl:hasDbXref>
        <oboInOwl:inSubset>envoPolar</oboInOwl:inSubset>
        <oboInOwl:inSubset>wwfBiome</oboInOwl:inSubset>
        <rdfs:label>tundra biome</rdfs:label>
    </owl:Class>
    


    <!-- http://purl.obolibrary.org/obo/ENVO_01000181 -->

    <owl:Class rdf:about="http://purl.obolibrary.org/obo/ENVO_01000181">
        <rdfs:subClassOf rdf:resource="http://purl.obolibrary.org/obo/ENVO_00000446"/>
        <obo:IAO_0000115>A mangrove biome is a terrestrial biome which includes, across its spatial extent, mangrove plants (Rhizophoraceae). Mangrove plants are able to withstand high levels of salinity as well as regions of anoxia and frequent tidal inundation. Mangrove biomes often occur near tropical and sub-tropical estuaries and depositional marine coastal environments where fine sediments (often with high organic content) collect in areas protected from high energy wave action.</obo:IAO_0000115>
        <oboInOwl:created_by>ORCID:0000-0002-4366-3088</oboInOwl:created_by>
        <oboInOwl:creation_date>2013-04-07T14:26:46Z</oboInOwl:creation_date>
        <oboInOwl:hasDbXref>LTER:322</oboInOwl:hasDbXref>
        <oboInOwl:inSubset>wwfBiome</oboInOwl:inSubset>
        <rdfs:comment>Preliminary definition. Depending on whether mangrove trees or shrubs are present, this class could be a child of shrubland biome or woodland biome. Consider creating the appropriate classes.</rdfs:comment>
        <rdfs:label>mangrove biome</rdfs:label>
    </owl:Class>
    <owl:Axiom>
        <owl:annotatedSource rdf:resource="http://purl.obolibrary.org/obo/ENVO_01000181"/>
        <owl:annotatedProperty rdf:resource="http://purl.obolibrary.org/obo/IAO_0000115"/>
        <owl:annotatedTarget>A mangrove biome is a terrestrial biome which includes, across its spatial extent, mangrove plants (Rhizophoraceae). Mangrove plants are able to withstand high levels of salinity as well as regions of anoxia and frequent tidal inundation. Mangrove biomes often occur near tropical and sub-tropical estuaries and depositional marine coastal environments where fine sediments (often with high organic content) collect in areas protected from high energy wave action.</owl:annotatedTarget>
        <oboInOwl:hasDbXref>ORCID:0000-0002-4366-3088</oboInOwl:hasDbXref>
        <oboInOwl:hasDbXref>https://en.wikipedia.org/wiki/Mangrove</oboInOwl:hasDbXref>
    </owl:Axiom>
    


    <!-- http://purl.obolibrary.org/obo/ENVO_01000182 -->

    <owl:Class rdf:about="http://purl.obolibrary.org/obo/ENVO_01000182">
        <rdfs:subClassOf rdf:resource="http://purl.obolibrary.org/obo/ENVO_01000179"/>
        <rdfs:subClassOf rdf:resource="http://purl.obolibrary.org/obo/ENVO_01001831"/>
        <obo:IAO_0000115>A temperate desert biome is a desert biome which has communities adapted to intermediate insolation, low rainfall, and large temperature variations between winter and summer. Winter temperatures may fall below 0 degrees Celsius. Some precipitation in this biome may fall as snow.</obo:IAO_0000115>
        <oboInOwl:created_by>ORCID:0000-0002-4366-3088</oboInOwl:created_by>
        <oboInOwl:creation_date>2013-04-07T14:28:08Z</oboInOwl:creation_date>
        <rdfs:comment>Preliminary definition. The semantics and definitions of &quot;mediterranean&quot;, &quot;subtropical&quot;, &quot;tropical&quot;, &quot;temperate&quot;, &quot;polar&quot;, and similar climate types may be transferred to an &quot;environmental condition&quot; class once the semantics of this class have been established.</rdfs:comment>
        <rdfs:label>temperate desert biome</rdfs:label>
    </owl:Class>
    <owl:Axiom>
        <owl:annotatedSource rdf:resource="http://purl.obolibrary.org/obo/ENVO_01000182"/>
        <owl:annotatedProperty rdf:resource="http://purl.obolibrary.org/obo/IAO_0000115"/>
        <owl:annotatedTarget>A temperate desert biome is a desert biome which has communities adapted to intermediate insolation, low rainfall, and large temperature variations between winter and summer. Winter temperatures may fall below 0 degrees Celsius. Some precipitation in this biome may fall as snow.</owl:annotatedTarget>
        <oboInOwl:hasDbXref>WWW:http://www.fs.fed.us/land/ecosysmgmt/colorimagemap/images/340.html</oboInOwl:hasDbXref>
    </owl:Axiom>
    


    <!-- http://purl.obolibrary.org/obo/ENVO_01000183 -->

    <owl:Class rdf:about="http://purl.obolibrary.org/obo/ENVO_01000183">
        <rdfs:subClassOf rdf:resource="http://purl.obolibrary.org/obo/ENVO_01000179"/>
        <rdfs:subClassOf rdf:resource="http://purl.obolibrary.org/obo/ENVO_01001830"/>
        <obo:IAO_0000115>A tropical desert biome is a desert biome which has communities adapted to temperatures above a monthly average of 18 degrees Celsius, high daily temperature ranges of approximately 20 degrees Celsius, very high insolation due to inhibited cloud formation, and very low precipitation. Tropical desert biomes located near coasts with cold upwellings may have cooler temperatures and reduced insolution due to fog.</obo:IAO_0000115>
        <oboInOwl:created_by>ORCID:0000-0002-4366-3088</oboInOwl:created_by>
        <oboInOwl:creation_date>2013-04-07T14:28:08Z</oboInOwl:creation_date>
        <rdfs:comment>Preliminary definition. The semantics and definitions of &quot;mediterranean&quot;, &quot;subtropical&quot;, &quot;tropical&quot;, &quot;temperate&quot;, &quot;polar&quot;, and similar climate types may be transferred to an &quot;environmental condition&quot; class once the semantics of this class have been established.</rdfs:comment>
        <rdfs:label>tropical desert biome</rdfs:label>
    </owl:Class>
    <owl:Axiom>
        <owl:annotatedSource rdf:resource="http://purl.obolibrary.org/obo/ENVO_01000183"/>
        <owl:annotatedProperty rdf:resource="http://purl.obolibrary.org/obo/IAO_0000115"/>
        <owl:annotatedTarget>A tropical desert biome is a desert biome which has communities adapted to temperatures above a monthly average of 18 degrees Celsius, high daily temperature ranges of approximately 20 degrees Celsius, very high insolation due to inhibited cloud formation, and very low precipitation. Tropical desert biomes located near coasts with cold upwellings may have cooler temperatures and reduced insolution due to fog.</owl:annotatedTarget>
        <oboInOwl:hasDbXref>WWW:http://www.earthonlinemedia.com/ebooks/tpe_3e/title_page.html</oboInOwl:hasDbXref>
    </owl:Axiom>
    


    <!-- http://purl.obolibrary.org/obo/ENVO_01000184 -->

    <owl:Class rdf:about="http://purl.obolibrary.org/obo/ENVO_01000184">
        <rdfs:subClassOf rdf:resource="http://purl.obolibrary.org/obo/ENVO_01000179"/>
        <rdfs:subClassOf rdf:resource="http://purl.obolibrary.org/obo/ENVO_01001832"/>
        <obo:IAO_0000115>A subtropical desert biome is a desert biome which has communities adapted to temperatures above a monthly average of 18 degrees Celsius, high daily temperature ranges of approximately 20 degrees Celsius, high insolation (but lower than that of a tropical desert biome), inhibited cloud formation, and very low precipitation. Subtropical desert biomes located near coasts with cold upwellings may have cooler temperatures and reduced insolution due to fog.</obo:IAO_0000115>
        <oboInOwl:created_by>ORCID:0000-0002-4366-3088</oboInOwl:created_by>
        <oboInOwl:creation_date>2013-04-07T14:28:08Z</oboInOwl:creation_date>
        <rdfs:comment>Preliminary definition. The semantics and definitions of &quot;mediterranean&quot;, &quot;subtropical&quot;, &quot;tropical&quot;, &quot;temperate&quot;, &quot;polar&quot;, and similar climate types may be transferred to an &quot;environmental condition&quot; class once the semantics of this class have been established.</rdfs:comment>
        <rdfs:label>subtropical desert biome</rdfs:label>
    </owl:Class>
    <owl:Axiom>
        <owl:annotatedSource rdf:resource="http://purl.obolibrary.org/obo/ENVO_01000184"/>
        <owl:annotatedProperty rdf:resource="http://purl.obolibrary.org/obo/IAO_0000115"/>
        <owl:annotatedTarget>A subtropical desert biome is a desert biome which has communities adapted to temperatures above a monthly average of 18 degrees Celsius, high daily temperature ranges of approximately 20 degrees Celsius, high insolation (but lower than that of a tropical desert biome), inhibited cloud formation, and very low precipitation. Subtropical desert biomes located near coasts with cold upwellings may have cooler temperatures and reduced insolution due to fog.</owl:annotatedTarget>
        <oboInOwl:hasDbXref>WWW:http://www.earthonlinemedia.com/ebooks/tpe_3e/title_page.html</oboInOwl:hasDbXref>
        <oboInOwl:hasDbXref>https://en.wikipedia.org/wiki/Subtropical#Semi-desert.2Fdesert_climate</oboInOwl:hasDbXref>
    </owl:Axiom>
    


    <!-- http://purl.obolibrary.org/obo/ENVO_01000185 -->

    <owl:Class rdf:about="http://purl.obolibrary.org/obo/ENVO_01000185">
        <rdfs:subClassOf rdf:resource="http://purl.obolibrary.org/obo/ENVO_01000179"/>
        <rdfs:subClassOf rdf:resource="http://purl.obolibrary.org/obo/ENVO_01001836"/>
        <obo:IAO_0000115>A montane desert biome is a desert biome which occurs in regions elevated above sea level and which has community structure determined by elevation-dependent environmental conditions.</obo:IAO_0000115>
        <oboInOwl:created_by>ORCID:0000-0002-4366-3088</oboInOwl:created_by>
        <oboInOwl:creation_date>2013-04-07T14:28:08Z</oboInOwl:creation_date>
        <rdfs:comment>Preliminary definition.</rdfs:comment>
        <rdfs:label>montane desert biome</rdfs:label>
    </owl:Class>
    


    <!-- http://purl.obolibrary.org/obo/ENVO_01000186 -->

    <owl:Class rdf:about="http://purl.obolibrary.org/obo/ENVO_01000186">
        <rdfs:subClassOf rdf:resource="http://purl.obolibrary.org/obo/ENVO_01000179"/>
        <rdfs:subClassOf rdf:resource="http://purl.obolibrary.org/obo/ENVO_01000339"/>
        <obo:IAO_0000115>A polar desert biome is a desert biome which is subject to low levels of insolation, annual precipitation less than 250 millimeters, and a mean temperature less than 10 degrees Celsius during its warmest month. Temperature changes in polar deserts frequently cross the freezing point of water.</obo:IAO_0000115>
        <oboInOwl:created_by>ORCID:0000-0002-4366-3088</oboInOwl:created_by>
        <oboInOwl:creation_date>2013-04-07T14:28:08Z</oboInOwl:creation_date>
        <oboInOwl:inSubset>envoPolar</oboInOwl:inSubset>
        <rdfs:comment>Preliminary definition. The semantics and definitions of &quot;mediterranean&quot;, &quot;subtropical&quot;, &quot;tropical&quot;, &quot;temperate&quot;, &quot;polar&quot;, and similar climate types may be transferred to an &quot;environmental condition&quot; class once the semantics of this class have been established.</rdfs:comment>
        <rdfs:label>polar desert biome</rdfs:label>
    </owl:Class>
    <owl:Axiom>
        <owl:annotatedSource rdf:resource="http://purl.obolibrary.org/obo/ENVO_01000186"/>
        <owl:annotatedProperty rdf:resource="http://purl.obolibrary.org/obo/IAO_0000115"/>
        <owl:annotatedTarget>A polar desert biome is a desert biome which is subject to low levels of insolation, annual precipitation less than 250 millimeters, and a mean temperature less than 10 degrees Celsius during its warmest month. Temperature changes in polar deserts frequently cross the freezing point of water.</owl:annotatedTarget>
        <oboInOwl:hasDbXref>https://en.wikipedia.org/wiki/Polar_desert</oboInOwl:hasDbXref>
    </owl:Axiom>
    


    <!-- http://purl.obolibrary.org/obo/ENVO_01000187 -->

    <owl:Class rdf:about="http://purl.obolibrary.org/obo/ENVO_01000187">
        <rdfs:subClassOf rdf:resource="http://purl.obolibrary.org/obo/ENVO_01000178"/>
        <rdfs:subClassOf rdf:resource="http://purl.obolibrary.org/obo/ENVO_01001832"/>
        <obo:IAO_0000115 xml:lang="en">A savanna biome which is subject to subtropical climate patterns.</obo:IAO_0000115>
        <oboInOwl:created_by>ORCID:0000-0002-4366-3088</oboInOwl:created_by>
        <oboInOwl:creation_date>2013-04-07T14:28:51Z</oboInOwl:creation_date>
        <oboInOwl:inSubset>wwfBiome</oboInOwl:inSubset>
        <rdfs:comment>Preliminary definition. The semantics and definitions of &quot;mediterranean&quot;, &quot;subtropical&quot;, &quot;tropical&quot;, &quot;temperate&quot;, &quot;polar&quot;, and similar climate types may be transferred to an &quot;environmental condition&quot; class once the semantics of this class have been established.</rdfs:comment>
        <rdfs:label>subtropical savanna biome</rdfs:label>
    </owl:Class>
    


    <!-- http://purl.obolibrary.org/obo/ENVO_01000188 -->

    <owl:Class rdf:about="http://purl.obolibrary.org/obo/ENVO_01000188">
        <rdfs:subClassOf rdf:resource="http://purl.obolibrary.org/obo/ENVO_01000178"/>
        <rdfs:subClassOf rdf:resource="http://purl.obolibrary.org/obo/ENVO_01001830"/>
        <obo:IAO_0000115 xml:lang="en">A savanna biome which is subject to tropical climate patterns.</obo:IAO_0000115>
        <oboInOwl:created_by>ORCID:0000-0002-4366-3088</oboInOwl:created_by>
        <oboInOwl:creation_date>2013-04-07T14:28:51Z</oboInOwl:creation_date>
        <oboInOwl:inSubset>wwfBiome</oboInOwl:inSubset>
        <rdfs:comment>Preliminary definition. The semantics and definitions of &quot;mediterranean&quot;, &quot;subtropical&quot;, &quot;tropical&quot;, &quot;temperate&quot;, &quot;polar&quot;, and similar climate types may be transferred to an &quot;environmental condition&quot; class once the semantics of this class have been established.</rdfs:comment>
        <rdfs:label>tropical savanna biome</rdfs:label>
    </owl:Class>
    


    <!-- http://purl.obolibrary.org/obo/ENVO_01000189 -->

    <owl:Class rdf:about="http://purl.obolibrary.org/obo/ENVO_01000189">
        <rdfs:subClassOf rdf:resource="http://purl.obolibrary.org/obo/ENVO_01000178"/>
        <rdfs:subClassOf rdf:resource="http://purl.obolibrary.org/obo/ENVO_01001831"/>
        <obo:IAO_0000115 xml:lang="en">A savanna biome which is subject to temperate climate patterns.</obo:IAO_0000115>
        <oboInOwl:created_by>ORCID:0000-0002-4366-3088</oboInOwl:created_by>
        <oboInOwl:creation_date>2013-04-07T14:28:51Z</oboInOwl:creation_date>
        <oboInOwl:hasBroadSynonym>prairie biome</oboInOwl:hasBroadSynonym>
        <rdfs:comment>Preliminary definition. The semantics and definitions of &quot;mediterranean&quot;, &quot;subtropical&quot;, &quot;tropical&quot;, &quot;temperate&quot;, &quot;polar&quot;, and similar climate types may be transferred to an &quot;environmental condition&quot; class once the semantics of this class have been established.</rdfs:comment>
        <rdfs:label>temperate savanna biome</rdfs:label>
    </owl:Class>
    


    <!-- http://purl.obolibrary.org/obo/ENVO_01000190 -->

    <owl:Class rdf:about="http://purl.obolibrary.org/obo/ENVO_01000190">
        <rdfs:subClassOf rdf:resource="http://purl.obolibrary.org/obo/ENVO_01000178"/>
        <obo:IAO_0000115>A flooded savanna biome is a savanna biome which has very wet to saturated soil moisture content.</obo:IAO_0000115>
        <oboInOwl:created_by>ORCID:0000-0002-4366-3088</oboInOwl:created_by>
        <oboInOwl:creation_date>2013-04-07T14:28:51Z</oboInOwl:creation_date>
        <oboInOwl:hasBroadSynonym>swamp</oboInOwl:hasBroadSynonym>
        <oboInOwl:hasRelatedSynonym>marsh</oboInOwl:hasRelatedSynonym>
        <oboInOwl:inSubset>wwfBiome</oboInOwl:inSubset>
        <rdfs:label>flooded savanna biome</rdfs:label>
    </owl:Class>
    <owl:Axiom>
        <owl:annotatedSource rdf:resource="http://purl.obolibrary.org/obo/ENVO_01000190"/>
        <owl:annotatedProperty rdf:resource="http://purl.obolibrary.org/obo/IAO_0000115"/>
        <owl:annotatedTarget>A flooded savanna biome is a savanna biome which has very wet to saturated soil moisture content.</owl:annotatedTarget>
        <oboInOwl:hasDbXref>https://en.wikipedia.org/wiki/Flooded_grasslands_and_savannas</oboInOwl:hasDbXref>
    </owl:Axiom>
    


    <!-- http://purl.obolibrary.org/obo/ENVO_01000191 -->

    <owl:Class rdf:about="http://purl.obolibrary.org/obo/ENVO_01000191">
        <rdfs:subClassOf rdf:resource="http://purl.obolibrary.org/obo/ENVO_01000177"/>
        <rdfs:subClassOf rdf:resource="http://purl.obolibrary.org/obo/ENVO_01001832"/>
        <obo:IAO_0000115>A subtropical grassland in which dominant ecological communities have reached their climax successional state.</obo:IAO_0000115>
        <oboInOwl:creation_date>2013-04-07T14:29:48Z</oboInOwl:creation_date>
        <oboInOwl:inSubset>wwfBiome</oboInOwl:inSubset>
        <rdfs:label>subtropical grassland biome</rdfs:label>
    </owl:Class>
    


    <!-- http://purl.obolibrary.org/obo/ENVO_01000192 -->

    <owl:Class rdf:about="http://purl.obolibrary.org/obo/ENVO_01000192">
        <rdfs:subClassOf rdf:resource="http://purl.obolibrary.org/obo/ENVO_01000177"/>
        <rdfs:subClassOf rdf:resource="http://purl.obolibrary.org/obo/ENVO_01001830"/>
        <oboInOwl:created_by>ORCID:0000-0002-4366-3088</oboInOwl:created_by>
        <oboInOwl:creation_date>2013-04-07T14:29:48Z</oboInOwl:creation_date>
        <oboInOwl:inSubset>wwfBiome</oboInOwl:inSubset>
        <rdfs:comment>Preliminary definition. The semantics and definitions of &quot;mediterranean&quot;, &quot;subtropical&quot;, &quot;tropical&quot;, &quot;temperate&quot;, &quot;polar&quot;, and similar climate types may be transferred to an &quot;environmental condition&quot; class once the semantics of this class have been established.</rdfs:comment>
        <rdfs:label>tropical grassland biome</rdfs:label>
    </owl:Class>
    


    <!-- http://purl.obolibrary.org/obo/ENVO_01000193 -->

    <owl:Class rdf:about="http://purl.obolibrary.org/obo/ENVO_01000193">
        <rdfs:subClassOf rdf:resource="http://purl.obolibrary.org/obo/ENVO_01000177"/>
        <rdfs:subClassOf rdf:resource="http://purl.obolibrary.org/obo/ENVO_01001831"/>
        <oboInOwl:created_by>ORCID:0000-0002-4366-3088</oboInOwl:created_by>
        <oboInOwl:creation_date>2013-04-07T14:29:48Z</oboInOwl:creation_date>
        <oboInOwl:hasBroadSynonym>prairie biome</oboInOwl:hasBroadSynonym>
        <rdfs:comment>Preliminary definition. The semantics and definitions of &quot;mediterranean&quot;, &quot;subtropical&quot;, &quot;tropical&quot;, &quot;temperate&quot;, &quot;polar&quot;, and similar climate types may be transferred to an &quot;environmental condition&quot; class once the semantics of this class have been established.</rdfs:comment>
        <rdfs:label>temperate grassland biome</rdfs:label>
    </owl:Class>
    


    <!-- http://purl.obolibrary.org/obo/ENVO_01000194 -->

    <owl:Class rdf:about="http://purl.obolibrary.org/obo/ENVO_01000194">
        <rdfs:subClassOf rdf:resource="http://purl.obolibrary.org/obo/ENVO_01000177"/>
        <rdfs:subClassOf rdf:resource="http://purl.obolibrary.org/obo/ENVO_01001836"/>
        <obo:IAO_0000115>A montane grassland biome is a grassland biome which occurs in regions elevated above sea level and which has community structure determined by elevation-dependent environmental conditions.</obo:IAO_0000115>
        <oboInOwl:created_by>ORCID:0000-0002-4366-3088</oboInOwl:created_by>
        <oboInOwl:creation_date>2013-04-07T14:29:48Z</oboInOwl:creation_date>
        <oboInOwl:inSubset>wwfBiome</oboInOwl:inSubset>
        <rdfs:comment>Preliminary definition.</rdfs:comment>
        <rdfs:label>montane grassland biome</rdfs:label>
    </owl:Class>
    


    <!-- http://purl.obolibrary.org/obo/ENVO_01000195 -->

    <owl:Class rdf:about="http://purl.obolibrary.org/obo/ENVO_01000195">
        <rdfs:subClassOf rdf:resource="http://purl.obolibrary.org/obo/ENVO_01000177"/>
        <oboInOwl:created_by>ORCID:0000-0002-4366-3088</oboInOwl:created_by>
        <oboInOwl:creation_date>2013-04-07T14:29:48Z</oboInOwl:creation_date>
        <oboInOwl:inSubset>wwfBiome</oboInOwl:inSubset>
        <rdfs:label>flooded grassland biome</rdfs:label>
    </owl:Class>
    


    <!-- http://purl.obolibrary.org/obo/ENVO_01000196 -->

    <owl:Class rdf:about="http://purl.obolibrary.org/obo/ENVO_01000196">
        <rdfs:subClassOf rdf:resource="http://purl.obolibrary.org/obo/ENVO_01000174"/>
        <obo:IAO_0000115>A coniferous forest biome is a forest biome which contains densely packed populations or communities of coniferous trees, strongly limiting light penetration to the forest floor.</obo:IAO_0000115>
        <oboInOwl:created_by>ORCID:0000-0002-4366-3088</oboInOwl:created_by>
        <oboInOwl:creation_date>2013-04-07T14:31:01Z</oboInOwl:creation_date>
        <oboInOwl:hasOBONamespace>ENVO</oboInOwl:hasOBONamespace>
        <oboInOwl:id>ENVO:01000196</oboInOwl:id>
        <rdfs:comment>Preliminary definition.</rdfs:comment>
        <rdfs:label>coniferous forest biome</rdfs:label>
    </owl:Class>
    


    <!-- http://purl.obolibrary.org/obo/ENVO_01000197 -->

    <owl:Class rdf:about="http://purl.obolibrary.org/obo/ENVO_01000197">
        <rdfs:subClassOf rdf:resource="http://purl.obolibrary.org/obo/ENVO_01000174"/>
        <obo:IAO_0000115 xml:lang="en">A broadleaf forest ecosystem which is undergoing climactic ecological succession.</obo:IAO_0000115>
        <oboInOwl:created_by>ORCID:0000-0002-4366-3088</oboInOwl:created_by>
        <oboInOwl:creation_date>2013-04-07T14:31:01Z</oboInOwl:creation_date>
        <rdfs:label>broadleaf forest biome</rdfs:label>
    </owl:Class>
    


    <!-- http://purl.obolibrary.org/obo/ENVO_01000198 -->

    <owl:Class rdf:about="http://purl.obolibrary.org/obo/ENVO_01000198">
        <rdfs:subClassOf rdf:resource="http://purl.obolibrary.org/obo/ENVO_01000174"/>
        <obo:IAO_0000115>A mixed forest in which dominant ecological communities have reached their climax successional state.</obo:IAO_0000115>
        <oboInOwl:created_by>ORCID:0000-0002-4366-3088</oboInOwl:created_by>
        <oboInOwl:creation_date>2013-04-07T14:31:01Z</oboInOwl:creation_date>
        <oboInOwl:inSubset>wwfBiome</oboInOwl:inSubset>
        <rdfs:label>mixed forest biome</rdfs:label>
    </owl:Class>
    


    <!-- http://purl.obolibrary.org/obo/ENVO_01000199 -->

    <owl:Class rdf:about="http://purl.obolibrary.org/obo/ENVO_01000199">
        <rdfs:subClassOf rdf:resource="http://purl.obolibrary.org/obo/ENVO_01000174"/>
        <rdfs:subClassOf rdf:resource="http://purl.obolibrary.org/obo/ENVO_01001833"/>
        <obo:IAO_0000115>A mediterranean forest in which dominant ecological communities have reached their climax successional state.</obo:IAO_0000115>
        <oboInOwl:created_by>ORCID:0000-0002-4366-3088</oboInOwl:created_by>
        <oboInOwl:creation_date>2013-04-07T14:31:01Z</oboInOwl:creation_date>
        <oboInOwl:inSubset>wwfBiome</oboInOwl:inSubset>
        <rdfs:label>mediterranean forest biome</rdfs:label>
    </owl:Class>
    


    <!-- http://purl.obolibrary.org/obo/ENVO_01000200 -->

    <owl:Class rdf:about="http://purl.obolibrary.org/obo/ENVO_01000200">
        <rdfs:subClassOf rdf:resource="http://purl.obolibrary.org/obo/ENVO_01000197"/>
        <rdfs:subClassOf rdf:resource="http://purl.obolibrary.org/obo/ENVO_01001830"/>
        <obo:IAO_0000115>A tropical broadleaf forest in which dominant ecological communities have reached their climax successional state.</obo:IAO_0000115>
        <oboInOwl:created_by>ORCID:0000-0002-4366-3088</oboInOwl:created_by>
        <oboInOwl:creation_date>2013-04-07T14:32:28Z</oboInOwl:creation_date>
        <rdfs:label>tropical broadleaf forest biome</rdfs:label>
    </owl:Class>
    


    <!-- http://purl.obolibrary.org/obo/ENVO_01000201 -->

    <owl:Class rdf:about="http://purl.obolibrary.org/obo/ENVO_01000201">
        <rdfs:subClassOf rdf:resource="http://purl.obolibrary.org/obo/ENVO_01000197"/>
        <rdfs:subClassOf rdf:resource="http://purl.obolibrary.org/obo/ENVO_01001832"/>
        <obo:IAO_0000115>A subtropical broadleaf forest in which dominant ecological communities have reached their climax successional state.</obo:IAO_0000115>
        <oboInOwl:created_by>ORCID:0000-0002-4366-3088</oboInOwl:created_by>
        <oboInOwl:creation_date>2013-04-07T14:32:28Z</oboInOwl:creation_date>
        <rdfs:label>subtropical broadleaf forest biome</rdfs:label>
    </owl:Class>
    


    <!-- http://purl.obolibrary.org/obo/ENVO_01000202 -->

    <owl:Class rdf:about="http://purl.obolibrary.org/obo/ENVO_01000202">
        <rdfs:subClassOf rdf:resource="http://purl.obolibrary.org/obo/ENVO_01000197"/>
        <rdfs:subClassOf rdf:resource="http://purl.obolibrary.org/obo/ENVO_01001831"/>
        <obo:IAO_0000115>A broadleaf forest which is subject to temperate climate patterns.</obo:IAO_0000115>
        <oboInOwl:created_by>ORCID:0000-0002-4366-3088</oboInOwl:created_by>
        <oboInOwl:creation_date>2013-04-07T14:32:28Z</oboInOwl:creation_date>
        <oboInOwl:inSubset>wwfBiome</oboInOwl:inSubset>
        <rdfs:label>temperate broadleaf forest biome</rdfs:label>
    </owl:Class>
    


    <!-- http://purl.obolibrary.org/obo/ENVO_01000208 -->

    <owl:Class rdf:about="http://purl.obolibrary.org/obo/ENVO_01000208">
        <rdfs:subClassOf rdf:resource="http://purl.obolibrary.org/obo/ENVO_01000222"/>
        <rdfs:subClassOf rdf:resource="http://purl.obolibrary.org/obo/ENVO_01001833"/>
        <obo:IAO_0000115>A subtropical woodland biome which includes communities adapted to hot to warm, dry summers, mild to cold, rainy winters, and the influence of large, usually marine, bodies of water.</obo:IAO_0000115>
        <oboInOwl:created_by>ORCID:0000-0002-4366-3088</oboInOwl:created_by>
        <oboInOwl:creation_date>2013-04-07T15:01:04Z</oboInOwl:creation_date>
        <rdfs:comment>Preliminary definition. The semantics and definitions of &quot;mediterranean&quot;, &quot;subtropical&quot;, &quot;tropical&quot;, &quot;temperate&quot;, &quot;polar&quot;, and similar climate types may be transferred to an &quot;environmental condition&quot; class once the semantics of this class have been established.</rdfs:comment>
        <rdfs:label>mediterranean woodland biome</rdfs:label>
    </owl:Class>
    


    <!-- http://purl.obolibrary.org/obo/ENVO_01000209 -->

    <owl:Class rdf:about="http://purl.obolibrary.org/obo/ENVO_01000209">
        <rdfs:subClassOf rdf:resource="http://purl.obolibrary.org/obo/ENVO_01000196"/>
        <rdfs:subClassOf rdf:resource="http://purl.obolibrary.org/obo/ENVO_01001832"/>
        <obo:IAO_0000115>A coniferous forest biome which is subject to subtropical climate patterns.</obo:IAO_0000115>
        <oboInOwl:created_by>ORCID:0000-0002-4366-3088</oboInOwl:created_by>
        <oboInOwl:creation_date>2013-04-07T14:39:14Z</oboInOwl:creation_date>
        <oboInOwl:inSubset>wwfBiome</oboInOwl:inSubset>
        <rdfs:comment>Preliminary definition. The semantics and definitions of &quot;mediterranean&quot;, &quot;subtropical&quot;, &quot;tropical&quot;, &quot;temperate&quot;, &quot;polar&quot;, and similar climate types may be transferred to an &quot;environmental condition&quot; class once the semantics of this class have been established.</rdfs:comment>
        <rdfs:label>subtropical coniferous forest biome</rdfs:label>
    </owl:Class>
    


    <!-- http://purl.obolibrary.org/obo/ENVO_01000210 -->

    <owl:Class rdf:about="http://purl.obolibrary.org/obo/ENVO_01000210">
        <rdfs:subClassOf rdf:resource="http://purl.obolibrary.org/obo/ENVO_01000196"/>
        <rdfs:subClassOf rdf:resource="http://purl.obolibrary.org/obo/ENVO_01001830"/>
        <obo:IAO_0000115>A coniferous forest biome which is subject to tropical climate patterns.</obo:IAO_0000115>
        <oboInOwl:created_by>ORCID:0000-0002-4366-3088</oboInOwl:created_by>
        <oboInOwl:creation_date>2013-04-07T14:39:14Z</oboInOwl:creation_date>
        <oboInOwl:inSubset>wwfBiome</oboInOwl:inSubset>
        <rdfs:comment>Preliminary definition. The semantics and definitions of &quot;mediterranean&quot;, &quot;subtropical&quot;, &quot;tropical&quot;, &quot;temperate&quot;, &quot;polar&quot;, and similar climate types may be transferred to an &quot;environmental condition&quot; class once the semantics of this class have been established.</rdfs:comment>
        <rdfs:label>tropical coniferous forest biome</rdfs:label>
    </owl:Class>
    


    <!-- http://purl.obolibrary.org/obo/ENVO_01000211 -->

    <owl:Class rdf:about="http://purl.obolibrary.org/obo/ENVO_01000211">
        <rdfs:subClassOf rdf:resource="http://purl.obolibrary.org/obo/ENVO_01000196"/>
        <rdfs:subClassOf rdf:resource="http://purl.obolibrary.org/obo/ENVO_01001831"/>
        <obo:IAO_0000115>A coniferous forest biome which is subject to temperate climate patterns.</obo:IAO_0000115>
        <oboInOwl:created_by>ORCID:0000-0002-4366-3088</oboInOwl:created_by>
        <oboInOwl:creation_date>2013-04-07T14:39:14Z</oboInOwl:creation_date>
        <oboInOwl:inSubset>wwfBiome</oboInOwl:inSubset>
        <rdfs:comment>Preliminary definition. The semantics and definitions of &quot;mediterranean&quot;, &quot;subtropical&quot;, &quot;tropical&quot;, &quot;temperate&quot;, &quot;polar&quot;, and similar climate types may be transferred to an &quot;environmental condition&quot; class once the semantics of this class have been established.</rdfs:comment>
        <rdfs:label>temperate coniferous forest biome</rdfs:label>
    </owl:Class>
    


    <!-- http://purl.obolibrary.org/obo/ENVO_01000212 -->

    <owl:Class rdf:about="http://purl.obolibrary.org/obo/ENVO_01000212">
        <rdfs:subClassOf rdf:resource="http://purl.obolibrary.org/obo/ENVO_01000198"/>
        <rdfs:subClassOf rdf:resource="http://purl.obolibrary.org/obo/ENVO_01001831"/>
        <obo:IAO_0000115>A temperate mixed forest in which dominant ecological communities have reached their climax successional state.</obo:IAO_0000115>
        <oboInOwl:created_by>ORCID:0000-0002-4366-3088</oboInOwl:created_by>
        <oboInOwl:creation_date>2013-04-07T14:39:30Z</oboInOwl:creation_date>
        <oboInOwl:inSubset>wwfBiome</oboInOwl:inSubset>
        <rdfs:label>temperate mixed forest biome</rdfs:label>
    </owl:Class>
    


    <!-- http://purl.obolibrary.org/obo/ENVO_01000213 -->

    <owl:Class rdf:about="http://purl.obolibrary.org/obo/ENVO_01000213">
        <rdfs:subClassOf rdf:resource="http://purl.obolibrary.org/obo/ENVO_01000176"/>
        <rdfs:subClassOf rdf:resource="http://purl.obolibrary.org/obo/ENVO_01001832"/>
        <obo:IAO_0000115>A shrubland biome which is subject to subtropical climate patterns.</obo:IAO_0000115>
        <oboInOwl:created_by>ORCID:0000-0002-4366-3088</oboInOwl:created_by>
        <oboInOwl:creation_date>2013-04-07T14:40:32Z</oboInOwl:creation_date>
        <oboInOwl:inSubset>wwfBiome</oboInOwl:inSubset>
        <rdfs:comment>Preliminary definition. The semantics and definitions of &quot;mediterranean&quot;, &quot;subtropical&quot;, &quot;tropical&quot;, &quot;temperate&quot;, &quot;polar&quot;, and similar climate types may be transferred to an &quot;environmental condition&quot; class once the semantics of this class have been established.</rdfs:comment>
        <rdfs:label>subtropical shrubland biome</rdfs:label>
    </owl:Class>
    


    <!-- http://purl.obolibrary.org/obo/ENVO_01000214 -->

    <owl:Class rdf:about="http://purl.obolibrary.org/obo/ENVO_01000214">
        <rdfs:subClassOf rdf:resource="http://purl.obolibrary.org/obo/ENVO_01000176"/>
        <rdfs:subClassOf rdf:resource="http://purl.obolibrary.org/obo/ENVO_01001830"/>
        <obo:IAO_0000115 xml:lang="en">A shrubland biome which is subject to tropical climate patterns.</obo:IAO_0000115>
        <oboInOwl:created_by>ORCID:0000-0002-4366-3088</oboInOwl:created_by>
        <oboInOwl:creation_date>2013-04-07T14:40:32Z</oboInOwl:creation_date>
        <oboInOwl:inSubset>wwfBiome</oboInOwl:inSubset>
        <rdfs:comment>Preliminary definition. The semantics and definitions of &quot;mediterranean&quot;, &quot;subtropical&quot;, &quot;tropical&quot;, &quot;temperate&quot;, &quot;polar&quot;, and similar climate types may be transferred to an &quot;environmental condition&quot; class once the semantics of this class have been established.</rdfs:comment>
        <rdfs:label>tropical shrubland biome</rdfs:label>
    </owl:Class>
    


    <!-- http://purl.obolibrary.org/obo/ENVO_01000215 -->

    <owl:Class rdf:about="http://purl.obolibrary.org/obo/ENVO_01000215">
        <rdfs:subClassOf rdf:resource="http://purl.obolibrary.org/obo/ENVO_01000176"/>
        <rdfs:subClassOf rdf:resource="http://purl.obolibrary.org/obo/ENVO_01001831"/>
        <obo:IAO_0000115 xml:lang="en">A shrubland biome which is subject to temperate climate patterns.</obo:IAO_0000115>
        <oboInOwl:created_by>ORCID:0000-0002-4366-3088</oboInOwl:created_by>
        <oboInOwl:creation_date>2013-04-07T14:40:32Z</oboInOwl:creation_date>
        <oboInOwl:hasBroadSynonym>prairie biome</oboInOwl:hasBroadSynonym>
        <rdfs:comment>Preliminary definition. The semantics and definitions of &quot;mediterranean&quot;, &quot;subtropical&quot;, &quot;tropical&quot;, &quot;temperate&quot;, &quot;polar&quot;, and similar climate types may be transferred to an &quot;environmental condition&quot; class once the semantics of this class have been established.</rdfs:comment>
        <rdfs:label>temperate shrubland biome</rdfs:label>
    </owl:Class>
    


    <!-- http://purl.obolibrary.org/obo/ENVO_01000216 -->

    <owl:Class rdf:about="http://purl.obolibrary.org/obo/ENVO_01000216">
        <rdfs:subClassOf rdf:resource="http://purl.obolibrary.org/obo/ENVO_01000176"/>
        <rdfs:subClassOf rdf:resource="http://purl.obolibrary.org/obo/ENVO_01001836"/>
        <obo:IAO_0000115>A montane shrubland biome is a shrubland biome which occurs in regions elevated above sea level and which has community structure determined by elevation-dependent environmental conditions.</obo:IAO_0000115>
        <oboInOwl:created_by>ORCID:0000-0002-4366-3088</oboInOwl:created_by>
        <oboInOwl:creation_date>2013-04-07T14:40:32Z</oboInOwl:creation_date>
        <oboInOwl:inSubset>wwfBiome</oboInOwl:inSubset>
        <rdfs:comment>Preliminary definition.</rdfs:comment>
        <rdfs:label>montane shrubland biome</rdfs:label>
    </owl:Class>
    


    <!-- http://purl.obolibrary.org/obo/ENVO_01000217 -->

    <owl:Class rdf:about="http://purl.obolibrary.org/obo/ENVO_01000217">
        <rdfs:subClassOf rdf:resource="http://purl.obolibrary.org/obo/ENVO_01000213"/>
        <rdfs:subClassOf rdf:resource="http://purl.obolibrary.org/obo/ENVO_01001833"/>
        <obo:IAO_0000115>A mediterranean shrubland biome is a subtropical shrubland biome which includes communities adapted to hot to warm, dry summers, mild to cold, rainy winters, and the influence of large, usually marine, bodies of water.</obo:IAO_0000115>
        <oboInOwl:created_by>ORCID:0000-0002-4366-3088</oboInOwl:created_by>
        <oboInOwl:creation_date>2013-04-07T14:40:32Z</oboInOwl:creation_date>
        <oboInOwl:inSubset>wwfBiome</oboInOwl:inSubset>
        <rdfs:comment>Preliminary definition. The semantics and definitions of &quot;mediterranean&quot;, &quot;subtropical&quot;, &quot;tropical&quot;, &quot;temperate&quot;, &quot;polar&quot;, and similar climate types may be transferred to an &quot;environmental condition&quot; class once the semantics of this class have been established.</rdfs:comment>
        <rdfs:label>mediterranean shrubland biome</rdfs:label>
    </owl:Class>
    


    <!-- http://purl.obolibrary.org/obo/ENVO_01000218 -->

    <owl:Class rdf:about="http://purl.obolibrary.org/obo/ENVO_01000218">
        <rdfs:subClassOf rdf:resource="http://purl.obolibrary.org/obo/ENVO_01000176"/>
        <oboInOwl:created_by>ORCID:0000-0002-4366-3088</oboInOwl:created_by>
        <oboInOwl:creation_date>2013-04-07T14:40:32Z</oboInOwl:creation_date>
        <oboInOwl:hasOBONamespace>ENVO</oboInOwl:hasOBONamespace>
        <oboInOwl:id>ENVO:01000218</oboInOwl:id>
        <oboInOwl:inSubset>wwfBiome</oboInOwl:inSubset>
        <rdfs:comment>Preliminary definition. The semantics and definitions of &quot;mediterranean&quot;, &quot;subtropical&quot;, &quot;tropical&quot;, &quot;temperate&quot;, &quot;polar&quot;, and similar climate types may be transferred to an &quot;environmental condition&quot; class once the semantics of this class have been established.</rdfs:comment>
        <rdfs:label>xeric shrubland biome</rdfs:label>
    </owl:Class>
    


    <!-- http://purl.obolibrary.org/obo/ENVO_01000219 -->

    <owl:Class rdf:about="http://purl.obolibrary.org/obo/ENVO_01000219">
        <rdfs:subClassOf rdf:resource="http://purl.obolibrary.org/obo/ENVO_00000446"/>
        <obo:IAO_0000115>An anthropogenic terrestrial biome is a terrestrial biome which has community structures determined by human activity.</obo:IAO_0000115>
        <oboInOwl:created_by>ORCID:0000-0002-4366-3088</oboInOwl:created_by>
        <oboInOwl:creation_date>2013-04-07T14:45:22Z</oboInOwl:creation_date>
        <oboInOwl:hasExactSynonym>anthrome</oboInOwl:hasExactSynonym>
        <oboInOwl:hasExactSynonym>human biome</oboInOwl:hasExactSynonym>
        <rdfs:comment>Preliminary definition.</rdfs:comment>
        <rdfs:label>anthropogenic terrestrial biome</rdfs:label>
    </owl:Class>
    <owl:Axiom>
        <owl:annotatedSource rdf:resource="http://purl.obolibrary.org/obo/ENVO_01000219"/>
        <owl:annotatedProperty rdf:resource="http://purl.obolibrary.org/obo/IAO_0000115"/>
        <owl:annotatedTarget>An anthropogenic terrestrial biome is a terrestrial biome which has community structures determined by human activity.</owl:annotatedTarget>
        <oboInOwl:hasDbXref>http://www.eoearth.org/view/article/150128/</oboInOwl:hasDbXref>
    </owl:Axiom>
    


    <!-- http://purl.obolibrary.org/obo/ENVO_01000220 -->

    <owl:Class rdf:about="http://purl.obolibrary.org/obo/ENVO_01000220">
        <rdfs:subClassOf rdf:resource="http://purl.obolibrary.org/obo/ENVO_01000175"/>
        <rdfs:subClassOf rdf:resource="http://purl.obolibrary.org/obo/ENVO_01001830"/>
        <obo:IAO_0000115 xml:lang="en">A woodland biome which is subject to tropical climate patterns.</obo:IAO_0000115>
        <oboInOwl:created_by>ORCID:0000-0002-4366-3088</oboInOwl:created_by>
        <oboInOwl:creation_date>2013-04-07T15:01:04Z</oboInOwl:creation_date>
        <rdfs:comment>Preliminary definition. The semantics and definitions of &quot;mediterranean&quot;, &quot;subtropical&quot;, &quot;tropical&quot;, &quot;temperate&quot;, &quot;polar&quot;, and similar climate types may be transferred to an &quot;environmental condition&quot; class once the semantics of this class have been established.</rdfs:comment>
        <rdfs:label>tropical woodland biome</rdfs:label>
    </owl:Class>
    


    <!-- http://purl.obolibrary.org/obo/ENVO_01000221 -->

    <owl:Class rdf:about="http://purl.obolibrary.org/obo/ENVO_01000221">
        <rdfs:subClassOf rdf:resource="http://purl.obolibrary.org/obo/ENVO_01000175"/>
        <rdfs:subClassOf rdf:resource="http://purl.obolibrary.org/obo/ENVO_01001831"/>
        <obo:IAO_0000115 xml:lang="en">A woodland biome which is subject to temperate climate patterns.</obo:IAO_0000115>
        <oboInOwl:created_by>ORCID:0000-0002-4366-3088</oboInOwl:created_by>
        <oboInOwl:creation_date>2013-04-07T15:01:04Z</oboInOwl:creation_date>
        <rdfs:comment>Preliminary definition. The semantics and definitions of &quot;mediterranean&quot;, &quot;subtropical&quot;, &quot;tropical&quot;, &quot;temperate&quot;, &quot;polar&quot;, and similar climate types may be transferred to an &quot;environmental condition&quot; class once the semantics of this class have been established.</rdfs:comment>
        <rdfs:label>temperate woodland biome</rdfs:label>
    </owl:Class>
    


    <!-- http://purl.obolibrary.org/obo/ENVO_01000222 -->

    <owl:Class rdf:about="http://purl.obolibrary.org/obo/ENVO_01000222">
        <rdfs:subClassOf rdf:resource="http://purl.obolibrary.org/obo/ENVO_01000175"/>
        <rdfs:subClassOf rdf:resource="http://purl.obolibrary.org/obo/ENVO_01001832"/>
        <obo:IAO_0000115>A woodland biome which is subject to subtropical climate patterns.</obo:IAO_0000115>
        <oboInOwl:created_by>ORCID:0000-0002-4366-3088</oboInOwl:created_by>
        <oboInOwl:creation_date>2013-04-07T15:01:04Z</oboInOwl:creation_date>
        <rdfs:comment>Preliminary definition. The semantics and definitions of &quot;mediterranean&quot;, &quot;subtropical&quot;, &quot;tropical&quot;, &quot;temperate&quot;, &quot;polar&quot;, and similar climate types may be transferred to an &quot;environmental condition&quot; class once the semantics of this class have been established.</rdfs:comment>
        <rdfs:label>subtropical woodland biome</rdfs:label>
    </owl:Class>
    


    <!-- http://purl.obolibrary.org/obo/ENVO_01000223 -->

    <owl:Class rdf:about="http://purl.obolibrary.org/obo/ENVO_01000223">
        <rdfs:subClassOf rdf:resource="http://purl.obolibrary.org/obo/ENVO_01000178"/>
        <rdfs:subClassOf rdf:resource="http://purl.obolibrary.org/obo/ENVO_01001836"/>
        <obo:IAO_0000115>A montane savanna biome is a savanna biome which occurs in regions elevated above sea level and which has community structure determined by elevation-dependent environmental conditions.</obo:IAO_0000115>
        <oboInOwl:created_by>ORCID:0000-0002-4366-3088</oboInOwl:created_by>
        <oboInOwl:creation_date>2013-04-07T16:50:01Z</oboInOwl:creation_date>
        <rdfs:comment>Preliminary definition.</rdfs:comment>
        <rdfs:label>montane savanna biome</rdfs:label>
    </owl:Class>
    


    <!-- http://purl.obolibrary.org/obo/ENVO_01000224 -->

    <owl:Class rdf:about="http://purl.obolibrary.org/obo/ENVO_01000224">
        <rdfs:subClassOf rdf:resource="http://purl.obolibrary.org/obo/ENVO_01000191"/>
        <rdfs:subClassOf rdf:resource="http://purl.obolibrary.org/obo/ENVO_01001833"/>
        <obo:IAO_0000115>A subtropical grassland biome which includes communities adapted to hot to warm, dry summers, mild to cold, rainy winters, and the influence of large, usually marine, bodies of water.</obo:IAO_0000115>
        <oboInOwl:created_by>ORCID:0000-0002-4366-3088</oboInOwl:created_by>
        <oboInOwl:creation_date>2013-04-19T11:42:48Z</oboInOwl:creation_date>
        <rdfs:comment>Preliminary definition. The semantics and definitions of &quot;mediterranean&quot;, &quot;subtropical&quot;, &quot;tropical&quot;, &quot;temperate&quot;, &quot;polar&quot;, and similar climate types may be transferred to an &quot;environmental condition&quot; class once the semantics of this class have been established.</rdfs:comment>
        <rdfs:label>mediterranean grassland biome</rdfs:label>
    </owl:Class>
    


    <!-- http://purl.obolibrary.org/obo/ENVO_01000225 -->

    <owl:Class rdf:about="http://purl.obolibrary.org/obo/ENVO_01000225">
        <rdfs:subClassOf rdf:resource="http://purl.obolibrary.org/obo/ENVO_01000201"/>
        <obo:IAO_0000115>A subtropical dry broadleaf forest in which dominant ecological communities have reached their climax successional state.</obo:IAO_0000115>
        <oboInOwl:created_by>ORCID:0000-0002-4366-3088</oboInOwl:created_by>
        <oboInOwl:creation_date>2013-04-24T12:04:53Z</oboInOwl:creation_date>
        <oboInOwl:hasDbXref rdf:resource="https://www.worldwildlife.org/biomes/tropical-and-subtropical-dry-broadleaf-forests"/>
        <oboInOwl:inSubset>wwfBiome</oboInOwl:inSubset>
        <rdfs:label>subtropical dry broadleaf forest biome</rdfs:label>
    </owl:Class>
    


    <!-- http://purl.obolibrary.org/obo/ENVO_01000226 -->

    <owl:Class rdf:about="http://purl.obolibrary.org/obo/ENVO_01000226">
        <rdfs:subClassOf rdf:resource="http://purl.obolibrary.org/obo/ENVO_01000201"/>
        <obo:IAO_0000115>A subtropical moist broadleaf forest in which dominant ecological communities have reached their climax successional state.</obo:IAO_0000115>
        <oboInOwl:created_by>ORCID:0000-0002-4366-3088</oboInOwl:created_by>
        <oboInOwl:creation_date>2013-04-24T12:04:53Z</oboInOwl:creation_date>
        <oboInOwl:inSubset>wwfBiome</oboInOwl:inSubset>
        <rdfs:label>subtropical moist broadleaf forest biome</rdfs:label>
    </owl:Class>
    


    <!-- http://purl.obolibrary.org/obo/ENVO_01000227 -->

    <owl:Class rdf:about="http://purl.obolibrary.org/obo/ENVO_01000227">
        <rdfs:subClassOf rdf:resource="http://purl.obolibrary.org/obo/ENVO_01000200"/>
        <obo:IAO_0000115>A tropical dry broadleaf forest in which dominant ecological communities have reached their climax successional state.</obo:IAO_0000115>
        <oboInOwl:created_by>ORCID:0000-0002-4366-3088</oboInOwl:created_by>
        <oboInOwl:creation_date>2013-04-24T12:05:25Z</oboInOwl:creation_date>
        <oboInOwl:hasDbXref rdf:resource="https://www.worldwildlife.org/biomes/tropical-and-subtropical-dry-broadleaf-forests"/>
        <oboInOwl:inSubset>wwfBiome</oboInOwl:inSubset>
        <rdfs:label>tropical dry broadleaf forest biome</rdfs:label>
    </owl:Class>
    


    <!-- http://purl.obolibrary.org/obo/ENVO_01000228 -->

    <owl:Class rdf:about="http://purl.obolibrary.org/obo/ENVO_01000228">
        <rdfs:subClassOf rdf:resource="http://purl.obolibrary.org/obo/ENVO_01000200"/>
        <obo:IAO_0000115>A tropical moist broadleaf forest in which dominant ecological communities have reached their climax successional state.</obo:IAO_0000115>
        <oboInOwl:created_by>ORCID:0000-0002-4366-3088</oboInOwl:created_by>
        <oboInOwl:creation_date>2013-04-24T12:05:25Z</oboInOwl:creation_date>
        <oboInOwl:hasDbXref>SPIRE:Rainforest</oboInOwl:hasDbXref>
        <oboInOwl:hasRelatedSynonym>rainforest biome</oboInOwl:hasRelatedSynonym>
        <oboInOwl:inSubset>wwfBiome</oboInOwl:inSubset>
        <rdfs:label>tropical moist broadleaf forest biome</rdfs:label>
    </owl:Class>
    


    <!-- http://purl.obolibrary.org/obo/ENVO_01000229 -->

    <owl:Class rdf:about="http://purl.obolibrary.org/obo/ENVO_01000229">
        <rdfs:subClassOf rdf:resource="http://purl.obolibrary.org/obo/ENVO_01000187"/>
        <rdfs:subClassOf rdf:resource="http://purl.obolibrary.org/obo/ENVO_01001833"/>
        <obo:IAO_0000115>A savanna biome which is subject to mediterranean climate patterns.</obo:IAO_0000115>
        <oboInOwl:created_by>ORCID:0000-0002-4366-3088</oboInOwl:created_by>
        <oboInOwl:creation_date>2013-04-24T12:20:42Z</oboInOwl:creation_date>
        <oboInOwl:inSubset>wwfBiome</oboInOwl:inSubset>
        <rdfs:label>mediterranean savanna biome</rdfs:label>
    </owl:Class>
    


    <!-- http://purl.obolibrary.org/obo/ENVO_01000245 -->

    <owl:Class rdf:about="http://purl.obolibrary.org/obo/ENVO_01000245">
        <rdfs:subClassOf rdf:resource="http://purl.obolibrary.org/obo/ENVO_01000219"/>
        <obo:IAO_0000115 xml:lang="en">A cropland ecosystem which is undergoing climactic ecological succession.</obo:IAO_0000115>
        <oboInOwl:created_by>ORCID:0000-0002-4366-3088</oboInOwl:created_by>
        <oboInOwl:creation_date>2013-06-14T11:45:47Z</oboInOwl:creation_date>
        <rdfs:label>cropland biome</rdfs:label>
    </owl:Class>
    <owl:Axiom>
        <owl:annotatedSource rdf:resource="http://purl.obolibrary.org/obo/ENVO_01000245"/>
        <owl:annotatedProperty rdf:resource="http://purl.obolibrary.org/obo/IAO_0000115"/>
        <owl:annotatedTarget xml:lang="en">A cropland ecosystem which is undergoing climactic ecological succession.</owl:annotatedTarget>
        <oboInOwl:hasDbXref rdf:resource="http://dx.doi.org/10.1111/j.1466-8238.2010.00540.x"/>
        <oboInOwl:hasDbXref rdf:resource="http://dx.doi.org/10.1890/070062"/>
    </owl:Axiom>
    


    <!-- http://purl.obolibrary.org/obo/ENVO_01000246 -->

    <owl:Class rdf:about="http://purl.obolibrary.org/obo/ENVO_01000246">
        <rdfs:subClassOf rdf:resource="http://purl.obolibrary.org/obo/ENVO_00000428"/>
        <obo:IAO_0000115>A village biome is an anthropogenic terrestrial biome which contains settlements such as villages, towns, and/or small cities and which is primarily used for agricultural activity.</obo:IAO_0000115>
        <oboInOwl:created_by>ORCID:0000-0002-4366-3088</oboInOwl:created_by>
        <oboInOwl:creation_date>2013-06-14T11:45:47Z</oboInOwl:creation_date>
        <rdfs:comment>Villages are also described as agricultural settlements with greater than 100 persons per square kilometre; however, no upper limit is defined.</rdfs:comment>
        <rdfs:label>village biome</rdfs:label>
    </owl:Class>
    <owl:Axiom>
        <owl:annotatedSource rdf:resource="http://purl.obolibrary.org/obo/ENVO_01000246"/>
        <owl:annotatedProperty rdf:resource="http://purl.obolibrary.org/obo/IAO_0000115"/>
        <owl:annotatedTarget>A village biome is an anthropogenic terrestrial biome which contains settlements such as villages, towns, and/or small cities and which is primarily used for agricultural activity.</owl:annotatedTarget>
        <oboInOwl:hasDbXref>DOI:10.1111/j.1466-8238.2010.00540.x</oboInOwl:hasDbXref>
        <oboInOwl:hasDbXref>DOI:10.1890/070062</oboInOwl:hasDbXref>
    </owl:Axiom>
    


    <!-- http://purl.obolibrary.org/obo/ENVO_01000247 -->

    <owl:Class rdf:about="http://purl.obolibrary.org/obo/ENVO_01000247">
        <rdfs:subClassOf rdf:resource="http://purl.obolibrary.org/obo/ENVO_01000219"/>
        <obo:IAO_0000115>A rangeland biome is an anthropogenic terrestrial biome which is primarily used for the rearing and grazing of livestock.</obo:IAO_0000115>
        <oboInOwl:created_by>ORCID:0000-0002-4366-3088</oboInOwl:created_by>
        <oboInOwl:creation_date>2013-06-14T11:45:47Z</oboInOwl:creation_date>
        <rdfs:label>rangeland biome</rdfs:label>
    </owl:Class>
    <owl:Axiom>
        <owl:annotatedSource rdf:resource="http://purl.obolibrary.org/obo/ENVO_01000247"/>
        <owl:annotatedProperty rdf:resource="http://purl.obolibrary.org/obo/IAO_0000115"/>
        <owl:annotatedTarget>A rangeland biome is an anthropogenic terrestrial biome which is primarily used for the rearing and grazing of livestock.</owl:annotatedTarget>
        <oboInOwl:hasDbXref>DOI:10.1111/j.1466-8238.2010.00540.x</oboInOwl:hasDbXref>
        <oboInOwl:hasDbXref>DOI:10.1890/070062</oboInOwl:hasDbXref>
    </owl:Axiom>
    


    <!-- http://purl.obolibrary.org/obo/ENVO_01000248 -->

    <owl:Class rdf:about="http://purl.obolibrary.org/obo/ENVO_01000248">
        <rdfs:subClassOf rdf:resource="http://purl.obolibrary.org/obo/ENVO_00000428"/>
        <obo:IAO_0000115>A dense settlement biome is an anthropogenic terrestrial biome which is primarily used for human habitation, recreation, and industry within built structures with little other land use.</obo:IAO_0000115>
        <oboInOwl:created_by>ORCID:0000-0002-4366-3088</oboInOwl:created_by>
        <oboInOwl:creation_date>2013-06-14T11:45:47Z</oboInOwl:creation_date>
        <oboInOwl:id>ENVO:01000248</oboInOwl:id>
        <rdfs:label>dense settlement biome</rdfs:label>
    </owl:Class>
    <owl:Axiom>
        <owl:annotatedSource rdf:resource="http://purl.obolibrary.org/obo/ENVO_01000248"/>
        <owl:annotatedProperty rdf:resource="http://purl.obolibrary.org/obo/IAO_0000115"/>
        <owl:annotatedTarget>A dense settlement biome is an anthropogenic terrestrial biome which is primarily used for human habitation, recreation, and industry within built structures with little other land use.</owl:annotatedTarget>
        <oboInOwl:hasDbXref>DOI:10.1111/j.1466-8238.2010.00540.x</oboInOwl:hasDbXref>
        <oboInOwl:hasDbXref>DOI:10.1890/070062</oboInOwl:hasDbXref>
    </owl:Axiom>
    


    <!-- http://purl.obolibrary.org/obo/ENVO_01000249 -->

    <owl:Class rdf:about="http://purl.obolibrary.org/obo/ENVO_01000249">
        <rdfs:subClassOf rdf:resource="http://purl.obolibrary.org/obo/ENVO_01000248"/>
        <obo:IAO_0000115>An urban biome is a dense settlement biome which has been urbanised.</obo:IAO_0000115>
        <oboInOwl:created_by>ORCID:0000-0002-4366-3088</oboInOwl:created_by>
        <oboInOwl:creation_date>2013-06-14T11:45:47Z</oboInOwl:creation_date>
        <oboInOwl:hasDbXref>SPIRE:Urban</oboInOwl:hasDbXref>
        <oboInOwl:hasOBONamespace>ENVO</oboInOwl:hasOBONamespace>
        <oboInOwl:id>ENVO:01000249</oboInOwl:id>
        <rdfs:label>urban biome</rdfs:label>
    </owl:Class>
    <owl:Axiom>
        <owl:annotatedSource rdf:resource="http://purl.obolibrary.org/obo/ENVO_01000249"/>
        <owl:annotatedProperty rdf:resource="http://purl.obolibrary.org/obo/IAO_0000115"/>
        <owl:annotatedTarget>An urban biome is a dense settlement biome which has been urbanised.</owl:annotatedTarget>
        <oboInOwl:hasDbXref>DOI:10.1111/j.1466-8238.2010.00540.x</oboInOwl:hasDbXref>
        <oboInOwl:hasDbXref>DOI:10.1890/070062</oboInOwl:hasDbXref>
    </owl:Axiom>
    


    <!-- http://purl.obolibrary.org/obo/ENVO_01000250 -->

    <owl:Class rdf:about="http://purl.obolibrary.org/obo/ENVO_01000250">
        <rdfs:subClassOf rdf:resource="http://purl.obolibrary.org/obo/ENVO_01000196"/>
        <rdfs:subClassOf rdf:resource="http://purl.obolibrary.org/obo/ENVO_01001834"/>
        <obo:IAO_0000115>A  coniferous forest biome which includes communities adapted to subpolar conditions.</obo:IAO_0000115>
        <oboInOwl:creation_date>2013-09-04T06:41:53Z</oboInOwl:creation_date>
        <oboInOwl:hasDbXref>EcoLexicon:taiga</oboInOwl:hasDbXref>
        <oboInOwl:hasDbXref>LTER:72</oboInOwl:hasDbXref>
        <oboInOwl:hasDbXref>SPIRE:Taiga</oboInOwl:hasDbXref>
        <oboInOwl:hasNarrowSynonym>boreal forest</oboInOwl:hasNarrowSynonym>
        <oboInOwl:hasNarrowSynonym>taiga</oboInOwl:hasNarrowSynonym>
        <oboInOwl:inSubset>wwfBiome</oboInOwl:inSubset>
        <rdfs:label>subpolar coniferous forest biome</rdfs:label>
    </owl:Class>
    


    <!-- http://purl.obolibrary.org/obo/ENVO_01000252 -->

    <owl:Class rdf:about="http://purl.obolibrary.org/obo/ENVO_01000252">
        <rdfs:subClassOf rdf:resource="http://purl.obolibrary.org/obo/ENVO_00000873"/>
        <obo:IAO_0000115>A biome which is determined by a freshwater lake.</obo:IAO_0000115>
        <oboInOwl:creation_date>2013-09-19T11:11:01Z</oboInOwl:creation_date>
        <rdfs:label>freshwater lake biome</rdfs:label>
    </owl:Class>
    


    <!-- http://purl.obolibrary.org/obo/ENVO_01000253 -->

    <owl:Class rdf:about="http://purl.obolibrary.org/obo/ENVO_01000253">
        <rdfs:subClassOf rdf:resource="http://purl.obolibrary.org/obo/ENVO_00000873"/>
        <obo:IAO_0000115 xml:lang="en">A freshwater biome which is determined by a freshwater river.</obo:IAO_0000115>
        <oboInOwl:creation_date>2013-09-19T11:11:01Z</oboInOwl:creation_date>
        <rdfs:label>freshwater river biome</rdfs:label>
    </owl:Class>
    


    <!-- http://purl.obolibrary.org/obo/ENVO_01000339 -->

    <owl:Class rdf:about="http://purl.obolibrary.org/obo/ENVO_01000339">
        <rdfs:subClassOf rdf:resource="http://purl.obolibrary.org/obo/ENVO_00000428"/>
        <obo:IAO_0000115>A biome which is subject to polar climatic conditions.</obo:IAO_0000115>
        <oboInOwl:inSubset>envoPolar</oboInOwl:inSubset>
        <rdfs:comment>This class is primarily for inference and, in general, should not be used directly by annotators. If you&apos;re an annotator, please consider using a more informative term such as &apos;tundra biome&apos;.</rdfs:comment>
        <rdfs:label>polar biome</rdfs:label>
    </owl:Class>
    


    <!-- http://purl.obolibrary.org/obo/ENVO_01000854 -->

    <owl:Class rdf:about="http://purl.obolibrary.org/obo/ENVO_01000854">
        <rdfs:subClassOf rdf:resource="http://purl.obolibrary.org/obo/ENVO_01000049"/>
        <rdfs:subClassOf rdf:resource="http://purl.obolibrary.org/obo/ENVO_01001830"/>
        <obo:IAO_0000115>A marine coral reef biome which is located in a region with a tropical climate.</obo:IAO_0000115>
        <oboInOwl:inSubset>wwfBiome</oboInOwl:inSubset>
        <rdfs:label xml:lang="en">tropical marine coral reef biome</rdfs:label>
    </owl:Class>
    


    <!-- http://purl.obolibrary.org/obo/ENVO_01000856 -->

    <owl:Class rdf:about="http://purl.obolibrary.org/obo/ENVO_01000856">
        <rdfs:subClassOf rdf:resource="http://purl.obolibrary.org/obo/ENVO_01000046"/>
        <rdfs:subClassOf rdf:resource="http://purl.obolibrary.org/obo/ENVO_01001831"/>
        <obo:IAO_0000115>A marginal sea biome which is located in a region with a temperate climate.</obo:IAO_0000115>
        <obo:IAO_0000116>A component of the WWF Temperate Shelf and seas ecoregions grouping</obo:IAO_0000116>
        <oboInOwl:inSubset>wwfBiome</oboInOwl:inSubset>
        <rdfs:label xml:lang="en">temperate marginal sea biome</rdfs:label>
    </owl:Class>
    


    <!-- http://purl.obolibrary.org/obo/ENVO_01000857 -->

    <owl:Class rdf:about="http://purl.obolibrary.org/obo/ENVO_01000857">
        <rdfs:subClassOf rdf:resource="http://purl.obolibrary.org/obo/ENVO_01000047"/>
        <obo:IAO_0000115 xml:lang="en">A mediterranean sea biome which is subject to temperate climate patterns.</obo:IAO_0000115>
        <oboInOwl:inSubset>wwfBiome</oboInOwl:inSubset>
        <rdfs:label xml:lang="en">temperate mediterranean sea biome</rdfs:label>
    </owl:Class>
    


    <!-- http://purl.obolibrary.org/obo/ENVO_01000858 -->

    <owl:Class rdf:about="http://purl.obolibrary.org/obo/ENVO_01000858">
        <rdfs:subClassOf rdf:resource="http://purl.obolibrary.org/obo/ENVO_00000447"/>
        <obo:IAO_0000115>A marine biome which contains communities adapted to living in an environment determined by an upwelling process.</obo:IAO_0000115>
        <rdfs:label xml:lang="en">marine upwelling biome</rdfs:label>
    </owl:Class>
    


    <!-- http://purl.obolibrary.org/obo/ENVO_01000859 -->

    <owl:Class rdf:about="http://purl.obolibrary.org/obo/ENVO_01000859">
        <rdfs:subClassOf rdf:resource="http://purl.obolibrary.org/obo/ENVO_01000858"/>
        <rdfs:subClassOf rdf:resource="http://purl.obolibrary.org/obo/ENVO_01001830"/>
        <obo:IAO_0000115>A marine upwelling biome which is subject to tropical climate patterns.</obo:IAO_0000115>
        <oboInOwl:inSubset>wwfBiome</oboInOwl:inSubset>
        <rdfs:label xml:lang="en">tropical marine upwelling biome</rdfs:label>
    </owl:Class>
    


    <!-- http://purl.obolibrary.org/obo/ENVO_01000860 -->

    <owl:Class rdf:about="http://purl.obolibrary.org/obo/ENVO_01000860">
        <rdfs:subClassOf rdf:resource="http://purl.obolibrary.org/obo/ENVO_01000858"/>
        <rdfs:subClassOf rdf:resource="http://purl.obolibrary.org/obo/ENVO_01001831"/>
        <obo:IAO_0000115>A marine upwelling biome which is located in a region subject to temperate climate patterns.</obo:IAO_0000115>
        <oboInOwl:inSubset>wwfBiome</oboInOwl:inSubset>
        <rdfs:label xml:lang="en">temperate marine upwelling biome</rdfs:label>
    </owl:Class>
    


    <!-- http://purl.obolibrary.org/obo/ENVO_01001230 -->

    <owl:Class rdf:about="http://purl.obolibrary.org/obo/ENVO_01001230">
        <rdfs:subClassOf rdf:resource="http://purl.obolibrary.org/obo/ENVO_01000046"/>
        <rdfs:subClassOf rdf:resource="http://purl.obolibrary.org/obo/ENVO_01001830"/>
        <obo:IAO_0000115>A marginal sea biome which is located in a region with a tropical climate.</obo:IAO_0000115>
        <obo:IAO_0000116>A class which is complementary to the WWF Temperate Shelf and Seas ecoregions grouping</obo:IAO_0000116>
        <rdfs:label xml:lang="en">tropical marginal sea biome</rdfs:label>
    </owl:Class>
    


    <!-- http://purl.obolibrary.org/obo/ENVO_01001369 -->

    <owl:Class rdf:about="http://purl.obolibrary.org/obo/ENVO_01001369">
        <rdfs:subClassOf rdf:resource="http://purl.obolibrary.org/obo/ENVO_01000176"/>
        <obo:IAO_0000115>A shrubland biome which is densely vegetated by dwarf or short mangroves (and associates) that are generally less than 6 meters in height, is tidally influenced,  is located in tropical or subtropical areas.</obo:IAO_0000115>
        <oboInOwl:created_by rdf:resource="https://orcid.org/0000-0002-4366-3088"/>
        <oboInOwl:hasDbXref>CMECS:577</oboInOwl:hasDbXref>
        <oboInOwl:hasDbXref>https://cmecscatalog.org/cmecs/classification/unit/577.html</oboInOwl:hasDbXref>
        <oboInOwl:inSubset>envoCmecs</oboInOwl:inSubset>
        <oboInOwl:inSubset>envoMarine</oboInOwl:inSubset>
        <rdfs:comment>This class aligns to the Coastal and Marine Ecological Classification Standard (CMECS). In ENVO, we may adapt the definition for consistency, but the semantics (meaning) of the term should be unaffected. Please consult the CMECS catalogue (https://cmecscatalog.org/) for authoritative and semantically unconstrained definitions. CMECS provides the following notes: &quot;Commonly found on intertidal mud flats along the shores of estuaries. Tidal mangrove shrublands may include immature stands or stunted mature trees that indicate a harsh growing environment. Areas characterized by tall mangroves (&gt; 6 meters) are placed in the Tidal Mangrove Forest Biotic Group. Where tidal amplitude is relatively low, the vegetation forms narrow bands along the coastal plains, and it rarely penetrates inland more than several kilometers along rivers. Where tidal amplitude is greater, mangroves extend further inland along river courses, forming extensive stands in the major river deltas. Also, mangrove cays may occur within the lagoon complex of barrier reefs. The list of biotic communities for this group is long: a few examples are provided below, and the complete list is available in Appendix F&quot;</rdfs:comment>
        <rdfs:label xml:lang="en">tidal mangrove shrubland</rdfs:label>
    </owl:Class>
    


    <!-- http://purl.obolibrary.org/obo/ENVO_01001505 -->

    <owl:Class rdf:about="http://purl.obolibrary.org/obo/ENVO_01001505">
        <rdfs:subClassOf rdf:resource="http://purl.obolibrary.org/obo/ENVO_01000180"/>
        <rdfs:subClassOf rdf:resource="http://purl.obolibrary.org/obo/ENVO_01001835"/>
        <obo:IAO_0000115>A tundra biome which exists at high altitudes and where vegetation - dominated by a few species of dwarf shrubs, a few grasses, sedges, lichens, and mosses - is stunted due to low temperatures and high winds.</obo:IAO_0000115>
        <oboInOwl:created_by rdf:resource="https://orcid.org/0000-0002-4366-3088"/>
        <oboInOwl:creation_date rdf:datatype="http://www.w3.org/2001/XMLSchema#dateTime">2019-01-14T16:26:18Z</oboInOwl:creation_date>
        <oboInOwl:hasDbXref>SPIRE:Tundra</oboInOwl:hasDbXref>
        <oboInOwl:hasDbXref>http://sweetontology.net/realmCryo/AlpineTundra</oboInOwl:hasDbXref>
        <oboInOwl:hasExactSynonym>mountain tundra</oboInOwl:hasExactSynonym>
        <oboInOwl:inSubset>envoPolar</oboInOwl:inSubset>
        <rdfs:comment>The absence of trees in this biome is primarily due to high altitude rather than high latitude. On Earth, it lies roughly between the summer isotherm of 10 degrees Centigrade and the snow line. Primary productivity is low in this biome because of the extremes of climate.</rdfs:comment>
        <rdfs:label xml:lang="en">alpine tundra biome</rdfs:label>
    </owl:Class>
    <owl:Axiom>
        <owl:annotatedSource rdf:resource="http://purl.obolibrary.org/obo/ENVO_01001505"/>
        <owl:annotatedProperty rdf:resource="http://purl.obolibrary.org/obo/IAO_0000115"/>
        <owl:annotatedTarget>A tundra biome which exists at high altitudes and where vegetation - dominated by a few species of dwarf shrubs, a few grasses, sedges, lichens, and mosses - is stunted due to low temperatures and high winds.</owl:annotatedTarget>
        <oboInOwl:hasDbXref>https://en.wikipedia.org/wiki/Alpine_tundra</oboInOwl:hasDbXref>
    </owl:Axiom>
    <owl:Axiom>
        <owl:annotatedSource rdf:resource="http://purl.obolibrary.org/obo/ENVO_01001505"/>
        <owl:annotatedProperty rdf:resource="http://www.geneontology.org/formats/oboInOwl#hasExactSynonym"/>
        <owl:annotatedTarget>mountain tundra</owl:annotatedTarget>
        <oboInOwl:hasDbXref>https://orcid.org/0000-0003-4808-4736</oboInOwl:hasDbXref>
    </owl:Axiom>
    <owl:Axiom>
        <owl:annotatedSource rdf:resource="http://purl.obolibrary.org/obo/ENVO_01001505"/>
        <owl:annotatedProperty rdf:resource="http://www.w3.org/2000/01/rdf-schema#comment"/>
        <owl:annotatedTarget>The absence of trees in this biome is primarily due to high altitude rather than high latitude. On Earth, it lies roughly between the summer isotherm of 10 degrees Centigrade and the snow line. Primary productivity is low in this biome because of the extremes of climate.</owl:annotatedTarget>
        <oboInOwl:hasDbXref>https://orcid.org/0000-0003-4808-4736</oboInOwl:hasDbXref>
    </owl:Axiom>
    


    <!-- http://purl.obolibrary.org/obo/ENVO_01001798 -->

    <owl:Class rdf:about="http://purl.obolibrary.org/obo/ENVO_01001798">
        <rdfs:subClassOf rdf:resource="http://purl.obolibrary.org/obo/ENVO_01000198"/>
        <rdfs:subClassOf rdf:resource="http://purl.obolibrary.org/obo/ENVO_01001830"/>
        <obo:IAO_0000115>A tropical mixed forest in which dominant ecological communities have reached their climax successional state.</obo:IAO_0000115>
        <dc:creator rdf:resource="https://orcid.org/0000-0002-4366-3088"/>
        <dc:date rdf:datatype="http://www.w3.org/2001/XMLSchema#dateTime">2019-10-27T16:05:39Z</dc:date>
        <oboInOwl:inSubset>wwfBiome</oboInOwl:inSubset>
        <rdfs:label xml:lang="en">tropical mixed forest biome</rdfs:label>
    </owl:Class>
    


    <!-- http://purl.obolibrary.org/obo/ENVO_01001830 -->

    <owl:Class rdf:about="http://purl.obolibrary.org/obo/ENVO_01001830">
        <rdfs:subClassOf rdf:resource="http://purl.obolibrary.org/obo/ENVO_00000428"/>
        <obo:IAO_0000115>A biome which is subject to tropical climatic conditions.</obo:IAO_0000115>
        <dc:creator rdf:resource="https://orcid.org/0000-0002-4366-3088"/>
        <dc:date rdf:datatype="http://www.w3.org/2001/XMLSchema#dateTime">2019-11-06T15:56:17Z</dc:date>
        <rdfs:label xml:lang="en">tropical biome</rdfs:label>
    </owl:Class>
    


    <!-- http://purl.obolibrary.org/obo/ENVO_01001831 -->

    <owl:Class rdf:about="http://purl.obolibrary.org/obo/ENVO_01001831">
        <rdfs:subClassOf rdf:resource="http://purl.obolibrary.org/obo/ENVO_00000428"/>
        <obo:IAO_0000115>A biome which is subject to temperate climatic conditions.</obo:IAO_0000115>
        <dc:creator rdf:resource="https://orcid.org/0000-0002-4366-3088"/>
        <dc:date rdf:datatype="http://www.w3.org/2001/XMLSchema#dateTime">2019-11-06T15:57:04Z</dc:date>
        <rdfs:label xml:lang="en">temperate biome</rdfs:label>
    </owl:Class>
    


    <!-- http://purl.obolibrary.org/obo/ENVO_01001832 -->

    <owl:Class rdf:about="http://purl.obolibrary.org/obo/ENVO_01001832">
        <rdfs:subClassOf rdf:resource="http://purl.obolibrary.org/obo/ENVO_00000428"/>
        <obo:IAO_0000115>A biome which is subject to subtropical climatic conditions.</obo:IAO_0000115>
        <dc:creator rdf:resource="https://orcid.org/0000-0002-4366-3088"/>
        <dc:date rdf:datatype="http://www.w3.org/2001/XMLSchema#dateTime">2019-11-06T15:57:36Z</dc:date>
        <rdfs:label xml:lang="en">subtropical biome</rdfs:label>
    </owl:Class>
    


    <!-- http://purl.obolibrary.org/obo/ENVO_01001833 -->

    <owl:Class rdf:about="http://purl.obolibrary.org/obo/ENVO_01001833">
        <rdfs:subClassOf rdf:resource="http://purl.obolibrary.org/obo/ENVO_01001832"/>
        <obo:IAO_0000115>A biome which is subject to mediterranean climatic conditions.</obo:IAO_0000115>
        <dc:creator rdf:resource="https://orcid.org/0000-0002-4366-3088"/>
        <dc:date rdf:datatype="http://www.w3.org/2001/XMLSchema#dateTime">2019-11-06T15:58:10Z</dc:date>
        <rdfs:label xml:lang="en">mediterranean biome</rdfs:label>
    </owl:Class>
    


    <!-- http://purl.obolibrary.org/obo/ENVO_01001834 -->

    <owl:Class rdf:about="http://purl.obolibrary.org/obo/ENVO_01001834">
        <rdfs:subClassOf rdf:resource="http://purl.obolibrary.org/obo/ENVO_00000428"/>
        <obo:IAO_0000115>A biome which is subject to subpolar climatic conditions.</obo:IAO_0000115>
        <dc:creator rdf:resource="https://orcid.org/0000-0002-4366-3088"/>
        <dc:date rdf:datatype="http://www.w3.org/2001/XMLSchema#dateTime">2019-11-06T15:58:56Z</dc:date>
        <rdfs:label xml:lang="en">subpolar biome</rdfs:label>
    </owl:Class>
    


    <!-- http://purl.obolibrary.org/obo/ENVO_01001835 -->

    <owl:Class rdf:about="http://purl.obolibrary.org/obo/ENVO_01001835">
        <rdfs:subClassOf rdf:resource="http://purl.obolibrary.org/obo/ENVO_00000428"/>
        <obo:IAO_0000115>A biome which is subject to alpine altitudinal conditions.</obo:IAO_0000115>
        <dc:creator rdf:resource="https://orcid.org/0000-0002-4366-3088"/>
        <dc:date rdf:datatype="http://www.w3.org/2001/XMLSchema#dateTime">2019-11-06T15:59:35Z</dc:date>
        <rdfs:label xml:lang="en">alpine biome</rdfs:label>
    </owl:Class>
    


    <!-- http://purl.obolibrary.org/obo/ENVO_01001836 -->

    <owl:Class rdf:about="http://purl.obolibrary.org/obo/ENVO_01001836">
        <rdfs:subClassOf rdf:resource="http://purl.obolibrary.org/obo/ENVO_00000428"/>
        <obo:IAO_0000115>A biome which is subject to montane altitudinal conditions.</obo:IAO_0000115>
        <dc:creator rdf:resource="https://orcid.org/0000-0002-4366-3088"/>
        <dc:date rdf:datatype="http://www.w3.org/2001/XMLSchema#dateTime">2019-11-06T16:00:33Z</dc:date>
        <rdfs:label xml:lang="en">montane biome</rdfs:label>
    </owl:Class>
    


    <!-- http://purl.obolibrary.org/obo/ENVO_01001837 -->

    <owl:Class rdf:about="http://purl.obolibrary.org/obo/ENVO_01001837">
        <rdfs:subClassOf rdf:resource="http://purl.obolibrary.org/obo/ENVO_00000428"/>
        <obo:IAO_0000115>A biome which is subject to subapline altitudinal conditions.</obo:IAO_0000115>
        <dc:creator rdf:resource="https://orcid.org/0000-0002-4366-3088"/>
        <dc:date rdf:datatype="http://www.w3.org/2001/XMLSchema#dateTime">2019-11-06T16:01:49Z</dc:date>
        <rdfs:label xml:lang="en">subalpine biome</rdfs:label>
    </owl:Class>
    


    <!-- http://purl.obolibrary.org/obo/ENVO_01001838 -->

    <owl:Class rdf:about="http://purl.obolibrary.org/obo/ENVO_01001838">
        <rdfs:subClassOf rdf:resource="http://purl.obolibrary.org/obo/ENVO_00000428"/>
        <obo:IAO_0000115>A biome which is subject to arid environmental conditions.</obo:IAO_0000115>
        <dc:creator rdf:resource="https://orcid.org/0000-0002-4366-3088"/>
        <dc:date rdf:datatype="http://www.w3.org/2001/XMLSchema#dateTime">2019-11-06T16:06:47Z</dc:date>
        <rdfs:label xml:lang="en">arid biome</rdfs:label>
    </owl:Class>
    


    <!-- http://purl.obolibrary.org/obo/ENVO_03605008 -->

    <owl:Class rdf:about="http://purl.obolibrary.org/obo/ENVO_03605008">
        <rdfs:subClassOf rdf:resource="http://purl.obolibrary.org/obo/ENVO_00000873"/>
        <obo:IAO_0000115>A freshwater stream ecosystem which is undergoing climactic ecological succession.</obo:IAO_0000115>
        <dc:creator rdf:resource="https://orcid.org/0000-0001-9076-6066"/>
        <dc:date rdf:datatype="http://www.w3.org/2001/XMLSchema#dateTime">2024-01-10T19:19:00Z</dc:date>
        <rdfs:label xml:lang="en">freshwater stream biome</rdfs:label>
    </owl:Class>
</rdf:RDF>



<!-- Generated by the OWL API (version 4.5.29) https://github.com/owlcs/owlapi -->

