format-version: 1.2
ontology: pco

[Term]
id: PCO:0000000
name: collection of organisms
def: "A material entity that consists of two or more organisms, viruses, or viroids." []

[Term]
id: PCO:0000001
name: population
def: "A collection of organisms, all of the same species, that live in the same place." []
is_a: PCO:0000018  ! collection of organisms of the same species

[Term]
id: PCO:0000002
name: ecological community
def: "A collection of organisms of at least two different species, living in a particular area." []
is_a: PCO:0000000  ! collection of organisms

[Term]
id: PCO:0000017
name: species as a collection of organisms
def: "A collection of organisms that has as parts every organism of given species and no organisms of any other species." []
is_a: PCO:0000018  ! collection of organisms of the same species

[Term]
id: PCO:0000018
name: collection of organisms of the same species
def: "A material entity that has as parts two or more organisms, viruses, or viroids of the same species and no members of any other species." []
is_a: PCO:0000000  ! collection of organisms

[Term]
id: PCO:0000020
name: family
def: "A domestic group, or a number of domestic groups linked through descent (demonstrated or stipulated) from a common ancestor, marriage, or adoption." []
is_a: PCO:0000018  ! collection of organisms of the same species

[Term]
id: PCO:0000025
name: red population
is_a: PCO:0000000  ! collection of organisms

[Term]
id: PCO:0001000
name: pair of interacting organisms
is_a: PCO:0000000  ! collection of organisms

[Term]
id: PCO:0001001
name: pair of interacting organisms of the same species
is_a: PCO:0000018  ! collection of organisms of the same species
is_a: PCO:0001000  ! pair of interacting organisms

