format-version: 1.2
data-version: envo/releases/2025-08-19/subsets/biome-hierarchy.owl
ontology: envo/subsets/biome-hierarchy
property_value: owl:versionInfo "subsets/biome-hierarchy.owl 2025-08-19" xsd:string

[Term]
id: ENVO:00000428
name: biome
def: "A biome is an ecosystem which is undergoing climactic ecological succession." [DOI:10.1186/2041-1480-4-43, https://en.wikipedia.org/wiki/Biome]
comment: In this definition, there is an assumption that no major perturbations are occurring or have occurred in a time frame affects the successional dynamics of the ecosystem. A "major" perturbation is one which disrupts the community's ability to restore its (near) equilibrium. Usually, pioneer or early secondary successional processes would be in effect in such scenarios.
synonym: "EcosytemType" RELATED [NASA:earthrealm]
synonym: "major habitat type" EXACT [WWF:Biome]
xref: EcoLexicon:biome
xref: LTER:809 {xref="https://vocab.lternet.edu/vocab/vocab/index.php?tema=809&/biomes"}

[Term]
id: ENVO:00000446
name: terrestrial biome
def: "A biome which is  primarily or completely situated on a landmass." [https://en.wikipedia.org/wiki/Biome#Terrestrial_biomes]
synonym: "terrestrial realm" RELATED []
xref: LTER:798
xref: SPIRE:Terrestrial
is_a: ENVO:00000428 ! biome

[Term]
id: ENVO:00000447
name: marine biome
def: "An aquatic biome which is determined by a marine water body." [https://en.wikipedia.org/wiki/Ocean, https://orcid.org/0000-0002-4366-3088, ISBN:978-0-618-45504-1, MA:ma]
comment: This biome includes open-ocean and unprotected coastal ecosystems, characterized by exposure to wave action, tidal fluctuation, and ocean currents as well as systems that largely resemble these. Water in the marine biome is generally within the salinity range of seawater: 30 to 38 ppt.
subset: envoPolar
synonym: "marine realm" RELATED []
xref: SPIRE:Marine
is_a: ENVO:00002030 ! aquatic biome

[Term]
id: ENVO:00000873
name: freshwater biome
def: "An aquatic biome which is determined by a body of freshwater." [https://orcid.org/0000-0002-4366-3088, MA:ma]
subset: envoPolar
synonym: "freshwater realm" RELATED []
xref: SPIRE:Freshwater
is_a: ENVO:00002030 ! aquatic biome

[Term]
id: ENVO:00000887
name: large river biome
def: "A freshwater river biome which is determined by a large river." []
comment: "Large" is ambiguous. For details on "Large rivers" (e.g. the Mekong river) see http://worldwildlife.org/biomes/large-river-ecosystems This class will be replaced with a less ambiguous class.
subset: wwfBiome
is_a: ENVO:01000253 ! freshwater river biome

[Term]
id: ENVO:00000888
name: large river headwater biome
def: "A freshwater river biome which is determined by the headwaters of a large river." []
comment: "Large" is ambiguous. For details on "Large river headwaters" (e.g. the Upper Amazon headwaters) see http://worldwildlife.org/biomes/large-river-headwater-ecosystems This class will be replaced with a less ambiguous class.
subset: wwfBiome
is_a: ENVO:01000253 ! freshwater river biome

[Term]
id: ENVO:00000889
name: large river delta biome
def: "A freshwater river biome which is determined by the delta of a large river." []
comment: "Large" is ambiguous. For details on "Large river deltas" (e.g. the Niger river delta) see http://worldwildlife.org/biomes/large-river-delta-ecosystems This class will be replaced with a less ambiguous class.
subset: wwfBiome
is_a: ENVO:01000253 ! freshwater river biome

[Term]
id: ENVO:00000890
name: small river biome
def: "A freshwater river biome which is determined by a small river." []
comment: "Small" is ambiguous. For details on "Small rivers" (e.g. the Salween river) see http://worldwildlife.org/biomes/small-river-ecosystems. This class will be replaced with a less ambiguous class.
subset: wwfBiome
is_a: ENVO:01000253 ! freshwater river biome

[Term]
id: ENVO:00000891
name: large freshwater lake biome
def: "A freshwater biome which is determined by a large lake." []
comment: "Large" is ambiguous. For details on "Large lakes" (e.g. African rift lakes) see http://worldwildlife.org/biomes/large-lake-ecosystems This class will be replaced with a less ambiguous class.
subset: wwfBiome
is_a: ENVO:01000252 ! freshwater lake biome

[Term]
id: ENVO:00000892
name: small freshwater lake biome
def: "A freshwater lake biome which is determined by a small lake." []
comment: "Small" is ambiguous. For details on "Small lakes" (e.g. Cameroon crater lakes)  see http://worldwildlife.org/biomes/small-lake-ecosystems. This class will be replaced with a less ambiguous class.
subset: wwfBiome
is_a: ENVO:01000252 ! freshwater lake biome

[Term]
id: ENVO:00000893
name: xeric basin biome
def: "A biome which has little permanent surface water and a low relative abundance of springs." [https://www.worldwildlife.org/biomes/xeric-basin-ecosystems]
subset: wwfBiome
is_a: ENVO:00000873 ! freshwater biome
property_value: IAO:0000116 "The WWF definition is somewhat ambiguous, but workable." xsd:string

[Term]
id: ENVO:00002030
name: aquatic biome
def: "A biome which is determined by a water body and which has ecological climax communities adapted to life in or on water." []
xref: LTER:41
is_a: ENVO:00000428 ! biome

[Term]
id: ENVO:01000004
name: concentration basin mediterranean sea biome
def: "The concentration basin mediterranean sea biome comprises expressions of the mediterranean sea biome that have higher salinity than bordering oceans due to evaporation. Water exchange consists of inflow of the fresher oceanic water in the upper layer and outflow of the saltier mediterranean water in the lower layer of the connecting channel." [https://en.wikipedia.org/wiki/Mediterranean_sea, ORCID:0000-0002-4366-3088]
is_a: ENVO:01000047 ! mediterranean sea biome
created_by: ORCID:0000-0002-4366-3088
creation_date: 2010-03-19T09:32:59Z

[Term]
id: ENVO:01000020
name: estuarine biome
def: "Expressions of the estuarine biome occur at wide lower courses of a rivers where they flow into a sea. Estuaries experience tidal flows and their water is a changing mixture of fresh and salt." [ISBN:978-92-1-161386-5, ORCID:0000-0002-4366-3088]
xref: SPIRE:Estuarine
is_a: ENVO:00000447 ! marine biome
created_by: ORCID:0000-0002-4366-3088
creation_date: 2010-03-15T11:17:06Z

[Term]
id: ENVO:01000022
name: marine salt marsh biome
namespace: ENVO
def: "The marine salt marsh biome comprises marshes that are transitional intertidals between land and salty or brackish marine water (e.g.: sloughs, bays, estuaries). It is dominated by halophytic (salt tolerant) herbaceous plants. The daily tidal surges bring in nutrients, which tend to settle in roots of the plants within the salt marsh. The natural chemical activity of salty (or brackish) water and the tendency of algae to bloom in the shallow unshaded water also allow for great biodiversity." [https://en.wikipedia.org/wiki/Salt_marsh, ORCID:0000-0002-4366-3088]
is_a: ENVO:00000447 ! marine biome
created_by: ORCID:0000-0002-4366-3088
creation_date: 2010-03-15T11:17:06Z

[Term]
id: ENVO:01000023
name: marine pelagic biome
namespace: ENVO
def: "The marine pelagic biome (pelagic meaning open sea) is that of the marine water column, from the surface to the greatest depths." [ISBN:978-0-7506-3384-0]
subset: envoPolar
is_a: ENVO:00000447 ! marine biome
created_by: ORCID:0000-0002-4366-3088
creation_date: 2010-03-15T11:17:06Z

[Term]
id: ENVO:01000024
name: marine benthic biome
def: "The marine benthic biome (benthic meaning 'bottom') encompasses the seafloor and includes such areas as shores, littoral or intertidal areas, marine coral reefs, and the deep seabed." [ISBN:978-0-7506-3384-0, ORCID:0000-0002-4366-3088]
subset: envoPolar
xref: SPIRE:Benthic
is_a: ENVO:00000447 ! marine biome
created_by: ORCID:0000-0002-4366-3088
creation_date: 2010-03-15T11:17:06Z

[Term]
id: ENVO:01000025
name: marine neritic benthic zone biome
def: "The marine neritic zone biome comprises sea floor from the high tide mark to a continental shelf break. This zone generally extends to 200 m below average sea level." [ISBN:978-0-444-82619-0, ISBN:978-0-7506-3384-0, ORCID:0000-0002-4366-3088]
subset: envoPolar
is_a: ENVO:01000024 ! marine benthic biome
created_by: ORCID:0000-0002-4366-3088
creation_date: 2010-03-15T11:18:40Z

[Term]
id: ENVO:01000026
name: marine bathyal zone biome
def: "The marine bathyal zone biome comprises regions of the marine benthic biome between approximately 200 m and 3000 m depth. This zone generally coincides with the continental slope." [ISBN:978-0-444-82619-0, ORCID:0000-0002-4366-3088]
is_a: ENVO:01000024 ! marine benthic biome
created_by: ORCID:0000-0002-4366-3088
creation_date: 2010-03-15T11:18:40Z

[Term]
id: ENVO:01000027
name: marine abyssal zone biome
def: "The marine abyssal zone biome comprises regions of the marine benthic biome  between approximately 2500 m and 6000 m depth. This zone generally coincides with the continental rise and the abyssal plain." [ISBN:978-0-444-82619-0, ORCID:0000-0002-4366-3088]
is_a: ENVO:01000024 ! marine benthic biome
created_by: ORCID:0000-0002-4366-3088
creation_date: 2010-03-15T11:18:40Z

[Term]
id: ENVO:01000028
name: marine hadal zone biome
def: "The marine hadal zone biome describes sea floor deeper than 6000 m such as that of the oceanic trenches." [ISBN:978-0-444-82619-0, ORCID:0000-0002-4366-3088]
is_a: ENVO:01000024 ! marine benthic biome
created_by: ORCID:0000-0002-4366-3088
creation_date: 2010-03-15T11:18:40Z

[Term]
id: ENVO:01000029
name: marine reef biome
def: "A biome expressed by strips or ridges of rocks, sand, or coral that rises to or near the surface of a body of marine water." [ISBN:978-0-618-45504-1, ORCID:0000-0002-4366-3088]
is_a: ENVO:01000024 ! marine benthic biome
created_by: ORCID:0000-0002-4366-3088
creation_date: 2010-03-15T11:18:40Z

[Term]
id: ENVO:01000030
name: marine hydrothermal vent biome
def: "The marine hydrothermal vent biome comprises regions of the marine benthic biome where heat generated due to tectonic activity, either at divergent plate boundaries or convergent ocean plates where back-arc spreading occurs, is released or 'vented' to the surface. The resultant high temperature water jets are laden with dissolved metals and minerals." [ISBN:978-0-444-82619-0, ORCID:0000-0002-4366-3088]
is_a: ENVO:01000024 ! marine benthic biome
created_by: ORCID:0000-0002-4366-3088
creation_date: 2010-03-15T11:18:40Z

[Term]
id: ENVO:01000032
name: neritic pelagic zone biome
namespace: ENVO
def: "The neritic epipelagic zone biome comprises the marine water column above a continental shelf." [ISBN:978-0-444-82619-0, ISBN:978-0-7506-3384-0, ORCID:0000-0002-4366-3088]
is_a: ENVO:01000023 ! marine pelagic biome
disjoint_from: ENVO:01000033 ! oceanic pelagic zone biome
created_by: ORCID:0000-0002-4366-3088
creation_date: 2010-03-15T11:19:19Z

[Term]
id: ENVO:01000033
name: oceanic pelagic zone biome
namespace: ENVO
def: "The oceanic epipelagic zone biome comprises the marine water column offshore, beyond a continental shelf." [ISBN:978-0-444-82619-0, ISBN:978-0-7506-3384-0, ORCID:0000-0002-4366-3088]
is_a: ENVO:01000023 ! marine pelagic biome
created_by: ORCID:0000-0002-4366-3088
creation_date: 2010-03-15T11:19:19Z

[Term]
id: ENVO:01000034
name: oceanic sea surface microlayer biome
namespace: ENVO
def: "The oceanic sea surface microlayer (SML) biome comprises the top 1000 micrometers of the marine surface waters occurring offshore, away from a continental shelf. It is the boundary layer where all exchange occurs between the atmosphere and the ocean. The chemical, physical, and biological properties of the SML differ greatly from the sub-surface water just a few centimeters beneath." [https://en.wikipedia.org/wiki/Sea_surface_microlayer, ORCID:0000-0002-4366-3088]
is_a: ENVO:01000033 ! oceanic pelagic zone biome
created_by: ORCID:0000-0002-4366-3088
creation_date: 2010-03-15T11:21:03Z

[Term]
id: ENVO:01000035
name: oceanic epipelagic zone biome
namespace: ENVO
def: "The oceanic epipelagic zone biome comprises regions of the marine water column that occur offshore, beyond a continental shelf. This biome extends from the surface of the ocean to a depth of ca. 200-250m. Throughout the zone the light field tends to be asymmetrical vertically, so that the direction and elevation of the sun can still be detected. The oceanic epipelagic zone biome encompasses the euphotic zone and, where and when it occurs, the seasonal thermocline." [ISBN:978-0-444-82619-0, ORCID:0000-0002-4366-3088]
is_a: ENVO:01000033 ! oceanic pelagic zone biome
created_by: ORCID:0000-0002-4366-3088
creation_date: 2010-03-15T11:21:03Z

[Term]
id: ENVO:01000036
name: oceanic mesopelagic zone biome
namespace: ENVO
def: "The oceanic mesopelagic zone biome comprises regions of the marine water column that occur offshore, beyond a continental shelf. This biome extends through the water column from approximately 200-1000 m depth - the maximal depth of light penetration in all but the clearest oligotrophic ocean regions. In comparison to the epipelagic zone, dominant forms of pelagic organisms do not change very much; however, there are marked changes in species composition and the proportion of smaller-sized individuals decreases." [ISBN:978-0-444-82619-0, ORCID:0000-0002-4366-3088]
is_a: ENVO:01000033 ! oceanic pelagic zone biome
created_by: ORCID:0000-0002-4366-3088
creation_date: 2010-03-15T11:21:03Z

[Term]
id: ENVO:01000037
name: oceanic bathypelagic zone biome
namespace: ENVO
def: "The bathypelagic zone biome comprises the marine water column below approximately 1000 m water depth - the maximum depth to which detectable daylight penetrates in all but the clearest oligotrophic waters - and extends to about 2500 - 2700 m water depth. In the temperate Atlantic, the beginning of the bathypelagic zone biome approximates to the deep oxygen minimum and the base of the permanent thermocline." [ISBN:978-0-444-82619-0, ORCID:0000-0002-4366-3088]
is_a: ENVO:01000033 ! oceanic pelagic zone biome
created_by: ORCID:0000-0002-4366-3088
creation_date: 2010-03-15T11:21:03Z

[Term]
id: ENVO:01000038
name: oceanic abyssopelagic zone biome
namespace: ENVO
def: "The abyssopelagic zone biome comprises the marine water column below the bathypelagic zone biome at approximately 2500 -2700 m and extends either to the hadal pelagic zone biome (at approximately 6000 m) or to the benthopelagic zone biome within ca. 100 m of the seafloor. The depth of 2700 m may be critical for physiological reasons as the change in hydrostatic pressure across this depth may preclude organism migration." [ISBN:978-0-444-82619-0, ORCID:0000-0002-4366-3088]
is_a: ENVO:01000033 ! oceanic pelagic zone biome
created_by: ORCID:0000-0002-4366-3088
creation_date: 2010-03-15T11:21:03Z

[Term]
id: ENVO:01000039
name: oceanic hadal pelagic zone biome
namespace: ENVO
def: "The oceanic hadal pelagic zone biome comprises the water column in oceanic trenches occurring at depths between 6000m and 10,000m." [ISBN:978-0-444-82619-0, ORCID:0000-0002-4366-3088]
is_a: ENVO:01000033 ! oceanic pelagic zone biome
created_by: ORCID:0000-0002-4366-3088
creation_date: 2010-03-15T11:21:03Z

[Term]
id: ENVO:01000040
name: oceanic benthopelagic zone biome
namespace: ENVO
def: "The benthopelagic zone biome comprises regions of the marine water column which usually coincide with the benthic boundary layer (BBL) - the layer of isothermal and isohaline water contiguous to the sea floor. A general reversal in the declining gradient of pelagic biomass may be observed here, perhaps explained by viable nutrition on the sea floor being resuspended by bottom currents. This zone typically extends 100 m above the seafloor, but may reach upto1000 m during benthic storms." [ISBN:978-0-444-82619-0, ORCID:0000-0002-4366-3088]
is_a: ENVO:01000033 ! oceanic pelagic zone biome
created_by: ORCID:0000-0002-4366-3088
creation_date: 2010-03-15T11:21:03Z

[Term]
id: ENVO:01000041
name: neritic sea surface microlayer biome
namespace: ENVO
def: "The neritic sea surface microlayer (SML) biome comprises the top 1000 micrometers of marine surface waters occurring above a continental shelf. It is the boundary layer where all exchange occurs between the atmosphere and the ocean. The chemical, physical, and biological properties of the SML differ greatly from the sub-surface water just a few centimeters beneath." [https://en.wikipedia.org/wiki/Sea_surface_microlayer, ORCID:0000-0002-4366-3088]
is_a: ENVO:01000032 ! neritic pelagic zone biome
created_by: ORCID:0000-0002-4366-3088
creation_date: 2010-03-15T11:22:09Z

[Term]
id: ENVO:01000042
name: neritic epipelagic zone biome
namespace: ENVO
def: "The neritic epipelagic zone biome comprises the marine water column that occurs above a continental shelf and extends from the surface of the ocean to a depth of ca. 200-250m. Throughout the zone the light field tends to be asymmetrical vertically, so that the direction and elevation of the sun can still be detected. The epipelagic zone encompasses the euphotic zone and, where and when it occurs, the seasonal thermocline." [ISBN:978-0-444-82619-0, ORCID:0000-0002-4366-3088]
is_a: ENVO:01000032 ! neritic pelagic zone biome
created_by: ORCID:0000-0002-4366-3088
creation_date: 2010-03-15T11:22:09Z

[Term]
id: ENVO:01000043
name: neritic mesopelagic zone biome
def: "The neritic mesopelagic zone biome comprises the marine column that occurs above a continental shelf and extends from approximately 200 to 1000 m depth - the maximal depth of light penetration in all but the clearest oligotrophic ocean regions. In comparison to the epipelagic zone, dominant forms of pelagic organisms do not change very much; however, there are marked changes in species composition and the proportion of smaller-sized individuals decreases." [ISBN:978-0-444-82619-0, ORCID:0000-0002-4366-3088]
is_a: ENVO:01000032 ! neritic pelagic zone biome
created_by: ORCID:0000-0002-4366-3088
creation_date: 2010-03-15T11:22:09Z

[Term]
id: ENVO:01000045
name: epeiric sea biome
def: "The epeiric sea (also known as an epicontinental sea) biome comprises a shallow seas that extend over part of a continent. Epeiric seas are usually associated with the marine transgressions of the geologic  past, which have variously been due to either global eustatic sea level changes, local tectonic deformation, or both, and are occasionally semi-cyclic." [https://en.wikipedia.org/wiki/Epeiric_sea, ORCID:0000-0002-4366-3088]
synonym: "epicontinental sea biome" EXACT [https://en.wikipedia.org/wiki/Epeiric_sea]
is_a: ENVO:00000447 ! marine biome
created_by: ORCID:0000-0002-4366-3088
creation_date: 2010-03-15T11:23:23Z

[Term]
id: ENVO:01000046
name: marginal sea biome
def: "The marginal sea biome comprises parts of an ocean partially enclosed by land such as islands, archipelagos, or peninsulas. Unlike mediterranean seas, marginal seas have ocean currents caused by ocean winds. Many marginal seas are enclosed by island arcs that were formed from the subduction of one oceanic plate beneath another." [https://en.wikipedia.org/wiki/Marginal_sea, ORCID:0000-0002-4366-3088]
is_a: ENVO:00000447 ! marine biome
created_by: ORCID:0000-0002-4366-3088
creation_date: 2010-03-15T11:23:23Z

[Term]
id: ENVO:01000047
name: mediterranean sea biome
def: "The mediterranean sea biome comprises mostly enclosed seas that have limited exchange of deep water with outer oceans and where the water circulation is dominated by salinity and temperature differences rather than winds." [https://en.wikipedia.org/wiki/Mediterranean_sea, ORCID:0000-0002-4366-3088]
is_a: ENVO:00000447 ! marine biome
is_a: ENVO:01001833 ! mediterranean biome
created_by: ORCID:0000-0002-4366-3088
creation_date: 2010-03-15T11:23:23Z

[Term]
id: ENVO:01000048
name: ocean biome
def: "A marine biome which is determined by an ocean." [https://en.wikipedia.org/wiki/Ocean, ORCID:0000-0002-4366-3088]
comment: Ocean biomes are determined by major bodies of saline water, principal components of the hydrosphere. Approximately 71% of the Earth's surface is covered by ocean, a continuous body of water that is customarily divided into several principal oceans and smaller seas. More than half of this area is over 3,000 metres (9,800 ft) deep. Average oceanic salinity is around 35 parts per thousand (ppt) (3.5%), and nearly all seawater has a salinity in the range of 30 to 38 ppt.
subset: envoPolar
is_a: ENVO:00000447 ! marine biome
created_by: ORCID:0000-0002-4366-3088
creation_date: 2010-03-15T11:23:23Z

[Term]
id: ENVO:01000049
name: marine coral reef biome
namespace: ENVO
def: "The marine coral reef biome comprises constructional wave-resistant entities which are primarily built by corals and are often cemented together. The growth of these structures is aided by zooxanthellae, algae that are symbiotic with the reef-building corals." [ISBN:978-0-7506-3384-0, ORCID:0000-0002-4366-3088]
is_a: ENVO:01000029 ! marine reef biome
created_by: ORCID:0000-0002-4366-3088
creation_date: 2010-03-15T11:27:06Z

[Term]
id: ENVO:01000050
name: marine subtidal rocky reef biome
namespace: ENVO
def: "The marine rocky subtidal reef biome comprises regions of the marine reef biome composed mainly of rock and which harbour abundant communities of algae and invertebrates. These reefs are often very patchy, with alterations of rocks dominated by rich invertebrate assemblages and turf-forming calcareous red algae." [ISBN:978-0-7506-3384-0, ORCID:0000-0002-4366-3088]
is_a: ENVO:01000029 ! marine reef biome
created_by: ORCID:0000-0002-4366-3088
creation_date: 2010-03-15T11:27:06Z

[Term]
id: ENVO:01000051
name: marine black smoker biome
namespace: ENVO
def: "A marine black smoker biome comprises regions of the marine hydrothermal vent biome characterised by a black vent plume. This black plume is a consequence of dissolved metals and minerals forming complexes with sulphide and indicates polymetallic sulphide mineral deposits beneath the surface." [ISBN:978-0-444-82619-0, ORCID:0000-0002-4366-3088]
is_a: ENVO:01000030 ! marine hydrothermal vent biome
created_by: ORCID:0000-0002-4366-3088
creation_date: 2010-03-15T11:29:37Z

[Term]
id: ENVO:01000052
name: marine white smoker biome
namespace: ENVO
def: "A marine white smoker biome comprises regions of the marine hydrothermal vent biome characterised by lightly hued plumes, typically containing barium, calcium, and silicon. These vents tend to have lower temperature plumes when compared to black smoker environments." [https://en.wikipedia.org/wiki/Hydrothermal_vent, ORCID:0000-0002-4366-3088]
is_a: ENVO:01000030 ! marine hydrothermal vent biome
created_by: ORCID:0000-0002-4366-3088
creation_date: 2010-03-15T11:29:37Z

[Term]
id: ENVO:01000053
name: marine ultramafic hydrothermal vent biome
namespace: ENVO
def: "A marine ultramafic hydrothermal vent biome comprises regions of themarine  hydrothermal vent biome hosted on ultramafic (also referred to as ultrabasic) rocks. Ultramafic rocks are igneous and meta-igneous rocks with very low silica content (less than 45%), generally >18% MgO, high FeO, low potassium, and are composed of usually greater than 90% mafic minerals  (dark colored, high magnesium and iron content). The Earth's mantle is composed of ultramafic rocks." [https://en.wikipedia.org/wiki/Ultramafic, ISBN:978-0-444-82619-0, ORCID:0000-0002-4366-3088]
is_a: ENVO:01000030 ! marine hydrothermal vent biome
created_by: ORCID:0000-0002-4366-3088
creation_date: 2010-03-15T11:29:37Z

[Term]
id: ENVO:01000054
name: marine basaltic hydrothermal vent biome
namespace: ENVO
def: "A marine basaltic hydrothermal vent biome comprises regions of the marine hydrothermal vent biome hosted on basaltic rocks. Basalt generally has a composition of 45 to 55 wt % SiO2, 2 to 6 wt % total alkalis, 0.5 to 2.0 wt % TiO2, 5 to 14 wt % FeO and 14 wt % or more Al2O3. Contents of CaO are commonly near 10 wt %, those of MgO commonly in the range 5 to 12 wt %." [https://en.wikipedia.org/wiki/Basalt, ISBN:978-0-444-82619-0, ORCID:0000-0002-4366-3088]
is_a: ENVO:01000030 ! marine hydrothermal vent biome
created_by: ORCID:0000-0002-4366-3088
creation_date: 2010-03-15T11:29:37Z

[Term]
id: ENVO:01000123
name: marine sponge reef biome
namespace: ENVO
def: "The marine sponge reef biome comprises marine reefs primarily built by marine sponges. The primary frame-building sponges are all members of the order Hexactinosa. They are found only in glacier-scoured troughs of low-angle continental shelf. The seafloor is stable and consists of rock, coarse gravel, and large boulders." [https://en.wikipedia.org/wiki/Sponge_reef, ORCID:0000-0002-4366-3088]
is_a: ENVO:01000029 ! marine reef biome
created_by: ORCID:0000-0002-4366-3088
creation_date: 2010-03-17T04:43:05Z

[Term]
id: ENVO:01000127
name: marine cold seep biome
def: "A marine benthic biome which is determined by a cold seep." [https://en.wikipedia.org/wiki/Cold_seep, https://orcid.org/0000-0002-4366-3088]
comment: The marine cold seep biome comprises regions of the marine benthic biome where seepage of methane, hydrogen sulphide, hydrocarbon rich fluids and other fluids occurs.
is_a: ENVO:01000024 ! marine benthic biome
created_by: https://orcid.org/0000-0002-4366-3088
creation_date: 2010-03-19T08:33:56Z

[Term]
id: ENVO:01000128
name: dilution basin mediterranean sea biome
def: "The dilution basin mediterranean sea biome comprises expressions of the mediterranean sea biome with lower salinity than the surrounding ocean due to freshwater gains such as rainfall and rivers. Water exchange consists of outflow of the fresher mediterranean water in the upper layer and inflow of the saltier oceanic water in the lower layer of the channel. Renewal of deep water may not be sufficient to supply oxygen to the bottom." [https://en.wikipedia.org/wiki/Mediterranean_sea, ORCID:0000-0002-4366-3088]
is_a: ENVO:01000047 ! mediterranean sea biome
created_by: ORCID:0000-0002-4366-3088
creation_date: 2010-03-19T09:32:59Z

[Term]
id: ENVO:01000174
name: forest biome
def: "A forest ecosystem which is undergoing climactic ecological succession." []
xref: LTER:212
xref: SPIRE:Forest
is_a: ENVO:00000446 ! terrestrial biome
created_by: ORCID:0000-0002-4366-3088
creation_date: 2013-04-07T14:26:46Z

[Term]
id: ENVO:01000175
name: woodland biome
def: "A woodland biome is a terrestrial biome which includes, across its entire spatial extent, woody plants spaced sufficiently far apart to allow light penetration to support communities of herbaceous plants or shrubs living closer to the woodland floor." []
comment: Preliminary definition.
is_a: ENVO:00000446 ! terrestrial biome
created_by: ORCID:0000-0002-4366-3088
creation_date: 2013-04-07T14:26:46Z

[Term]
id: ENVO:01000176
name: shrubland biome
def: "A shrubland biome is a terrestrial biome which includes, across its entire spatial extent, dense groups of shrubs." []
comment: Preliminary definition.
is_a: ENVO:00000446 ! terrestrial biome
created_by: ORCID:0000-0002-4366-3088
creation_date: 2013-04-07T14:26:46Z

[Term]
id: ENVO:01000177
name: grassland biome
def: "A grassland ecosystem in which dominant ecological communities have reached their climax successional state." []
xref: SPIRE:Savannah_or_grassland
is_a: ENVO:00000446 ! terrestrial biome
created_by: ORCID:0000-0002-4366-3088
creation_date: 2013-04-07T14:26:46Z

[Term]
id: ENVO:01000178
name: savanna biome
def: "A woodland biome which has seasonal water availability and includes trees spaced sufficiently far apart to allow an unbroken layer of grass, sedge (Cyperaceae) or  rush (Juncaceae) communities to live." []
xref: SPIRE:Savannah_or_grassland
is_a: ENVO:01000175 ! woodland biome
created_by: ORCID:0000-0002-4366-3088
creation_date: 2013-04-07T14:26:46Z

[Term]
id: ENVO:01000179
name: desert biome
def: "A desert ecosystem which is undergoing climactic ecological succession." []
subset: wwfBiome
xref: SPIRE:Desert_or_dune
is_a: ENVO:00000428 ! biome
created_by: ORCID:0000-0002-4366-3088
creation_date: 2013-04-07T14:26:46Z

[Term]
id: ENVO:01000180
name: tundra biome
def: "A tundra ecosystem which is undergoing climactic ecological succession." []
subset: envoPolar
subset: wwfBiome
xref: SPIRE:Tundra
is_a: ENVO:00000446 ! terrestrial biome
created_by: ORCID:0000-0002-4366-3088
creation_date: 2013-04-07T14:26:46Z

[Term]
id: ENVO:01000181
name: mangrove biome
def: "A mangrove biome is a terrestrial biome which includes, across its spatial extent, mangrove plants (Rhizophoraceae). Mangrove plants are able to withstand high levels of salinity as well as regions of anoxia and frequent tidal inundation. Mangrove biomes often occur near tropical and sub-tropical estuaries and depositional marine coastal environments where fine sediments (often with high organic content) collect in areas protected from high energy wave action." [https://en.wikipedia.org/wiki/Mangrove, ORCID:0000-0002-4366-3088]
comment: Preliminary definition. Depending on whether mangrove trees or shrubs are present, this class could be a child of shrubland biome or woodland biome. Consider creating the appropriate classes.
subset: wwfBiome
xref: LTER:322
is_a: ENVO:00000446 ! terrestrial biome
created_by: ORCID:0000-0002-4366-3088
creation_date: 2013-04-07T14:26:46Z

[Term]
id: ENVO:01000182
name: temperate desert biome
def: "A temperate desert biome is a desert biome which has communities adapted to intermediate insolation, low rainfall, and large temperature variations between winter and summer. Winter temperatures may fall below 0 degrees Celsius. Some precipitation in this biome may fall as snow." [WWW:http\://www.fs.fed.us/land/ecosysmgmt/colorimagemap/images/340.html]
comment: Preliminary definition. The semantics and definitions of "mediterranean", "subtropical", "tropical", "temperate", "polar", and similar climate types may be transferred to an "environmental condition" class once the semantics of this class have been established.
is_a: ENVO:01000179 ! desert biome
is_a: ENVO:01001831 ! temperate biome
created_by: ORCID:0000-0002-4366-3088
creation_date: 2013-04-07T14:28:08Z

[Term]
id: ENVO:01000183
name: tropical desert biome
def: "A tropical desert biome is a desert biome which has communities adapted to temperatures above a monthly average of 18 degrees Celsius, high daily temperature ranges of approximately 20 degrees Celsius, very high insolation due to inhibited cloud formation, and very low precipitation. Tropical desert biomes located near coasts with cold upwellings may have cooler temperatures and reduced insolution due to fog." [WWW:http\://www.earthonlinemedia.com/ebooks/tpe_3e/title_page.html]
comment: Preliminary definition. The semantics and definitions of "mediterranean", "subtropical", "tropical", "temperate", "polar", and similar climate types may be transferred to an "environmental condition" class once the semantics of this class have been established.
is_a: ENVO:01000179 ! desert biome
is_a: ENVO:01001830 ! tropical biome
created_by: ORCID:0000-0002-4366-3088
creation_date: 2013-04-07T14:28:08Z

[Term]
id: ENVO:01000184
name: subtropical desert biome
def: "A subtropical desert biome is a desert biome which has communities adapted to temperatures above a monthly average of 18 degrees Celsius, high daily temperature ranges of approximately 20 degrees Celsius, high insolation (but lower than that of a tropical desert biome), inhibited cloud formation, and very low precipitation. Subtropical desert biomes located near coasts with cold upwellings may have cooler temperatures and reduced insolution due to fog." [https://en.wikipedia.org/wiki/Subtropical#Semi-desert.2Fdesert_climate, WWW:http\://www.earthonlinemedia.com/ebooks/tpe_3e/title_page.html]
comment: Preliminary definition. The semantics and definitions of "mediterranean", "subtropical", "tropical", "temperate", "polar", and similar climate types may be transferred to an "environmental condition" class once the semantics of this class have been established.
is_a: ENVO:01000179 ! desert biome
is_a: ENVO:01001832 ! subtropical biome
created_by: ORCID:0000-0002-4366-3088
creation_date: 2013-04-07T14:28:08Z

[Term]
id: ENVO:01000185
name: montane desert biome
def: "A montane desert biome is a desert biome which occurs in regions elevated above sea level and which has community structure determined by elevation-dependent environmental conditions." []
comment: Preliminary definition.
is_a: ENVO:01000179 ! desert biome
is_a: ENVO:01001836 ! montane biome
created_by: ORCID:0000-0002-4366-3088
creation_date: 2013-04-07T14:28:08Z

[Term]
id: ENVO:01000186
name: polar desert biome
def: "A polar desert biome is a desert biome which is subject to low levels of insolation, annual precipitation less than 250 millimeters, and a mean temperature less than 10 degrees Celsius during its warmest month. Temperature changes in polar deserts frequently cross the freezing point of water." [https://en.wikipedia.org/wiki/Polar_desert]
comment: Preliminary definition. The semantics and definitions of "mediterranean", "subtropical", "tropical", "temperate", "polar", and similar climate types may be transferred to an "environmental condition" class once the semantics of this class have been established.
subset: envoPolar
is_a: ENVO:01000179 ! desert biome
is_a: ENVO:01000339 ! polar biome
created_by: ORCID:0000-0002-4366-3088
creation_date: 2013-04-07T14:28:08Z

[Term]
id: ENVO:01000187
name: subtropical savanna biome
def: "A savanna biome which is subject to subtropical climate patterns." []
comment: Preliminary definition. The semantics and definitions of "mediterranean", "subtropical", "tropical", "temperate", "polar", and similar climate types may be transferred to an "environmental condition" class once the semantics of this class have been established.
subset: wwfBiome
is_a: ENVO:01000178 ! savanna biome
is_a: ENVO:01001832 ! subtropical biome
created_by: ORCID:0000-0002-4366-3088
creation_date: 2013-04-07T14:28:51Z

[Term]
id: ENVO:01000188
name: tropical savanna biome
def: "A savanna biome which is subject to tropical climate patterns." []
comment: Preliminary definition. The semantics and definitions of "mediterranean", "subtropical", "tropical", "temperate", "polar", and similar climate types may be transferred to an "environmental condition" class once the semantics of this class have been established.
subset: wwfBiome
is_a: ENVO:01000178 ! savanna biome
is_a: ENVO:01001830 ! tropical biome
created_by: ORCID:0000-0002-4366-3088
creation_date: 2013-04-07T14:28:51Z

[Term]
id: ENVO:01000189
name: temperate savanna biome
def: "A savanna biome which is subject to temperate climate patterns." []
comment: Preliminary definition. The semantics and definitions of "mediterranean", "subtropical", "tropical", "temperate", "polar", and similar climate types may be transferred to an "environmental condition" class once the semantics of this class have been established.
synonym: "prairie biome" BROAD []
is_a: ENVO:01000178 ! savanna biome
is_a: ENVO:01001831 ! temperate biome
created_by: ORCID:0000-0002-4366-3088
creation_date: 2013-04-07T14:28:51Z

[Term]
id: ENVO:01000190
name: flooded savanna biome
def: "A flooded savanna biome is a savanna biome which has very wet to saturated soil moisture content." [https://en.wikipedia.org/wiki/Flooded_grasslands_and_savannas]
subset: wwfBiome
synonym: "marsh" RELATED []
synonym: "swamp" BROAD []
is_a: ENVO:01000178 ! savanna biome
created_by: ORCID:0000-0002-4366-3088
creation_date: 2013-04-07T14:28:51Z

[Term]
id: ENVO:01000191
name: subtropical grassland biome
def: "A subtropical grassland in which dominant ecological communities have reached their climax successional state." []
subset: wwfBiome
is_a: ENVO:01000177 ! grassland biome
is_a: ENVO:01001832 ! subtropical biome
creation_date: 2013-04-07T14:29:48Z

[Term]
id: ENVO:01000192
name: tropical grassland biome
comment: Preliminary definition. The semantics and definitions of "mediterranean", "subtropical", "tropical", "temperate", "polar", and similar climate types may be transferred to an "environmental condition" class once the semantics of this class have been established.
subset: wwfBiome
is_a: ENVO:01000177 ! grassland biome
is_a: ENVO:01001830 ! tropical biome
created_by: ORCID:0000-0002-4366-3088
creation_date: 2013-04-07T14:29:48Z

[Term]
id: ENVO:01000193
name: temperate grassland biome
comment: Preliminary definition. The semantics and definitions of "mediterranean", "subtropical", "tropical", "temperate", "polar", and similar climate types may be transferred to an "environmental condition" class once the semantics of this class have been established.
synonym: "prairie biome" BROAD []
is_a: ENVO:01000177 ! grassland biome
is_a: ENVO:01001831 ! temperate biome
created_by: ORCID:0000-0002-4366-3088
creation_date: 2013-04-07T14:29:48Z

[Term]
id: ENVO:01000194
name: montane grassland biome
def: "A montane grassland biome is a grassland biome which occurs in regions elevated above sea level and which has community structure determined by elevation-dependent environmental conditions." []
comment: Preliminary definition.
subset: wwfBiome
is_a: ENVO:01000177 ! grassland biome
is_a: ENVO:01001836 ! montane biome
created_by: ORCID:0000-0002-4366-3088
creation_date: 2013-04-07T14:29:48Z

[Term]
id: ENVO:01000195
name: flooded grassland biome
subset: wwfBiome
is_a: ENVO:01000177 ! grassland biome
created_by: ORCID:0000-0002-4366-3088
creation_date: 2013-04-07T14:29:48Z

[Term]
id: ENVO:01000196
name: coniferous forest biome
namespace: ENVO
def: "A coniferous forest biome is a forest biome which contains densely packed populations or communities of coniferous trees, strongly limiting light penetration to the forest floor." []
comment: Preliminary definition.
is_a: ENVO:01000174 ! forest biome
created_by: ORCID:0000-0002-4366-3088
creation_date: 2013-04-07T14:31:01Z

[Term]
id: ENVO:01000197
name: broadleaf forest biome
def: "A broadleaf forest ecosystem which is undergoing climactic ecological succession." []
is_a: ENVO:01000174 ! forest biome
created_by: ORCID:0000-0002-4366-3088
creation_date: 2013-04-07T14:31:01Z

[Term]
id: ENVO:01000198
name: mixed forest biome
def: "A mixed forest in which dominant ecological communities have reached their climax successional state." []
subset: wwfBiome
is_a: ENVO:01000174 ! forest biome
created_by: ORCID:0000-0002-4366-3088
creation_date: 2013-04-07T14:31:01Z

[Term]
id: ENVO:01000199
name: mediterranean forest biome
def: "A mediterranean forest in which dominant ecological communities have reached their climax successional state." []
subset: wwfBiome
is_a: ENVO:01000174 ! forest biome
is_a: ENVO:01001833 ! mediterranean biome
created_by: ORCID:0000-0002-4366-3088
creation_date: 2013-04-07T14:31:01Z

[Term]
id: ENVO:01000200
name: tropical broadleaf forest biome
def: "A tropical broadleaf forest in which dominant ecological communities have reached their climax successional state." []
is_a: ENVO:01000197 ! broadleaf forest biome
is_a: ENVO:01001830 ! tropical biome
created_by: ORCID:0000-0002-4366-3088
creation_date: 2013-04-07T14:32:28Z

[Term]
id: ENVO:01000201
name: subtropical broadleaf forest biome
def: "A subtropical broadleaf forest in which dominant ecological communities have reached their climax successional state." []
is_a: ENVO:01000197 ! broadleaf forest biome
is_a: ENVO:01001832 ! subtropical biome
created_by: ORCID:0000-0002-4366-3088
creation_date: 2013-04-07T14:32:28Z

[Term]
id: ENVO:01000202
name: temperate broadleaf forest biome
def: "A broadleaf forest which is subject to temperate climate patterns." []
subset: wwfBiome
is_a: ENVO:01000197 ! broadleaf forest biome
is_a: ENVO:01001831 ! temperate biome
created_by: ORCID:0000-0002-4366-3088
creation_date: 2013-04-07T14:32:28Z

[Term]
id: ENVO:01000208
name: mediterranean woodland biome
def: "A subtropical woodland biome which includes communities adapted to hot to warm, dry summers, mild to cold, rainy winters, and the influence of large, usually marine, bodies of water." []
comment: Preliminary definition. The semantics and definitions of "mediterranean", "subtropical", "tropical", "temperate", "polar", and similar climate types may be transferred to an "environmental condition" class once the semantics of this class have been established.
is_a: ENVO:01000222 ! subtropical woodland biome
is_a: ENVO:01001833 ! mediterranean biome
created_by: ORCID:0000-0002-4366-3088
creation_date: 2013-04-07T15:01:04Z

[Term]
id: ENVO:01000209
name: subtropical coniferous forest biome
def: "A coniferous forest biome which is subject to subtropical climate patterns." []
comment: Preliminary definition. The semantics and definitions of "mediterranean", "subtropical", "tropical", "temperate", "polar", and similar climate types may be transferred to an "environmental condition" class once the semantics of this class have been established.
subset: wwfBiome
is_a: ENVO:01000196 ! coniferous forest biome
is_a: ENVO:01001832 ! subtropical biome
created_by: ORCID:0000-0002-4366-3088
creation_date: 2013-04-07T14:39:14Z

[Term]
id: ENVO:01000210
name: tropical coniferous forest biome
def: "A coniferous forest biome which is subject to tropical climate patterns." []
comment: Preliminary definition. The semantics and definitions of "mediterranean", "subtropical", "tropical", "temperate", "polar", and similar climate types may be transferred to an "environmental condition" class once the semantics of this class have been established.
subset: wwfBiome
is_a: ENVO:01000196 ! coniferous forest biome
is_a: ENVO:01001830 ! tropical biome
created_by: ORCID:0000-0002-4366-3088
creation_date: 2013-04-07T14:39:14Z

[Term]
id: ENVO:01000211
name: temperate coniferous forest biome
def: "A coniferous forest biome which is subject to temperate climate patterns." []
comment: Preliminary definition. The semantics and definitions of "mediterranean", "subtropical", "tropical", "temperate", "polar", and similar climate types may be transferred to an "environmental condition" class once the semantics of this class have been established.
subset: wwfBiome
is_a: ENVO:01000196 ! coniferous forest biome
is_a: ENVO:01001831 ! temperate biome
created_by: ORCID:0000-0002-4366-3088
creation_date: 2013-04-07T14:39:14Z

[Term]
id: ENVO:01000212
name: temperate mixed forest biome
def: "A temperate mixed forest in which dominant ecological communities have reached their climax successional state." []
subset: wwfBiome
is_a: ENVO:01000198 ! mixed forest biome
is_a: ENVO:01001831 ! temperate biome
created_by: ORCID:0000-0002-4366-3088
creation_date: 2013-04-07T14:39:30Z

[Term]
id: ENVO:01000213
name: subtropical shrubland biome
def: "A shrubland biome which is subject to subtropical climate patterns." []
comment: Preliminary definition. The semantics and definitions of "mediterranean", "subtropical", "tropical", "temperate", "polar", and similar climate types may be transferred to an "environmental condition" class once the semantics of this class have been established.
subset: wwfBiome
is_a: ENVO:01000176 ! shrubland biome
is_a: ENVO:01001832 ! subtropical biome
created_by: ORCID:0000-0002-4366-3088
creation_date: 2013-04-07T14:40:32Z

[Term]
id: ENVO:01000214
name: tropical shrubland biome
def: "A shrubland biome which is subject to tropical climate patterns." []
comment: Preliminary definition. The semantics and definitions of "mediterranean", "subtropical", "tropical", "temperate", "polar", and similar climate types may be transferred to an "environmental condition" class once the semantics of this class have been established.
subset: wwfBiome
is_a: ENVO:01000176 ! shrubland biome
is_a: ENVO:01001830 ! tropical biome
created_by: ORCID:0000-0002-4366-3088
creation_date: 2013-04-07T14:40:32Z

[Term]
id: ENVO:01000215
name: temperate shrubland biome
def: "A shrubland biome which is subject to temperate climate patterns." []
comment: Preliminary definition. The semantics and definitions of "mediterranean", "subtropical", "tropical", "temperate", "polar", and similar climate types may be transferred to an "environmental condition" class once the semantics of this class have been established.
synonym: "prairie biome" BROAD []
is_a: ENVO:01000176 ! shrubland biome
is_a: ENVO:01001831 ! temperate biome
created_by: ORCID:0000-0002-4366-3088
creation_date: 2013-04-07T14:40:32Z

[Term]
id: ENVO:01000216
name: montane shrubland biome
def: "A montane shrubland biome is a shrubland biome which occurs in regions elevated above sea level and which has community structure determined by elevation-dependent environmental conditions." []
comment: Preliminary definition.
subset: wwfBiome
is_a: ENVO:01000176 ! shrubland biome
is_a: ENVO:01001836 ! montane biome
created_by: ORCID:0000-0002-4366-3088
creation_date: 2013-04-07T14:40:32Z

[Term]
id: ENVO:01000217
name: mediterranean shrubland biome
def: "A mediterranean shrubland biome is a subtropical shrubland biome which includes communities adapted to hot to warm, dry summers, mild to cold, rainy winters, and the influence of large, usually marine, bodies of water." []
comment: Preliminary definition. The semantics and definitions of "mediterranean", "subtropical", "tropical", "temperate", "polar", and similar climate types may be transferred to an "environmental condition" class once the semantics of this class have been established.
subset: wwfBiome
is_a: ENVO:01000213 ! subtropical shrubland biome
is_a: ENVO:01001833 ! mediterranean biome
created_by: ORCID:0000-0002-4366-3088
creation_date: 2013-04-07T14:40:32Z

[Term]
id: ENVO:01000218
name: xeric shrubland biome
namespace: ENVO
comment: Preliminary definition. The semantics and definitions of "mediterranean", "subtropical", "tropical", "temperate", "polar", and similar climate types may be transferred to an "environmental condition" class once the semantics of this class have been established.
subset: wwfBiome
is_a: ENVO:01000176 ! shrubland biome
created_by: ORCID:0000-0002-4366-3088
creation_date: 2013-04-07T14:40:32Z

[Term]
id: ENVO:01000219
name: anthropogenic terrestrial biome
def: "An anthropogenic terrestrial biome is a terrestrial biome which has community structures determined by human activity." [http://www.eoearth.org/view/article/150128/]
comment: Preliminary definition.
synonym: "anthrome" EXACT []
synonym: "human biome" EXACT []
is_a: ENVO:00000446 ! terrestrial biome
created_by: ORCID:0000-0002-4366-3088
creation_date: 2013-04-07T14:45:22Z

[Term]
id: ENVO:01000220
name: tropical woodland biome
def: "A woodland biome which is subject to tropical climate patterns." []
comment: Preliminary definition. The semantics and definitions of "mediterranean", "subtropical", "tropical", "temperate", "polar", and similar climate types may be transferred to an "environmental condition" class once the semantics of this class have been established.
is_a: ENVO:01000175 ! woodland biome
is_a: ENVO:01001830 ! tropical biome
created_by: ORCID:0000-0002-4366-3088
creation_date: 2013-04-07T15:01:04Z

[Term]
id: ENVO:01000221
name: temperate woodland biome
def: "A woodland biome which is subject to temperate climate patterns." []
comment: Preliminary definition. The semantics and definitions of "mediterranean", "subtropical", "tropical", "temperate", "polar", and similar climate types may be transferred to an "environmental condition" class once the semantics of this class have been established.
is_a: ENVO:01000175 ! woodland biome
is_a: ENVO:01001831 ! temperate biome
created_by: ORCID:0000-0002-4366-3088
creation_date: 2013-04-07T15:01:04Z

[Term]
id: ENVO:01000222
name: subtropical woodland biome
def: "A woodland biome which is subject to subtropical climate patterns." []
comment: Preliminary definition. The semantics and definitions of "mediterranean", "subtropical", "tropical", "temperate", "polar", and similar climate types may be transferred to an "environmental condition" class once the semantics of this class have been established.
is_a: ENVO:01000175 ! woodland biome
is_a: ENVO:01001832 ! subtropical biome
created_by: ORCID:0000-0002-4366-3088
creation_date: 2013-04-07T15:01:04Z

[Term]
id: ENVO:01000223
name: montane savanna biome
def: "A montane savanna biome is a savanna biome which occurs in regions elevated above sea level and which has community structure determined by elevation-dependent environmental conditions." []
comment: Preliminary definition.
is_a: ENVO:01000178 ! savanna biome
is_a: ENVO:01001836 ! montane biome
created_by: ORCID:0000-0002-4366-3088
creation_date: 2013-04-07T16:50:01Z

[Term]
id: ENVO:01000224
name: mediterranean grassland biome
def: "A subtropical grassland biome which includes communities adapted to hot to warm, dry summers, mild to cold, rainy winters, and the influence of large, usually marine, bodies of water." []
comment: Preliminary definition. The semantics and definitions of "mediterranean", "subtropical", "tropical", "temperate", "polar", and similar climate types may be transferred to an "environmental condition" class once the semantics of this class have been established.
is_a: ENVO:01000191 ! subtropical grassland biome
is_a: ENVO:01001833 ! mediterranean biome
created_by: ORCID:0000-0002-4366-3088
creation_date: 2013-04-19T11:42:48Z

[Term]
id: ENVO:01000225
name: subtropical dry broadleaf forest biome
def: "A subtropical dry broadleaf forest in which dominant ecological communities have reached their climax successional state." []
subset: wwfBiome
xref: https://www.worldwildlife.org/biomes/tropical-and-subtropical-dry-broadleaf-forests
is_a: ENVO:01000201 ! subtropical broadleaf forest biome
created_by: ORCID:0000-0002-4366-3088
creation_date: 2013-04-24T12:04:53Z

[Term]
id: ENVO:01000226
name: subtropical moist broadleaf forest biome
def: "A subtropical moist broadleaf forest in which dominant ecological communities have reached their climax successional state." []
subset: wwfBiome
is_a: ENVO:01000201 ! subtropical broadleaf forest biome
created_by: ORCID:0000-0002-4366-3088
creation_date: 2013-04-24T12:04:53Z

[Term]
id: ENVO:01000227
name: tropical dry broadleaf forest biome
def: "A tropical dry broadleaf forest in which dominant ecological communities have reached their climax successional state." []
subset: wwfBiome
xref: https://www.worldwildlife.org/biomes/tropical-and-subtropical-dry-broadleaf-forests
is_a: ENVO:01000200 ! tropical broadleaf forest biome
created_by: ORCID:0000-0002-4366-3088
creation_date: 2013-04-24T12:05:25Z

[Term]
id: ENVO:01000228
name: tropical moist broadleaf forest biome
def: "A tropical moist broadleaf forest in which dominant ecological communities have reached their climax successional state." []
subset: wwfBiome
synonym: "rainforest biome" RELATED []
xref: SPIRE:Rainforest
is_a: ENVO:01000200 ! tropical broadleaf forest biome
created_by: ORCID:0000-0002-4366-3088
creation_date: 2013-04-24T12:05:25Z

[Term]
id: ENVO:01000229
name: mediterranean savanna biome
def: "A savanna biome which is subject to mediterranean climate patterns." []
subset: wwfBiome
is_a: ENVO:01000187 ! subtropical savanna biome
is_a: ENVO:01001833 ! mediterranean biome
created_by: ORCID:0000-0002-4366-3088
creation_date: 2013-04-24T12:20:42Z

[Term]
id: ENVO:01000245
name: cropland biome
def: "A cropland ecosystem which is undergoing climactic ecological succession." [http://dx.doi.org/10.1111/j.1466-8238.2010.00540.x, http://dx.doi.org/10.1890/070062]
is_a: ENVO:01000219 ! anthropogenic terrestrial biome
created_by: ORCID:0000-0002-4366-3088
creation_date: 2013-06-14T11:45:47Z

[Term]
id: ENVO:01000246
name: village biome
def: "A village biome is an anthropogenic terrestrial biome which contains settlements such as villages, towns, and/or small cities and which is primarily used for agricultural activity." [DOI:10.1111/j.1466-8238.2010.00540.x, DOI:10.1890/070062]
comment: Villages are also described as agricultural settlements with greater than 100 persons per square kilometre; however, no upper limit is defined.
is_a: ENVO:00000428 ! biome
created_by: ORCID:0000-0002-4366-3088
creation_date: 2013-06-14T11:45:47Z

[Term]
id: ENVO:01000247
name: rangeland biome
def: "A rangeland biome is an anthropogenic terrestrial biome which is primarily used for the rearing and grazing of livestock." [DOI:10.1111/j.1466-8238.2010.00540.x, DOI:10.1890/070062]
is_a: ENVO:01000219 ! anthropogenic terrestrial biome
created_by: ORCID:0000-0002-4366-3088
creation_date: 2013-06-14T11:45:47Z

[Term]
id: ENVO:01000248
name: dense settlement biome
def: "A dense settlement biome is an anthropogenic terrestrial biome which is primarily used for human habitation, recreation, and industry within built structures with little other land use." [DOI:10.1111/j.1466-8238.2010.00540.x, DOI:10.1890/070062]
is_a: ENVO:00000428 ! biome
created_by: ORCID:0000-0002-4366-3088
creation_date: 2013-06-14T11:45:47Z

[Term]
id: ENVO:01000249
name: urban biome
namespace: ENVO
def: "An urban biome is a dense settlement biome which has been urbanised." [DOI:10.1111/j.1466-8238.2010.00540.x, DOI:10.1890/070062]
xref: SPIRE:Urban
is_a: ENVO:01000248 ! dense settlement biome
created_by: ORCID:0000-0002-4366-3088
creation_date: 2013-06-14T11:45:47Z

[Term]
id: ENVO:01000250
name: subpolar coniferous forest biome
def: "A  coniferous forest biome which includes communities adapted to subpolar conditions." []
subset: wwfBiome
synonym: "boreal forest" NARROW []
synonym: "taiga" NARROW []
xref: EcoLexicon:taiga
xref: LTER:72
xref: SPIRE:Taiga
is_a: ENVO:01000196 ! coniferous forest biome
is_a: ENVO:01001834 ! subpolar biome
creation_date: 2013-09-04T06:41:53Z

[Term]
id: ENVO:01000252
name: freshwater lake biome
def: "A biome which is determined by a freshwater lake." []
is_a: ENVO:00000873 ! freshwater biome
creation_date: 2013-09-19T11:11:01Z

[Term]
id: ENVO:01000253
name: freshwater river biome
def: "A freshwater biome which is determined by a freshwater river." []
is_a: ENVO:00000873 ! freshwater biome
creation_date: 2013-09-19T11:11:01Z

[Term]
id: ENVO:01000339
name: polar biome
def: "A biome which is subject to polar climatic conditions." []
comment: This class is primarily for inference and, in general, should not be used directly by annotators. If you're an annotator, please consider using a more informative term such as 'tundra biome'.
subset: envoPolar
is_a: ENVO:00000428 ! biome

[Term]
id: ENVO:01000854
name: tropical marine coral reef biome
def: "A marine coral reef biome which is located in a region with a tropical climate." []
subset: wwfBiome
is_a: ENVO:01000049 ! marine coral reef biome
is_a: ENVO:01001830 ! tropical biome

[Term]
id: ENVO:01000856
name: temperate marginal sea biome
def: "A marginal sea biome which is located in a region with a temperate climate." []
subset: wwfBiome
is_a: ENVO:01000046 ! marginal sea biome
is_a: ENVO:01001831 ! temperate biome
property_value: IAO:0000116 "A component of the WWF Temperate Shelf and seas ecoregions grouping" xsd:string

[Term]
id: ENVO:01000857
name: temperate mediterranean sea biome
def: "A mediterranean sea biome which is subject to temperate climate patterns." []
subset: wwfBiome
is_a: ENVO:01000047 ! mediterranean sea biome

[Term]
id: ENVO:01000858
name: marine upwelling biome
def: "A marine biome which contains communities adapted to living in an environment determined by an upwelling process." []
is_a: ENVO:00000447 ! marine biome

[Term]
id: ENVO:01000859
name: tropical marine upwelling biome
def: "A marine upwelling biome which is subject to tropical climate patterns." []
subset: wwfBiome
is_a: ENVO:01000858 ! marine upwelling biome
is_a: ENVO:01001830 ! tropical biome

[Term]
id: ENVO:01000860
name: temperate marine upwelling biome
def: "A marine upwelling biome which is located in a region subject to temperate climate patterns." []
subset: wwfBiome
is_a: ENVO:01000858 ! marine upwelling biome
is_a: ENVO:01001831 ! temperate biome

[Term]
id: ENVO:01001230
name: tropical marginal sea biome
def: "A marginal sea biome which is located in a region with a tropical climate." []
is_a: ENVO:01000046 ! marginal sea biome
is_a: ENVO:01001830 ! tropical biome
property_value: IAO:0000116 "A class which is complementary to the WWF Temperate Shelf and Seas ecoregions grouping" xsd:string

[Term]
id: ENVO:01001369
name: tidal mangrove shrubland
def: "A shrubland biome which is densely vegetated by dwarf or short mangroves (and associates) that are generally less than 6 meters in height, is tidally influenced,  is located in tropical or subtropical areas." []
comment: This class aligns to the Coastal and Marine Ecological Classification Standard (CMECS). In ENVO, we may adapt the definition for consistency, but the semantics (meaning) of the term should be unaffected. Please consult the CMECS catalogue (https://cmecscatalog.org/) for authoritative and semantically unconstrained definitions. CMECS provides the following notes: "Commonly found on intertidal mud flats along the shores of estuaries. Tidal mangrove shrublands may include immature stands or stunted mature trees that indicate a harsh growing environment. Areas characterized by tall mangroves (> 6 meters) are placed in the Tidal Mangrove Forest Biotic Group. Where tidal amplitude is relatively low, the vegetation forms narrow bands along the coastal plains, and it rarely penetrates inland more than several kilometers along rivers. Where tidal amplitude is greater, mangroves extend further inland along river courses, forming extensive stands in the major river deltas. Also, mangrove cays may occur within the lagoon complex of barrier reefs. The list of biotic communities for this group is long: a few examples are provided below, and the complete list is available in Appendix F"
subset: envoCmecs
subset: envoMarine
xref: CMECS:577
xref: https://cmecscatalog.org/cmecs/classification/unit/577.html
is_a: ENVO:01000176 ! shrubland biome
created_by: https://orcid.org/0000-0002-4366-3088

[Term]
id: ENVO:01001505
name: alpine tundra biome
def: "A tundra biome which exists at high altitudes and where vegetation - dominated by a few species of dwarf shrubs, a few grasses, sedges, lichens, and mosses - is stunted due to low temperatures and high winds." [https://en.wikipedia.org/wiki/Alpine_tundra]
comment: The absence of trees in this biome is primarily due to high altitude rather than high latitude. On Earth, it lies roughly between the summer isotherm of 10 degrees Centigrade and the snow line. Primary productivity is low in this biome because of the extremes of climate. {xref="https://orcid.org/0000-0003-4808-4736"}
subset: envoPolar
synonym: "mountain tundra" EXACT [https://orcid.org/0000-0003-4808-4736]
xref: http://sweetontology.net/realmCryo/AlpineTundra
xref: SPIRE:Tundra
is_a: ENVO:01000180 ! tundra biome
is_a: ENVO:01001835 ! alpine biome
created_by: https://orcid.org/0000-0002-4366-3088
creation_date: 2019-01-14T16:26:18Z

[Term]
id: ENVO:01001798
name: tropical mixed forest biome
def: "A tropical mixed forest in which dominant ecological communities have reached their climax successional state." []
subset: wwfBiome
is_a: ENVO:01000198 ! mixed forest biome
is_a: ENVO:01001830 ! tropical biome
property_value: http://purl.org/dc/elements/1.1/creator https://orcid.org/0000-0002-4366-3088
property_value: http://purl.org/dc/elements/1.1/date 2019-10-27T16:05:39Z xsd:dateTime

[Term]
id: ENVO:01001830
name: tropical biome
def: "A biome which is subject to tropical climatic conditions." []
is_a: ENVO:00000428 ! biome
property_value: http://purl.org/dc/elements/1.1/creator https://orcid.org/0000-0002-4366-3088
property_value: http://purl.org/dc/elements/1.1/date 2019-11-06T15:56:17Z xsd:dateTime

[Term]
id: ENVO:01001831
name: temperate biome
def: "A biome which is subject to temperate climatic conditions." []
is_a: ENVO:00000428 ! biome
property_value: http://purl.org/dc/elements/1.1/creator https://orcid.org/0000-0002-4366-3088
property_value: http://purl.org/dc/elements/1.1/date 2019-11-06T15:57:04Z xsd:dateTime

[Term]
id: ENVO:01001832
name: subtropical biome
def: "A biome which is subject to subtropical climatic conditions." []
is_a: ENVO:00000428 ! biome
property_value: http://purl.org/dc/elements/1.1/creator https://orcid.org/0000-0002-4366-3088
property_value: http://purl.org/dc/elements/1.1/date 2019-11-06T15:57:36Z xsd:dateTime

[Term]
id: ENVO:01001833
name: mediterranean biome
def: "A biome which is subject to mediterranean climatic conditions." []
is_a: ENVO:01001832 ! subtropical biome
property_value: http://purl.org/dc/elements/1.1/creator https://orcid.org/0000-0002-4366-3088
property_value: http://purl.org/dc/elements/1.1/date 2019-11-06T15:58:10Z xsd:dateTime

[Term]
id: ENVO:01001834
name: subpolar biome
def: "A biome which is subject to subpolar climatic conditions." []
is_a: ENVO:00000428 ! biome
property_value: http://purl.org/dc/elements/1.1/creator https://orcid.org/0000-0002-4366-3088
property_value: http://purl.org/dc/elements/1.1/date 2019-11-06T15:58:56Z xsd:dateTime

[Term]
id: ENVO:01001835
name: alpine biome
def: "A biome which is subject to alpine altitudinal conditions." []
is_a: ENVO:00000428 ! biome
property_value: http://purl.org/dc/elements/1.1/creator https://orcid.org/0000-0002-4366-3088
property_value: http://purl.org/dc/elements/1.1/date 2019-11-06T15:59:35Z xsd:dateTime

[Term]
id: ENVO:01001836
name: montane biome
def: "A biome which is subject to montane altitudinal conditions." []
is_a: ENVO:00000428 ! biome
property_value: http://purl.org/dc/elements/1.1/creator https://orcid.org/0000-0002-4366-3088
property_value: http://purl.org/dc/elements/1.1/date 2019-11-06T16:00:33Z xsd:dateTime

[Term]
id: ENVO:01001837
name: subalpine biome
def: "A biome which is subject to subapline altitudinal conditions." []
is_a: ENVO:00000428 ! biome
property_value: http://purl.org/dc/elements/1.1/creator https://orcid.org/0000-0002-4366-3088
property_value: http://purl.org/dc/elements/1.1/date 2019-11-06T16:01:49Z xsd:dateTime

[Term]
id: ENVO:01001838
name: arid biome
def: "A biome which is subject to arid environmental conditions." []
is_a: ENVO:00000428 ! biome
property_value: http://purl.org/dc/elements/1.1/creator https://orcid.org/0000-0002-4366-3088
property_value: http://purl.org/dc/elements/1.1/date 2019-11-06T16:06:47Z xsd:dateTime

[Term]
id: ENVO:03605008
name: freshwater stream biome
def: "A freshwater stream ecosystem which is undergoing climactic ecological succession." []
is_a: ENVO:00000873 ! freshwater biome
property_value: http://purl.org/dc/elements/1.1/creator https://orcid.org/0000-0001-9076-6066
property_value: http://purl.org/dc/elements/1.1/date 2024-01-10T19:19:00Z xsd:dateTime

