format-version: 1.2
data-version: envo/releases/2025-10-20/subsets/envoOmics.owl
subsetdef: disposition_slim "Disposition slim"
subsetdef: environmental_hazards "environmental_hazards"
subsetdef: EnvO-Lite-GSC "EnvO-Lite-GSC"
subsetdef: envoANZSoil "envoANZSoil"
subsetdef: envoAstro "envoAstro"
subsetdef: envoAtmo "envoAtmo"
subsetdef: envoCesab "envoCesab"
subsetdef: envoCmecs "envoCmecs"
subsetdef: envoEmpo "envoEmpo"
subsetdef: envoEOVs "envoEOVs"
subsetdef: envoMarine "envoMarine"
subsetdef: envoMeo "envoMeo"
subsetdef: envoNceas "envoNceas"
subsetdef: envoOmics "envoOmics"
subsetdef: envoPlastics "envoPlastics"
subsetdef: envoPolar "envoPolar"
subsetdef: mpath_slim "Pathology slim"
subsetdef: nlcd2011 "nlcd2011"
subsetdef: relational_slim "Relational slim: types of quality that require an additional entity in order to exist"
subsetdef: ro-eco "ro-eco"
subsetdef: scalar_slim "Scalar slim"
subsetdef: value_slim "Value slim"
subsetdef: wwfBiome "wwfBiome"
synonymtypedef: OMO:0003004 "plural form"
ontology: envo/subsets/envoOmics
property_value: owl:versionInfo "2025-10-20" xsd:string

[Term]
id: ENVO:00000340
name: particle of sand
namespace: ENVO
def: "A particle which 1) is composed primarily of and derived from rock or mineral sources and 2) is or was part of a portion of sand." [https://en.wikipedia.org/wiki/Sand]
comment: In general, sand grains are larger than those of silt, but finer than those of gravel.
synonym: "grain of sand" EXACT []
synonym: "granule of sand" EXACT []
synonym: "sand granule" EXACT []
is_a: ENVO:01003002 ! particle
disjoint_from: ENVO:01000017 ! sand

[Term]
id: ENVO:00000343
name: particle of silt
namespace: ENVO
def: "A particle which 1) is primarily composed of quartz or feldspar and 2) is or was part of a portion of silt." []
comment: The distinction between silt and clay varies by discipline. Geologists and soil scientists usually consider the separation to occur at a particle size of 2 μm (clays being finer than silts), sedimentologists often use 4–5 μm, and colloid chemists use 1 μm. Geotechnical engineers distinguish between silts and clays based on the plasticity properties of the soil, as measured by the soils' Atterberg limits. ISO 14688 grades clay particles as being smaller than 2 μm and silt particles as being larger. Mixtures of sand, silt and less than 40% clay are called loam. {xref="Properties"}
synonym: "grain of silt" EXACT []
synonym: "granule of silt" EXACT []
is_a: ENVO:01003002 ! particle

[Term]
id: ENVO:00000369
alt_id: ENVO:01000060

[Term]
id: ENVO:00001998
name: soil
namespace: ENVO
def: "An environmental material which is primarily composed of minerals, varying proportions of sand, silt, and clay, organic material such as humus, interstitial gases, liquids, and a broad range of resident micro- and macroorganisms." [https://en.wikipedia.org/wiki/Soil]
comment: 'In engineering terms, soil is referred to as regolith, or loose rock material that lies above the 'solid geology'. Soil is commonly referred to as "earth" or "dirt"; technically, the term "dirt" should be restricted to displaced soil.' https://en.wikipedia.org/wiki/Soil\n\n" The upper limit of soil is the boundary between soil and air, shallow water, live plants, or plant materials that have not begun to decompose. Areas are not considered to have soil if the surface is permanently covered by water too deep (typically more than 2.5 meters) for the growth of rooted plants.\n\nThe lower boundary that separates soil from the nonsoil underneath is most difficult to define. Soil consists of horizons near the Earth's surface that, in contrast to the underlying parent material, have been altered by the interactions of climate, relief, and living organisms over time. Commonly, soil grades at its lower boundary to hard rock or to earthy materials virtually devoid of animals, roots, or other marks of biological activity. For purposes of classification, the lower boundary of soil is arbitrarily set at 200 cm."  Soil taxonomy, 2nd Ed., quoted in http://www.nrcs.usda.gov/wps/portal/nrcs/detail/soils/edu/?cid=nrcs142p2_054280
subset: EnvO-Lite-GSC
subset: ENVO:03605015
synonym: "regolith" BROAD []
xref: https://en.wikipedia.org/wiki/Soil
xref: LTER:535
xref: SPIRE:Soil
xref: SWEETRealm:Soil
is_a: ENVO:00010483 ! environmental material
relationship: has_disposition ENVO:06105304 ! water-holding capacity of soil
relationship: has_part ENVO:00002982 ! clay
relationship: has_part ENVO:01000016 ! silt
relationship: has_part ENVO:01000017 ! sand
relationship: has_part ENVO:01000155 ! organic material
relationship: has_part ENVO:01000256 ! mineral material
relationship: part_of ENVO:01000820 ! pedosphere
property_value: IAO:0000116 "The various 'has part' and 'has quality' relations may not hold true for all soils; however, I have yet to find counter examples. Require input from a pedologist or similar. [pbuttigieg]" xsd:string

[Term]
id: ENVO:00002006
name: liquid water
namespace: ENVO
def: "An environmental material primarily composed of dihydrogen oxide in its liquid form." [MA:ma]
subset: ENVO:03605019
synonym: "water" BROAD []
xref: EcoLexicon:water
xref: https://en.wikipedia.org/wiki/Water
xref: LTER:617
is_a: ENVO:01000815 ! liquid environmental material

[Term]
id: ENVO:00002007
name: sediment
namespace: ENVO
def: "Particulate environmental material which is formed as a result of the transport and deposition of particles by flowing liquid." [https://en.wikipedia.org/wiki/Sediment]
comment: Sediment is typically deposited on the bed or bottom of a body of water or other liquid.
subset: EnvO-Lite-GSC
subset: ENVO:03605026
subset: envoPolar
xref: EcoLexicon:sediment
xref: EcoLexicon:sedimentation
xref: https://en.wikipedia.org/wiki/Sediment
xref: LTER:492
xref: LTER:493
xref: SWEETRealm:Sediment
is_a: ENVO:01000060

[Term]
id: ENVO:00002010
name: saline water
namespace: ENVO
def: "Water which contains a significant concentration of dissolved salts." []
comment: The threshold salt concentration for classifying water as saline varies, but typically begins at about 1,000 to 3,000 parts salt per million parts water or 0.1–0.3% salt by weight.
subset: ENVO:03605019
synonym: "salt water" EXACT []
xref: EcoLexicon:saltwater
xref: https://en.wikipedia.org/wiki/Saline_water
xref: SWEETRealm:SalineWater
xref: SWEETRealm:SaltWater
is_a: ENVO:00002006 ! liquid water

[Term]
id: ENVO:00002011
name: fresh water
namespace: ENVO
def: "Water which has a low concentration of dissolved solutes, particularly that of sodium chloride." []
comment: The lower bound of solute concentration required for water to be considered freshwater is variable, but is always less than that of seawater, and often cited as less than 1 gram of solutes per 1 litre of water.
subset: ENVO:03605019
subset: envoEmpo
subset: envoPolar
synonym: "freshwater" EXACT []
synonym: "sweet water" RELATED []
xref: EcoLexicon:fresh_water
xref: https://en.wikipedia.org/wiki/Fresh_water
xref: LTER:216
xref: SWEETRealm:FreshWater
is_a: ENVO:00002006 ! liquid water

[Term]
id: ENVO:00002982
name: clay
namespace: ENVO
def: "Particulate environmental material which 1) is composed primarily of clay particles, with only minor proportions of other materials, 2) demonstrates plasticity when wet, and 3) is capable of hardening when dried or fired." [https://en.wikipedia.org/wiki/Clay]
comment: This definition is intentionally ambiguous to support the multiple thresholds set by different authorities.The distinction between silt and clay varies by discipline. Geologists and soil scientists usually consider the separation to occur at a particle size of 2 μm (clays being finer than silts), sedimentologists often use 4–5 μm, and colloid chemists use 1 μm. Geotechnical engineers distinguish between silts and clays based on the plasticity properties of the soil, as measured by the soils' Atterberg limits. ISO 14688 grades clay particles as being smaller than 2 μm and silt particles as being larger. Mixtures of sand, silt and less than 40% clay are called loam. Similar mixtures with greater than 40% clay are often considered clay soils. {xref="https://en.wikipedia.org/wiki/Clay"}
xref: EcoLexicon:clay
xref: SWEETRealm:Clay
is_a: ENVO:01000060
disjoint_from: ENVO:01000016 ! silt
relationship: has_part ENVO:01003003 ! particle of clay
property_value: IAO:0000116 "Do not oversimplify the particulate environmental material subclasses with design patterns or similar. The materials have properties that their components do not - write full definitions including these where possible." xsd:string

[Term]
id: ENVO:00005791
name: sterile water
namespace: ENVO
def: "Sterile water is water which does not contain lliving organisms." []
subset: ENVO:03605019
is_a: ENVO:00002006 ! liquid water

[Term]
id: ENVO:00005801
name: rhizosphere
namespace: ENVO
def: "The narrow region of soil that is directly influenced by root secretions and associated soil microorganisms." [https://en.wikipedia.org/wiki/Rhizosphere_%28ecology%29]
subset: ENVO:03605014
subset: ENVO:03605024
xref: LTER:472
is_a: ENVO:01001110 ! ecosystem
relationship: part_of ENVO:00001998 ! soil

[Term]
id: ENVO:00010483
name: environmental material
namespace: ENVO
def: "A material entity which other material entities in an environmental system are primarily or partially composed of." [http://ontology.buffalo.edu/smith/articles/niches.html, https://dx.doi.org/10.1186/2041-1480-4-43, https://en.wikipedia.org/wiki/Material]
comment: Everything under this parent must be a mass noun (i.e. not countable). All subclasses are to be understood as being composed primarily of the named entity, rather than restricted to that entity. For example, "ENVO:water" is to be understood as "environmental material composed primarly of some CHEBI:water".
comment: Instances of this class are portions of environmental materials, such as seawater in bucket, a water parcel in the photic zone of a lake, or the concrete that composes a building part. Instances of these portions may have fiat or non-fiat boundaries. For example, a water parcel has not physical boundaries, while the seawater in a bucket is bounded by the internal surfaces of the bucket.
synonym: "portion of environmental material" EXACT []

[Term]
id: ENVO:01000016
name: silt
namespace: ENVO
def: "Particulate environmental material which is primarily composed of silt particles." [https://en.wikipedia.org/wiki/Silt]
comment: This definition is intentionally ambiguous to support the multiple thresholds set by different authorities. Some authorities consider this soil material that contains 80% or more silt and less than 12% clay. In the Udden-Wentworth scale (due to Krumbein), silt particles range between 0.0039 to 0.0625 mm, larger than clay but smaller than sand particles. ISO 14688 grades silts between 0.002 mm and 0.063 mm. In actuality, silt is chemically distinct from clay, and unlike clay, grains of silt are approximately the same size in all dimensions; furthermore, their size ranges overlap. Clays are formed from thin plate-shaped particles held together by electrostatic forces, so present a cohesion. According to the U.S. Department of Agriculture Soil Texture Classification system, the sand-silt distinction is made at the 0.05 mm particle size. The USDA system has been adopted by the Food and Agriculture Organization (FAO). In the Unified Soil Classification System (USCS) and the AASHTO Soil Classification system, the sand-silt distinction is made at the 0.075 mm particle size (i.e., material passing the #200 sieve). Silts and clays are distinguished mechanically by their plasticity. {xref="https://sis.agr.gc.ca/cansis/glossary/t/index.html", xref="https://en.wikipedia.org/wiki/Silt"}
xref: EcoLexicon:silt
xref: https://en.wikipedia.org/wiki/Silt
xref: SWEETRealm:Silt
is_a: ENVO:01000060
disjoint_from: ENVO:01000017 ! sand
relationship: has_part ENVO:00000343 ! particle of silt
property_value: IAO:0000116 "Do not oversimplify the particulate environmental material subclasses with design patterns or similar. The materials have properties that their components do not - write full definitions including these where possible." xsd:string

[Term]
id: ENVO:01000017
name: sand
namespace: ENVO
def: "Particulate environmental material which is composed primarily of particles of sand with only minor proportions of other substances." [https://en.wikipedia.org/wiki/Sand]
comment: This definition is intentionally ambiguous to support the multiple thresholds set by different authorities. Some authorities consider as sands soil material that contains 85% or more sand; the percentage of silt plus 1.5 times the percentage of clay does not exceed 15. coarse sand (sable grossier) 25% or more very coarse and coarse sand, and less than 50% any other one grade of sand. {xref="https://sis.agr.gc.ca/cansis/glossary/t/index.html"}
xref: EcoLexicon:sand
xref: https://en.wikipedia.org/wiki/Sand
xref: LTER:484
xref: SWEETRealm:Sand
is_a: ENVO:01000060
relationship: has_part ENVO:00000340 ! particle of sand
property_value: IAO:0000116 "Do not oversimplify the particulate environmental material subclasses with design patterns or similar. The materials have properties that their components do not - write full definitions including these where possible." xsd:string

[Term]
id: ENVO:01000060
is_a: ENVO:00010483 ! environmental material
relationship: has_part ENVO:01003002 ! particle

[Term]
id: ENVO:01000155
name: organic material
namespace: ENVO
def: "Environmental material derived from living organisms and composed primarily of one or more biomacromolecules." [ISBN:978-0-618-45504-1, ORCID:0000-0002-4366-3088]
synonym: "biomass" EXACT []
xref: EcoLexicon:organic_material
is_a: ENVO:00010483 ! environmental material
created_by: ORCID:0000-0002-4366-3088
creation_date: 2010-03-20T08:40:04Z

[Term]
id: ENVO:01000254
name: environmental system
namespace: ENVO
def: "A system which has the disposition to environ one or more material entities." [DOI:10.1186/2041-1480-4-43]
comment: In ENVO's alignment with the Basic Formal Ontology, this class is being considered as a subclass of a proposed BFO class "system". The relation "environed_by" is also under development. Roughly, a system which includes a material entity (at least partially) within its site and causally influences that entity may be considered to environ it. Following the completion of this alignment, this class' definition and the definitions of its subclasses will be revised.
synonym: "environment" EXACT []
xref: EcoLexicon:environment
creation_date: 2013-09-23T16:04:08Z

[Term]
id: ENVO:01000256
name: mineral material
namespace: ENVO
def: "A mineral material is an environmental material which is primarily composed of some substance that is naturally occurring, solid and stable at room temperature, representable by a chemical formula, usually abiogenic, and that has an ordered atomic structure." [https://en.wikipedia.org/wiki/Mineral]
xref: LTER:341
is_a: ENVO:00010483 ! environmental material
property_value: IAO:0000116 "Look for \"mineral\" in a chemical or geochemical ontology to formalise the composed primarily of link.\nFrom https://en.wikipedia.org/wiki/ [A mineral] is different from a rock, which can be an aggregate of minerals or non-minerals and does not have a specific chemical composition. The exact definition of a mineral is under debate, especially with respect to the requirement a valid species be abiogenic, and to a lesser extent with regards to it having an ordered atomic structure." xsd:string
created_by: ORCID:0000-0002-4366-3088
creation_date: 2013-10-05T12:37:41Z

[Term]
id: ENVO:01000267
name: atmosphere
namespace: ENVO
def: "An atmosphere is a layer of gases surrounding a material body of sufficient mass that is held in place by the gravity of the body." [https://en.wikipedia.org/wiki/Atmosphere, https://en.wikipedia.org/wiki/Physical_geography]
xref: LTER:48
is_a: ENVO:01001678 ! fluid layer
relationship: adjacent_to ENVO:01000799 ! astronomical body
created_by: ORCID:0000-0002-4366-3088
creation_date: 2013-10-10T08:14:50Z

[Term]
id: ENVO:01000281
name: layer
namespace: ENVO
def: "A material entity which 1) is spatially continuous, 2) is composed of material of comparable thickness, composition, and physical properties, and 3) is physically distinct from adjacent portions of environmental material." [https://en.wiktionary.org/wiki/layer]
subset: envoPolar
created_by: https://orcid.org/0000-0002-4366-3088
creation_date: 2013-10-15T16:42:02Z

[Term]
id: ENVO:01000306
name: freshwater environment
namespace: ENVO
def: "An aquatic environment which is determined by freshwater." []
subset: envoEmpo
subset: envoOmics
subset: envoPolar
synonym: "fresh water environment" EXACT []
is_a: ENVO:01000317 ! aquatic environment
intersection_of: ENVO:01000317 ! aquatic environment
intersection_of: determined_by ENVO:00002011 ! fresh water
property_value: IAO:0000118 "Water (non-saline)" xsd:string {xref="http://press.igsb.anl.gov/earthmicrobiome/protocols-and-standards/emp-ontology-empo/"}

[Term]
id: ENVO:01000307
name: saline water environment
namespace: ENVO
def: "An environmental system which has its properties and dynamics determined by saline water." []
subset: envoEmpo
subset: envoOmics
subset: envoPolar
is_a: ENVO:01000317 ! aquatic environment
intersection_of: ENVO:01000317 ! aquatic environment
intersection_of: determined_by ENVO:00002010 ! saline water
property_value: IAO:0000118 "Water (saline)" xsd:string {xref="http://press.igsb.anl.gov/earthmicrobiome/protocols-and-standards/emp-ontology-empo/"}

[Term]
id: ENVO:01000317
name: aquatic environment
namespace: ENVO
def: "An environment whose dynamics are strongly influenced by water." []
is_a: ENVO:01000254 ! environmental system
intersection_of: ENVO:01000254 ! environmental system
intersection_of: determined_by ENVO:00002006 ! liquid water

[Term]
id: ENVO:01000637
name: outer space
namespace: ENVO
def: "Outer space is a hard vacuum containing a low density of particles, predominantly a plasma of hydrogen and helium as well as electromagnetic radiation, magnetic fields, neutrinos, dust and cosmic rays that exists between celestial bodies." [https://en.wikipedia.org/wiki/Outer_space]
subset: envoAstro
synonym: "space" BROAD []
is_a: ENVO:00010483 ! environmental material

[Term]
id: ENVO:01000638
name: planetary crust
namespace: ENVO
def: "A planetary crust is the outermost solid shell of a rocky planet or natural satellite, which is chemically distinct from the underlying mantle." [https://en.wikipedia.org/wiki/Crust_(geology)]
comment: This class is meant to be applicable accross planets. Earth's crust would be an instance.
synonym: "crust" BROAD []
is_a: ENVO:01000639 ! planetary structural layer

[Term]
id: ENVO:01000639
name: planetary structural layer
namespace: ENVO
def: "A planetary structural layer is laminar part of a terrestrial planet or other rocky body large enough to have differentiation by density. Planetary layers have differing physicochemical properties and composition." []
is_a: ENVO:01000281 ! layer
relationship: part_of ENVO:01000800 ! planet
property_value: IAO:0000116 "Label should be improved to match definition." xsd:string

[Term]
id: ENVO:01000646
name: lithosphere
namespace: ENVO
def: "A lithosphere is the outermost shell of a terrestrial-type planet or natural satellite that is defined by its rigid mechanical properties." [https://en.wikipedia.org/wiki/Lithosphere]
comment: Earth's lithosphere includes the crust and uppermost mantle.
is_a: ENVO:01000639 ! planetary structural layer
relationship: composed_primarily_of ENVO:01000814 ! solid environmental material
relationship: has_part ENVO:01000638 ! planetary crust

[Term]
id: ENVO:01000799
name: astronomical body
namespace: ENVO
def: "An object which is naturally occuring, bound together by gravitational or electromagnetic forces, and surrounded by space." [https://en.wikipedia.org/wiki/Astronomical_object]
comment: Astronomical bodies are usually cohesive, thus the use of the term 'object' sensu BFO 'object'.
subset: envoAstro
synonym: "celestial body" RELATED []
is_a: ENVO:01000804 ! astronomical object

[Term]
id: ENVO:01000800
name: planet
namespace: ENVO
def: "A planet is an astronomical body orbiting a star or stellar remnant that is massive enough to be rounded by its own gravity, is not massive enough to cause thermonuclear fusion, and has cleared its neighbouring region of planetesimals." [http://solarsystem.nasa.gov/planets/whatisaplanet, https://en.wikipedia.org/wiki/Planet]
comment: Considerable debate on the definition of planet exists.
subset: envoAstro
subset: envoPolar
is_a: ENVO:01000799 ! astronomical body

[Term]
id: ENVO:01000804
name: astronomical object
namespace: ENVO
def: "An object which is composed of one or more gravitationally bound structures that are associated with a position in space." [https://en.wikipedia.org/wiki/Astronomical_object]
comment: If there is only one astronomical body involved, this class is equivalent to ENVO:01000799. This may be problematic with reasoning, but it seems to be true to the rather fuzzy definitions found thus far.
subset: envoAstro
synonym: "celestial object" RELATED []
relationship: has_part ENVO:01000799 ! astronomical body
relationship: has_quality ENVO:01001164 ! geodiversity
relationship: surrounded_by ENVO:01000637 ! outer space

[Term]
id: ENVO:01000813
name: astronomical body part
namespace: ENVO
def: "A material part of an astronomical body." []
comment: Material parts of astronomical bodies generally have boundaries formed by discontinuities in qualities, composition, or other physical characterisitcs. These boundaries are sometimes sharp, and sometimes diffuse, with different classification systems and communities declaring varying thresholds (e.g. for where a shoreline, forest, or other entity begins and ends). However, some boundaries are declared by fiat - that is, by arbitrary human convention or decree - particularly by regulatory or other authorities and communities of practice. The classes in this hierarchy attempt to offer generalisable definitions that allow multiple classfiication systems to map to and interoperate through. If desired, we can create classes that declare thresholds used by a given authority or community under the more generic ones, annotated with source information.
subset: envoAstro
subset: envoPolar
relationship: part_of ENVO:01000799 ! astronomical body
property_value: IAO:0000116 "Also note that some astronomical body parts (ABPs) may have fiat boundaries: if there's strong debate about where an ABP begins or ends (over and above fuzzy boundaries), with different official classifications setting different thresholds or limits, axiomatise the class with fiat boundaries of the appropriate dimension." xsd:string
property_value: IAO:0000116 "Note that material entities may have immaterial entities (e.g. sites) as parts." xsd:string
property_value: IAO:0000116 "This class includes material parts of astronomical bodies. Immaterial parts, such as magnetospheres, are represented as sites under the influence of magnetic fields.Please post countercases in the ENVO tracker for revision of this hierarchy if needed." xsd:string

[Term]
id: ENVO:01000814
name: solid environmental material
namespace: ENVO
def: "An environmental material which is in a solid state." []
comment: This is a defined class: its subclasses will not be asserted, but filled by inference.
is_a: ENVO:00010483 ! environmental material

[Term]
id: ENVO:01000815
name: liquid environmental material
namespace: ENVO
def: "An environmental material which is in a liquid state." []
comment: This is a defined class: most of its subclasses will not be asserted, but filled by inference.
subset: envoPolar
is_a: ENVO:02000140 ! fluid environmental material

[Term]
id: ENVO:01000817
name: biosphere
namespace: ENVO
def: "An astronomical body part which includes all the living entities within the gravitational sphere of influence of that body, as well as the non-living and dead entities with which they interact." [http://www.biology-online.org/dictionary/Biosphere, https://en.wikipedia.org/wiki/Biosphere]
comment: The gravitational sphere of influence referenced in this class' definition is the Hill sphere: a region in which an object dominates the attraction of satellites despite gravitational perturbations.
subset: envoAstro
subset: envoPolar
is_a: ENVO:01000813 ! astronomical body part
property_value: IAO:0000116 "Whether this class should be grouped with classes such as \"hydrosphere\" and \"cryosphere\" requires some discussion." xsd:string

[Term]
id: ENVO:01000819
name: hydrosphere
namespace: ENVO
def: "An astronomical body part which is composed of the combined mass of water found on, under, and over the surface of a planet." [https://en.wikipedia.org/wiki/Hydrosphere]
comment: This is a very broad and, in practice, poorly defined term. Please consider using or requesting a more specific class.
subset: envoAstro
subset: envoPolar
is_a: ENVO:01001477 ! liquid astronomical body part
relationship: composed_primarily_of ENVO:00002006 ! liquid water

[Term]
id: ENVO:01000820
name: pedosphere
namespace: ENVO
def: "An astronomical body part which is composed of soil, subject to soil formation processes, and found on the surface of a lithosphere." [https://en.wikipedia.org/wiki/Pedosphere]
comment: This is a very broad and, in practice, poorly defined term. Please consider using or requesting a more specific class.
subset: envoAstro
is_a: ENVO:01000813 ! astronomical body part
relationship: composed_primarily_of ENVO:00001998 ! soil
relationship: overlaps ENVO:01000267 ! atmosphere
relationship: overlaps ENVO:01000646 ! lithosphere
relationship: overlaps ENVO:01000817 ! biosphere
relationship: overlaps ENVO:01000819 ! hydrosphere

[Term]
id: ENVO:01000999
name: rhizosphere environment
namespace: ENVO
def: "An environmental system determined by the presence of a plant rhizosphere." []
subset: envoEmpo
subset: envoOmics
is_a: ENVO:01000254 ! environmental system
relationship: overlaps ENVO:00005801 ! rhizosphere
relationship: overlaps ENVO:01001001 ! plant-associated environment
property_value: IAO:0000118 "Plant rhizosphere" xsd:string {comment="http://press.igsb.anl.gov/earthmicrobiome/protocols-and-standards/emp-ontology-empo/"}

[Term]
id: ENVO:01001000
name: environmental system determined by an organism
namespace: ENVO
def: "An environmental system which is determined by a living organism." []
subset: envoEmpo
subset: envoOmics
synonym: "host-associated environment" RELATED []
is_a: ENVO:01000254 ! environmental system

[Term]
id: ENVO:01001001
name: plant-associated environment
namespace: ENVO
def: "An environmental system determined by a green plant." []
subset: envoEmpo
subset: envoOmics
synonym: "plant environment" BROAD []
synonym: "Viridiplantae-associated environment" EXACT []
property_value: IAO:0000118 "Plant" xsd:string {xref="http://press.igsb.anl.gov/earthmicrobiome/protocols-and-standards/emp-ontology-empo/"}

[Term]
id: ENVO:01001002
name: animal-associated environment
namespace: ENVO
def: "An environmental system determined by an animal." []
subset: envoEmpo
subset: envoMeo
subset: envoOmics
synonym: "animal environment" BROAD []
synonym: "Metazoan-associated environment" EXACT []
property_value: IAO:0000118 "Animal" xsd:string {xref="http://press.igsb.anl.gov/earthmicrobiome/protocols-and-standards/emp-ontology-empo/"}

[Term]
id: ENVO:01001028
name: sediment permeated by freshwater
namespace: ENVO
def: "Sediment which has its porespace filled by water which has very low levels of sodium chloride and/or other salts." []
comment: We do not specify numeric thresholds for saline vs. non-saline here, as this is variable. Consider specifying this on the information and/or data layer for your purposes. If you require an ENVO class with a fixed threshold, please request one using our issue tracker.
subset: envoEmpo
subset: envoOmics
is_a: ENVO:00002007 ! sediment
relationship: surrounded_by ENVO:00002011 ! fresh water

[Term]
id: ENVO:01001029
name: fecal environment
namespace: ENVO
def: "An environmental system which has its properties and dynamics determined by feces." []
subset: envoEmpo
subset: envoMeo
subset: envoOmics
is_a: ENVO:01000254 ! environmental system
property_value: IAO:0000118 "Animal distal gut" xsd:string {xref="http://press.igsb.anl.gov/earthmicrobiome/protocols-and-standards/emp-ontology-empo/", comment="The label of this EMPO class is ambiguous, but pers. comm. with L Thompson (http://orcid.org/0000-0002-3911-1280) reveals that this is essentially limited to fecal samples."}

[Term]
id: ENVO:01001030
name: environment determined by a metazoan secretion
namespace: ENVO
def: "An environmental system which has its properties and dynamics determined by a bodily secretion of a metazoan." []
subset: envoEmpo
subset: envoMeo
subset: envoOmics
is_a: ENVO:01000254 ! environmental system
property_value: IAO:0000118 "Animal secretion" xsd:string {xref="http://press.igsb.anl.gov/earthmicrobiome/protocols-and-standards/emp-ontology-empo/"}

[Term]
id: ENVO:01001031
name: environment determined by a plant substance
namespace: ENVO
def: "An environmental system which has its properties and dynamics determined by a substance produced by a plant." []
subset: envoEmpo
subset: envoMeo
subset: envoOmics
is_a: ENVO:01000254 ! environmental system
property_value: IAO:0000118 "Plant secretion" xsd:string {xref="http://press.igsb.anl.gov/earthmicrobiome/protocols-and-standards/emp-ontology-empo/"}

[Term]
id: ENVO:01001032
name: environment determined by a biofilm on a plant surface
namespace: ENVO
def: "An environmental system which has its properties and dynamics determined by a biofilm on the surface of a plant." []
subset: envoEmpo
subset: envoMeo
subset: envoOmics
property_value: IAO:0000118 "Plant surface" xsd:string {xref="http://press.igsb.anl.gov/earthmicrobiome/protocols-and-standards/emp-ontology-empo/"}

[Term]
id: ENVO:01001033
name: digestive tract environment
namespace: ENVO
def: "An environmental system which has its properties and dynamics determined by a digestive tract." []
subset: envoEmpo
subset: envoMeo
subset: envoOmics
is_a: ENVO:2100000 ! anatomical entity environment
property_value: IAO:0000118 "Animal proximal gut" xsd:string {xref="http://press.igsb.anl.gov/earthmicrobiome/protocols-and-standards/emp-ontology-empo/", comment="This EMPO class includes examples of microbial environments determined by the \"gut intestine, gizzard, crop, lumen, [and] mucosa\"."}

[Term]
id: ENVO:01001034
name: environment determined by a biofilm on an animal surface
namespace: ENVO
def: "An environmental system which has its properties and dynamics determined by a biofilm on the surface of a animal." []
subset: envoEmpo
subset: envoMeo
subset: envoOmics
property_value: IAO:0000118 "Animal surface" xsd:string {xref="http://press.igsb.anl.gov/earthmicrobiome/protocols-and-standards/emp-ontology-empo/"}

[Term]
id: ENVO:01001035
name: environment determined by a biofilm on a fungal surface
namespace: ENVO
def: "An environmental system which has its properties and dynamics determined by a biofilm on the surface of a fungus." []
subset: envoEmpo
subset: envoMeo
subset: envoOmics
property_value: IAO:0000118 "Fungus surface" xsd:string {xref="http://press.igsb.anl.gov/earthmicrobiome/protocols-and-standards/emp-ontology-empo/"}

[Term]
id: ENVO:01001036
name: sediment permeated by saline water
namespace: ENVO
def: "Sediment which has its porespace filled by water with increased levels of sodium chloride and other salts." []
comment: We do not specify numeric thresholds for saline vs. non-saline here, as this is variable. Consider specifying this on the information and/or data layer for your purposes. If you require an ENVO class with a fixed threshold, please request one using our issue tracker.
subset: ENVO:03605026
subset: envoEmpo
subset: envoOmics
is_a: ENVO:00002007 ! sediment
relationship: surrounded_by ENVO:00002010 ! saline water

[Term]
id: ENVO:01001041
name: fungi-associated environment
namespace: ENVO
def: "An environmental system determined by a fungal structure." []
subset: envoEmpo
subset: envoMeo
subset: envoOmics
synonym: "fungus environment" BROAD []
synonym: "fungus-associated environment" EXACT []
property_value: IAO:0000118 "Fungus" xsd:string {xref="http://press.igsb.anl.gov/earthmicrobiome/protocols-and-standards/emp-ontology-empo/"}

[Term]
id: ENVO:01001042
name: sterile water environment
namespace: ENVO
def: "An environmental system which has its properties and dynamics determined by sterile water." []
comment: This term can be understood as a negative experimental control primarily composed of sterile water. The quantity of sterile water used may be contaminated; to express pure sterile water, please use http://purl.obolibrary.org/obo/ENVO_00005791
subset: envoEmpo
subset: envoOmics
is_a: ENVO:01000317 ! aquatic environment
intersection_of: ENVO:01000317 ! aquatic environment
intersection_of: determined_by ENVO:00005791 ! sterile water
relationship: composed_primarily_of ENVO:00005791 ! sterile water
property_value: IAO:0000118 "Negative" xsd:string {xref="http://press.igsb.anl.gov/earthmicrobiome/protocols-and-standards/emp-ontology-empo/"}

[Term]
id: ENVO:01001043
name: hypersaline water environment
namespace: ENVO
def: "An environmental system which has its properties and dynamics determined by hypersaline water." []
subset: envoEmpo
subset: envoOmics
subset: envoPolar
is_a: ENVO:01000307 ! saline water environment
property_value: IAO:0000118 "Hypersaline (saline)" xsd:string {xref="http://press.igsb.anl.gov/earthmicrobiome/protocols-and-standards/emp-ontology-empo/", comment="Examples inlcude water from hypersaline samples or brines (>50 psu)"}

[Term]
id: ENVO:01001044
name: soil environment
namespace: ENVO
def: "An environmental system which has its properties and dynamics determined by soil." []
subset: envoEmpo
subset: envoOmics
is_a: ENVO:01000254 ! environmental system
intersection_of: ENVO:01000254 ! environmental system
intersection_of: determined_by ENVO:00001998 ! soil
property_value: IAO:0000118 "Soil (non-saline)" xsd:string {xref="http://press.igsb.anl.gov/earthmicrobiome/protocols-and-standards/emp-ontology-empo/"}

[Term]
id: ENVO:01001046
name: planetary subsurface environment
namespace: ENVO
def: "An environmental system which has its properties and dynamics determined by the subsurface zone of a planet." []
subset: envoEmpo
subset: envoMeo
subset: envoOmics
is_a: ENVO:01000254 ! environmental system

[Term]
id: ENVO:01001047
name: non-saline planetary subsurface environment
namespace: ENVO
def: "An environmental system which has its properties and dynamics determined by those parts of a planetary subsurface zone which are not saline." []
subset: envoEmpo
subset: envoMeo
subset: envoOmics
is_a: ENVO:01001046 ! planetary subsurface environment
property_value: IAO:0000118 "Subsurface (non-saline)" xsd:string {xref="http://press.igsb.anl.gov/earthmicrobiome/protocols-and-standards/emp-ontology-empo/"}

[Term]
id: ENVO:01001048
name: sediment environment
namespace: ENVO
def: "An environmental system which has its properties and dynamics determined by sediment." []
subset: envoEmpo
subset: envoOmics
is_a: ENVO:01000254 ! environmental system
intersection_of: ENVO:01000254 ! environmental system
intersection_of: determined_by ENVO:00002007 ! sediment

[Term]
id: ENVO:01001049
name: non-saline sediment environment
namespace: ENVO
def: "An environmental system which has its properties and dynamics determined by sediment permeated by non-saline water." []
subset: envoEmpo
subset: envoOmics
is_a: ENVO:01001048 ! sediment environment
intersection_of: ENVO:01001048 ! sediment environment
intersection_of: determined_by ENVO:01001028 ! sediment permeated by freshwater
property_value: IAO:0000118 "Sediment (non-saline)" xsd:string {xref="http://press.igsb.anl.gov/earthmicrobiome/protocols-and-standards/emp-ontology-empo/"}

[Term]
id: ENVO:01001050
name: saline sediment environment
namespace: ENVO
def: "An environmental system which has its properties and dynamics determined by sediment permeated by saline water." []
subset: envoEmpo
subset: envoOmics
is_a: ENVO:01001048 ! sediment environment
intersection_of: ENVO:01001048 ! sediment environment
intersection_of: determined_by ENVO:01001036 ! sediment permeated by saline water
property_value: IAO:0000118 "Sediment (saline)" xsd:string {xref="http://press.igsb.anl.gov/earthmicrobiome/protocols-and-standards/emp-ontology-empo/"}

[Term]
id: ENVO:01001051
name: environment determined by a biofilm on a non-saline surface
namespace: ENVO
def: "An environmental system which has its properties and dynamics determined by a biofilm on a surface which is exposed to non-saline materials." []
subset: envoEmpo
subset: envoMeo
subset: envoOmics
property_value: IAO:0000118 "Surface (non-saline)" xsd:string {xref="http://press.igsb.anl.gov/earthmicrobiome/protocols-and-standards/emp-ontology-empo/"}

[Term]
id: ENVO:01001052
name: aerosol environment
namespace: ENVO
def: "An environmental system which has its properties and dynamics determined by an aerosol." []
subset: envoEmpo
subset: envoOmics
is_a: ENVO:01000254 ! environmental system

[Term]
id: ENVO:01001053
name: saline aerosol environment
namespace: ENVO
def: "An environmental system which has its properties and dynamics determined by a saline aerosol." []
subset: envoEmpo
subset: envoOmics
is_a: ENVO:01001052 ! aerosol environment
property_value: IAO:0000118 "Aerosol (saline)" xsd:string {xref="http://press.igsb.anl.gov/earthmicrobiome/protocols-and-standards/emp-ontology-empo/", comment="seaspray or other aerosolized saline material (>5 psu)"}

[Term]
id: ENVO:01001054
name: non-saline aerosol environment
namespace: ENVO
def: "An environmental system which has its properties and dynamics determined by an aerosol with a low concentration of dissolved solutes." []
subset: envoEmpo
subset: envoOmics
is_a: ENVO:01001052 ! aerosol environment
property_value: IAO:0000118 "Aerosol (non-saline)" xsd:string {xref="http://press.igsb.anl.gov/earthmicrobiome/protocols-and-standards/emp-ontology-empo/", comment="aerosolized dust or liquid"}

[Term]
id: ENVO:01001055
name: environment associated with an animal part or small animal
namespace: ENVO
def: "An environmental system determined by part of a living or dead animal, or a whole small animal." []
subset: envoEmpo
subset: envoMeo
subset: envoOmics
is_a: ENVO:01001110 ! ecosystem
property_value: IAO:0000118 "Animal corpus" xsd:string {xref="http://press.igsb.anl.gov/earthmicrobiome/protocols-and-standards/emp-ontology-empo/"}

[Term]
id: ENVO:01001056
name: environment determined by a biofilm on a saline surface
namespace: ENVO
def: "An environmental system which has its properties and dynamics determined by a biofilm on a surface which is exposed to saline materials." []
subset: envoEmpo
subset: envoMeo
subset: envoOmics
property_value: IAO:0000118 "Surface (saline)" xsd:string {xref="http://press.igsb.anl.gov/earthmicrobiome/protocols-and-standards/emp-ontology-empo/"}

[Term]
id: ENVO:01001057
name: environment associated with a plant part or small plant
namespace: ENVO
def: "An environmental system determined by part of a living or dead plant, or a whole small plant." []
subset: envoEmpo
subset: envoMeo
subset: envoOmics
property_value: IAO:0000118 "Plant corpus" xsd:string {xref="http://press.igsb.anl.gov/earthmicrobiome/protocols-and-standards/emp-ontology-empo/"}

[Term]
id: ENVO:01001058
name: environment associated with a fungal tissue
namespace: ENVO
def: "An environmental system determined by part of a living or dead fungus." []
subset: envoEmpo
subset: envoMeo
subset: envoOmics
property_value: IAO:0000118 "Fungus corpus" xsd:string {xref="http://press.igsb.anl.gov/earthmicrobiome/protocols-and-standards/emp-ontology-empo/"}

[Term]
id: ENVO:01001059
name: mock community culture
namespace: ENVO
def: "A cell culture which is composed of a microbial community of known composition." []
comment: Mock communities are typically used as positive controls in experiments.
subset: envoEmpo
subset: envoOmics
is_a: ENVO:02000008 ! cell culture
property_value: IAO:0000118 "Mock community" xsd:string {xref="http://press.igsb.anl.gov/earthmicrobiome/protocols-and-standards/emp-ontology-empo/"}

[Term]
id: ENVO:01001060
name: single strain cell culture
namespace: ENVO
def: "A cell culture which is composed of a single population of bacterial or archaeal cells." []
subset: envoEmpo
subset: envoOmics
is_a: ENVO:02000008 ! cell culture
property_value: IAO:0000118 "Single strain" xsd:string {xref="http://press.igsb.anl.gov/earthmicrobiome/protocols-and-standards/emp-ontology-empo/"}

[Term]
id: ENVO:01001110
name: ecosystem
namespace: ENVO
def: "An environmental system which includes both living and non-living components." [https://en.wikipedia.org/wiki/Ecosystem]
comment: This class will be primarily filled by inference, any environmental system which necessarily includes living parts should be autoclassified here.
xref: LTER:173 {xref="https://vocab.lternet.edu/vocab/vocab/index.php?tema=173&/ecosystems"}
is_a: ENVO:01000254 ! environmental system

[Term]
id: ENVO:01001164
name: geodiversity
namespace: ENVO
def: "A quality which inheres in a astronomical body or astronomical body part by virtue of the variation in its material composition, participation in geological processes, and the variation in is land- and hydroforms." [https://en.wikipedia.org/wiki/Geodiversity]
comment: Materials which are usually assessed when appraising geodiversity include minerals, rocks, sediments, fossils, soils and water. Landforms factored into geodiversity metrics typically include folds, faults, and other expressions of morphology or relations between units of earth material. Natural processes that are included in measures of geodiversity are those which either maintain or change materials or geoforms, including tectonics, sediment transport, and pedogenesis. Geodiversity does not usually factor in anthropogenic entities. {xref=""}

[Term]
id: ENVO:01001176
name: environment associated with an aquatic invertebrate
namespace: ENVO
def: "An environment which has its properties and composition largely determined by the presence of a metazoan which lacks a vetebral column and which has a habitat that is found in an aquatic environmental system." []
subset: envoMeo
subset: envoOmics
xref: http://purl.jp/bio/11/meo/MEO_0000871 {comment="Not currently live, may need to be switched to alternative PURLs."}

[Term]
id: ENVO:01001477
name: liquid astronomical body part
namespace: ENVO
def: "A part of an astronomical body which is primarily composed of liquid material." []
is_a: ENVO:01001479 ! fluid astronomical body part
intersection_of: ENVO:01001479 ! fluid astronomical body part
intersection_of: composed_primarily_of ENVO:01000815 ! liquid environmental material
created_by: https://orcid.org/0000-0002-4366-3088

[Term]
id: ENVO:01001479
name: fluid astronomical body part
namespace: ENVO
def: "A part of an astronomical body which is primarily composed of fluid." [https://en.wikipedia.org/wiki/Fluid]
is_a: ENVO:01000813 ! astronomical body part
intersection_of: ENVO:01000813 ! astronomical body part
intersection_of: composed_primarily_of ENVO:02000140 ! fluid environmental material
created_by: https://orcid.org/0000-0002-4366-3088
creation_date: 2018-10-04T13:59:22Z

[Term]
id: ENVO:01001678
name: fluid layer
namespace: ENVO
def: "A layer which is composed primarily of some fluid." []
is_a: ENVO:01000281 ! layer
property_value: http://purl.org/dc/elements/1.1/creator https://orcid.org/0000-0002-4366-3088
property_value: http://purl.org/dc/elements/1.1/date 2019-07-22T17:35:08Z xsd:dateTime

[Term]
id: ENVO:01001686
name: mass of environmental material
namespace: ENVO
def: "An object which is composed primarily of an environmental material" []
comment: This class and its subclasses refer to objects that are discrete accumulations of environmental materials, generally primarily composed of one or a few main material types.
property_value: http://purl.org/dc/elements/1.1/creator https://orcid.org/0000-0002-4366-3088
property_value: http://purl.org/dc/elements/1.1/date 2019-08-20T09:38:29Z xsd:dateTime

[Term]
id: ENVO:01001687
name: mass of solid material
namespace: ENVO
def: "An mass of environmental material which is composed primarily of a solid environmental material" []
comment: This class and its subclasses refer to objects that are discrete accumulations of environmental materials, generally primarily composed of one or a few main material types.
is_a: ENVO:01001686 ! mass of environmental material
intersection_of: ENVO:01001686 ! mass of environmental material
intersection_of: composed_primarily_of ENVO:01000814 ! solid environmental material
property_value: http://purl.org/dc/elements/1.1/creator https://orcid.org/0000-0002-4366-3088
property_value: http://purl.org/dc/elements/1.1/date 2019-08-20T09:41:27Z xsd:dateTime

[Term]
id: ENVO:01003001
name: water-holding capacity
namespace: ENVO
def: "A disposition of a material entity which is realised when it is saturated with liquid water." []
property_value: http://purl.org/dc/elements/1.1/creator https://orcid.org/0000-0002-4366-3088

[Term]
id: ENVO:01003002
name: particle
namespace: ENVO
def: "A mass of solid material which is either 1) a minute fragment of a larger mass or 2) one of a collection of small masses composing an aggregate." [https://en.wiktionary.org/wiki/particle]
synonym: "grain" RELATED []
is_a: ENVO:01001687 ! mass of solid material
relationship: part_of ENVO:01000060

[Term]
id: ENVO:01003003
name: particle of clay
namespace: ENVO
def: "A particle which 1) is composed primarily of hydrous aluminium phyllosilicate minerals, in turn composed of aluminium and silicon ions bonded into tiny, thin plates by interconnecting oxygen and hydroxide ions, and 2) is or was part of a portion of clay." [https://en.wikipedia.org/wiki/Clay#Properties]
comment: The distinction between silt and clay varies by discipline. Geologists and soil scientists usually consider the separation to occur at a particle size of 2 μm (clays being finer than silts), sedimentologists often use 4–5 μm, and colloid chemists use 1 μm. Geotechnical engineers distinguish between silts and clays based on the plasticity properties of the soil, as measured by the soils' Atterberg limits. ISO 14688 grades clay particles as being smaller than 2 μm and silt particles as being larger. Mixtures of sand, silt and less than 40% clay are called loam. {xref="Properties"}
synonym: "clay particle" EXACT []
is_a: ENVO:01003002 ! particle

[Term]
id: ENVO:02000008
name: cell culture
namespace: ENVO
def: "A cell culture is a growth of cells in vitro in an artificial medium for experimental research." [URL:http\://stemcells.nih.gov/StemCells/Templates/StemCellContentPage.aspx?NRMODE=Published&NRNODEGUID=%7b3C35BAB6-0FE6-4C4E-95F2-2CB61B58D96D%7d&NRORIGINALURL=%2finfo%2fglossary%2easp&NRCACHEHINT=NoModifyGuest#cellculture]
xref: https://en.wikipedia.org/wiki/Cell_culture
is_a: ENVO:01000155 ! organic material

[Term]
id: ENVO:02000140
name: fluid environmental material
namespace: ENVO
def: "An environmental material which is unable to resist shear forces and continuously deforms when subject to them." [https://en.wikipedia.org/wiki/Fluid, https://github.com/EnvironmentOntology/envo/issues/940]
synonym: "fluid" NARROW []
is_a: ENVO:00010483 ! environmental material

[Term]
id: ENVO:06105304
name: water-holding capacity of soil
namespace: ENVO
def: "Water-holding capacity which inheres in some soil." [https://www.canr.msu.edu/news/why_is_soil_water_holding_capacity_important]
synonym: "soil water-holding capacity" EXACT []
is_a: ENVO:01003001 ! water-holding capacity
relationship: characteristic_of ENVO:00001998 ! soil
property_value: http://purl.org/dc/elements/1.1/creator http://orcid.org/0000-0002-8461-9745
property_value: http://purl.org/dc/terms/creator https://orcid.org/0000-0001-6284-4821

[Term]
id: ENVO:2100000
name: anatomical entity environment
namespace: ENVO
def: "An environment which is determined by an anatomical entity." []
is_a: ENVO:01000254 ! environmental system
relationship: part_of ENVO:01001000 ! environmental system determined by an organism

[Typedef]
id: adjacent_to
namespace: ENVO
xref: RO:0002220

[Typedef]
id: attached_to
namespace: ENVO
xref: RO:0002371

[Typedef]
id: bounding_layer_of
namespace: ENVO
xref: RO:0002007

[Typedef]
id: capable_of
namespace: ENVO
xref: RO:0002215

[Typedef]
id: causal_agent_in_process
namespace: ENVO
xref: RO:0002500

[Typedef]
id: causally_downstream_of_or_within
namespace: ENVO
xref: RO:0002427

[Typedef]
id: causally_upstream_of
namespace: ENVO
xref: RO:0002411

[Typedef]
id: causally_upstream_of_or_within
namespace: ENVO
xref: RO:0002418

[Typedef]
id: characteristic_of
namespace: ENVO
xref: RO:0000052

[Typedef]
id: characteristic_of_part_of
namespace: ENVO
xref: RO:0002314

[Typedef]
id: composed_primarily_of
namespace: ENVO
xref: RO:0002473

[Typedef]
id: concretizes
namespace: ENVO
xref: RO:0000059

[Typedef]
id: connected_to
namespace: ENVO
xref: RO:0002170

[Typedef]
id: connects
name: connects
namespace: ENVO
xref: RO:0002176

[Typedef]
id: contains_process
namespace: ENVO
xref: BFO:0000067

[Typedef]
id: continuous_with
namespace: ENVO
xref: RO:0002150

[Typedef]
id: derives_from
namespace: ENVO
xref: RO:0001000
is_a: derives_from_part_of ! derives from part of

[Typedef]
id: derives_from_part_of
name: derives from part of
namespace: ENVO
def: "A relation between two distinct material entities, the new entity and the old entity, in which the new entity begins to exist through the separation or transformation of a part of the old entity, and the new entity inherits a significant portion of the matter belonging to that part of the old entity." []
xref: ENVO:01003004

[Typedef]
id: derives_into
namespace: ENVO
xref: RO:0001001

[Typedef]
id: determined_by
namespace: ENVO
xref: RO:0002507

[Typedef]
id: determined_by_part_of
namespace: ENVO
xref: RO:0002509

[Typedef]
id: disconnected_from
name: disconnected_from
namespace: ENVO
def: "A is disconnected_from B if they have no parts in common." [https://orcid.org/0000-0002-6601-2165]
synonym: "non_overlapping_with" EXACT []
expand_assertion_to: "Class: <http://www.w3.org/2002/07/owl#Nothing> EquivalentTo: (BFO_0000050 some ?X) and (BFO_0000050 some ?Y)" []
is_metadata_tag: true
is_class_level: true

[Typedef]
id: distributary_of
namespace: ENVO
xref: RO:0002377

[Typedef]
id: during_which_ends
namespace: ENVO
xref: RO:0002084

[Typedef]
id: during_which_starts
namespace: ENVO
xref: RO:0002088

[Typedef]
id: ends
namespace: ENVO
xref: RO:0002229

[Typedef]
id: formed_as_result_of
namespace: ENVO
xref: RO:0002354

[Typedef]
id: generates
name: generates
namespace: ENVO
def: "A relation between a process and a disposition such that the existence of the disposition is caused by the execution of the process." []
xref: ENVO:2000036
property_value: IAO:0000116 "Consider ceding to RO" xsd:string
created_by: https://orcid.org/0000-0002-6601-2165
creation_date: 2018-11-03T20:58:13Z

[Typedef]
id: has_characteristic
namespace: ENVO
xref: RO:0000053

[Typedef]
id: has_component
namespace: ENVO
xref: RO:0002180

[Typedef]
id: has_disposition
namespace: ENVO
xref: RO:0000091

[Typedef]
id: has_end_location
namespace: ENVO
xref: RO:0002232

[Typedef]
id: has_function
namespace: ENVO
xref: RO:0000085

[Typedef]
id: has_habitat
name: has habitat
namespace: ENVO
xref: RO:0002303

[Typedef]
id: has_increased_levels_of
name: has increased levels of
namespace: ENVO
def: "A has part relationship between a whole and a part, where the number of parts present in the whole is higher than in comparable entities." []
comment: This relation is present in ENVO to support compositional classes such as "X-enriched soil". These will later be formalized, and a different relation from RO may be chosen.
xref: ENVO:02000200
property_value: seeAlso https://github.com/EnvironmentOntology/envo/issues/1380
is_a: has_component

[Typedef]
id: has_input
namespace: ENVO
xref: RO:0002233

[Typedef]
id: has_member
namespace: ENVO
xref: RO:0002351

[Typedef]
id: has_output
namespace: ENVO
xref: RO:0002234

[Typedef]
id: has_part
namespace: ENVO
xref: BFO:0000051

[Typedef]
id: has_part_that_occurs_in
namespace: ENVO
xref: RO:0002479

[Typedef]
id: has_participant
namespace: ENVO
xref: RO:0000057

[Typedef]
id: has_quality
namespace: ENVO
xref: RO:0000086

[Typedef]
id: has_role
namespace: ENVO
xref: RO:0000087

[Typedef]
id: input_of
namespace: ENVO
xref: RO:0002352

[Typedef]
id: involved_in
namespace: ENVO
xref: RO:0002331

[Typedef]
id: involved_in_negative_regulation_of
namespace: ENVO
xref: RO:0002430

[Typedef]
id: located_in
namespace: ENVO
xref: RO:0001025

[Typedef]
id: location_of
namespace: ENVO
xref: RO:0001015

[Typedef]
id: member_of
namespace: ENVO
xref: RO:0002350

[Typedef]
id: negatively_regulates
namespace: ENVO
xref: RO:0002212

[Typedef]
id: obsolete_contains
namespace: ENVO
xref: RO:0001019

[Typedef]
id: obsolete_determined_by
name: obsolete determined by
namespace: ENVO
xref: ENVO:2100001
is_obsolete: true

[Typedef]
id: obsolete_determined_by_part_of
name: obsolete determined by part of
namespace: ENVO
xref: ENVO:2100007
is_obsolete: true

[Typedef]
id: occurs_in
namespace: ENVO
xref: BFO:0000066

[Typedef]
id: output_of
namespace: ENVO
xref: RO:0002353

[Typedef]
id: overlaps
namespace: ENVO
xref: RO:0002131

[Typedef]
id: part_of
namespace: ENVO
xref: BFO:0000050

[Typedef]
id: partially_overlaps
namespace: ENVO
xref: RO:0002151

[Typedef]
id: partially_surrounded_by
name: partially_surrounded_by
namespace: ENVO
def: "x partially_surrounded_by y if and only if (1) x is adjacent to y and for the region r that is adjacent to x, r partially overlaps y (2) the shared boundary between x and y occupies  a non-trivial proportion of the outermost boundary of x" []
comment: Definition modified from 'surrounded by'.
xref: ENVO:01001307
property_value: IAO:0000112 "A duck swimming in a pond is partially surrounded by air and partially surrounded by water." xsd:string

[Typedef]
id: participates_in
namespace: ENVO
xref: RO:0000056

[Typedef]
id: preceded_by
namespace: ENVO
xref: BFO:0000062

[Typedef]
id: precedes
namespace: ENVO
xref: BFO:0000063

[Typedef]
id: process_has_causal_agent
namespace: ENVO
xref: RO:0002608

[Typedef]
id: realized_in
namespace: ENVO
xref: BFO:0000054

[Typedef]
id: realizes
namespace: ENVO
xref: BFO:0000055

[Typedef]
id: regulates_(processual)
name: regulates (processual)
namespace: ENVO
xref: RO:0002211

[Typedef]
id: results_in_expansion_of
name: results in expansion of
namespace: ENVO
def: "A process, p, results in the expansion of a material entity, m, if the spatial extent of m is increased as a result of participating in p." []
xref: ENVO:02500016
property_value: IAO:0000112 "Afforestation results in the expansion of a forest." xsd:string

[Typedef]
id: results_in_formation_of_anatomical_entity
namespace: ENVO
xref: RO:0002297

[Typedef]
id: results_in_proliferation_of
name: results in proliferation of
namespace: ENVO
comment: To be ceded to RO
xref: ENVO:02500020

[Typedef]
id: results_in_transformation_into
name: results in transformation into
namespace: ENVO
xref: ENVO:02500006

[Typedef]
id: starts_during
namespace: ENVO
xref: RO:0002091

[Typedef]
id: surrounded_by
name: surrounded by
namespace: ENVO
xref: RO:0002219

[Typedef]
id: towards
namespace: ENVO
xref: RO:0002503

[Typedef]
id: tributary_of
namespace: ENVO
xref: RO:0002376

