format-version: 1.2
data-version: envo/releases/2023-02-13/subsets/envoCesab.owl
subsetdef: disposition_slim "Disposition slim"
subsetdef: environmental_hazards "environmental_hazards"
subsetdef: EnvO-Lite-GSC "EnvO-Lite-GSC"
subsetdef: envoANZSoil "envoANZSoil"
subsetdef: envoAstro "envoAstro"
subsetdef: envoAtmo "envoAtmo"
subsetdef: envoCesab "envoCesab"
subsetdef: envoCmecs "envoCmecs"
subsetdef: envoEmpo "envoEmpo"
subsetdef: envoEOVs "envoEOVs"
subsetdef: envoMarine "envoMarine"
subsetdef: envoMeo "envoMeo"
subsetdef: envoNceas "envoNceas"
subsetdef: envoOmics "envoOmics"
subsetdef: envoPlastics "envoPlastics"
subsetdef: envoPolar "envoPolar"
subsetdef: mpath_slim "Pathology slim"
subsetdef: nlcd2011 "nlcd2011"
subsetdef: relational_slim "Relational slim: types of quality that require an additional entity in order to exist"
subsetdef: ro-eco "ro-eco"
subsetdef: scalar_slim "Scalar slim"
subsetdef: value_slim "Value slim"
subsetdef: wwfBiome "wwfBiome"
synonymtypedef: PLURAL "plurals"
ontology: envo/subsets/envoCesab
property_value: owl:versionInfo "2023-02-13" xsd:string

[Term]
id: ENVO:00000191
name: solid astronomical body part
namespace: ENVO
def: "A part of an astronomical body which is primarily composed of a continuous volume of solid material, shaped by one or more environmental processes." [https://en.wikipedia.org/wiki/Landform]
synonym: "geological feature" RELATED [ADL:FTT]
synonym: "landform" RELATED []
synonym: "physiographic feature" RELATED []
xref: EcoLexicon:landform
xref: EcoLexicon:landforms
xref: FTT:754
xref: FTT:96
xref: SWEETRealm:Landform
xref: TGN:21400
xref: TGN:21401
is_a: ENVO:01000813 ! astronomical body part

[Term]
id: ENVO:00000549
name: container of an intermittent water body
namespace: ENVO
def: "A depression which is is periodically filled with water when water supply exceeds evapotranspiration and bed seepage." [MA:ma] {comment="https://orcid.org/0000-0002-4366-3088"}
comment: This was formerly represented as a water body, which would not be valid during dry periods. This class more properly refers to the container of the water body, thusfar always some depression, which periodically contains a water body.
synonym: "intermittent body of water" EXACT [Getty:TGN]
synonym: "intermittent water body" EXACT []
xref: TGN:21198
is_a: ENVO:01001884 ! surface landform
property_value: IAO:0000116 "Despite the relocation from its position under 'water body' and the rewording of the definition, the class was not obsoleted as the entity being referenced is effectively the same." xsd:string

[Term]
id: ENVO:00003074
name: manufactured product
namespace: ENVO
def: "A material entity that has been processed by humans or their technology in any way, including intermediate products as well as final products." [] {comment="https://en.wikipedia.org/wiki/Manufactured_product"}
synonym: "manufactured good" EXACT []
relationship: output_of ENVO:01000993 ! manufacturing process

[Term]
id: ENVO:00010483
name: environmental material
namespace: ENVO
def: "A portion of environmental material is a fiat object part which forms the medium or part of the medium of an environmental system." [DOI:10.1186/2041-1480-4-43, MA:ma, ORCID:0000-0002-4366-3088, URL:http\://ontology.buffalo.edu/smith/articles/niches.html]
comment: Everything under this parent must be a mass noun. All subclasses are to be understood as being composed primarily of the named entity, rather than restricted to that entity. For example, "ENVO:water" is to be understood as "environmental material composed primarly of some CHEBI:water". This class is currently being aligned to the Basic Formal Ontology. Following this alignment, its definition and the definitions of its subclasses will be revised.
synonym: "portion of environmental material" EXACT []

[Term]
id: ENVO:01000637
name: outer space
namespace: ENVO
def: "Outer space is a hard vacuum containing a low density of particles, predominantly a plasma of hydrogen and helium as well as electromagnetic radiation, magnetic fields, neutrinos, dust and cosmic rays that exists between celestial bodies." [https://en.wikipedia.org/wiki/Outer_space]
subset: envoAstro
synonym: "space" BROAD []
is_a: ENVO:00010483 ! environmental material

[Term]
id: ENVO:01000799
name: astronomical body
namespace: ENVO
def: "An object which is naturally occuring, bound together by gravitational or electromagnetic forces, and surrounded by space." [https://en.wikipedia.org/wiki/Astronomical_object]
comment: Astronomical bodies are usually cohesive, thus the use of the term 'object' sensu BFO 'object'.
subset: envoAstro
synonym: "celestial body" RELATED []
is_a: ENVO:01000804 ! astronomical object

[Term]
id: ENVO:01000804
name: astronomical object
namespace: ENVO
def: "An object which is composed of one or more gravitationally bound structures that are associated with a position in space." [https://en.wikipedia.org/wiki/Astronomical_object]
comment: If there is only one astronomical body involved, this class is equivalent to ENVO:01000799. This may be problematic with reasoning, but it seems to be true to the rather fuzzy definitions found thus far.
subset: envoAstro
synonym: "celestial object" RELATED []
relationship: has_part ENVO:01000799 ! astronomical body
relationship: has_quality ENVO:01001164 ! geodiversity
relationship: surrounded_by ENVO:01000637 ! outer space

[Term]
id: ENVO:01000813
name: astronomical body part
namespace: ENVO
def: "A material part of an astronomical body." []
subset: envoAstro
subset: envoPolar
relationship: part_of ENVO:01000799 ! astronomical body

[Term]
id: ENVO:01000975
name: animal trap
namespace: ENVO
def: "A manufactured product which is designed to catch and hold animals." [http://www.thefreedictionary.com/trap]
subset: envoCesab
is_a: ENVO:00003074 ! manufactured product

[Term]
id: ENVO:01000976
name: pitfall trap
namespace: ENVO
def: "An animal trap which consists of a container set flush with the ground such that animals moving along the ground may fall in and be available for examination or collection." [Barber H (1931) Traps for cave-inhabiting insects. J Elisha Mitchell Sci Soc. 46:259–266., Hertz M (1927) Huomioita petokuoriaisten olinpaikoista. Luonnon Ystava. 31:218–222., Mitchell B (1963) Ecology of two carabid beetles\, Bembidion lampros (Herbst) and Trechus quadristriatus (Shrank). J Animal Ecol. 32(3): 377-392.]
subset: envoCesab
is_a: ENVO:01000975 ! animal trap

[Term]
id: ENVO:01000977
name: dry pitfall trap
namespace: ENVO
def: "A pitfall trap in which a glass, plastic, or metal container devoid of accumulations of any liquid is used to contain any animal that falls inside." [http://www.animalethics.org.au/policies-and-guidelines/wildlife-research/pitfall-traps, ISBN:978-0-646-04569-6, ISBN:978-94-009-1225-0]
subset: envoCesab
is_a: ENVO:01000976 ! pitfall trap

[Term]
id: ENVO:01000978
name: wet pitfall trap
namespace: ENVO
def: "A pitfall trap in which the container used to hold trapped animals is filled with a liquid solution formulated to hold, kill, and preserve any animal or animals which falls within it." [http://www.animalethics.org.au/policies-and-guidelines/wildlife-research/pitfall-traps, ISBN:978-0-646-04569-6, ISBN:978-94-009-1225-0]
comment: Aqueous solutions used in these traps include: formalin (10% formaldehyde), alcohol, methylated spirits, trisodium phosphate and picric acid.
subset: envoCesab
is_a: ENVO:01000976 ! pitfall trap

[Term]
id: ENVO:01000979
name: channel of an intermittent river
namespace: ENVO
def: "A channel of an intermittent stream which contains a river when water supply exceeds evapotranspiration and bed seepage." [http://irbas.cesab.org/, https://en.wikipedia.org/wiki/Intermittent_river]
subset: envoCesab
synonym: "ephemeral river" EXACT []
synonym: "intermittent river" EXACT []
synonym: "temporary river" RELATED []
is_a: ENVO:01000980 ! channel of an intermittent stream

[Term]
id: ENVO:01000980
name: channel of an intermittent stream
namespace: ENVO
def: "A channel through which a directional flow of water periodically occurs, ceasing when bed seepage or evapotranspiration exceed the available water supply." [http://encyclopedia2.thefreedictionary.com/Intermittent+stream]
synonym: "intermittent stream" EXACT []
is_a: ENVO:00000549 ! container of an intermittent water body

[Term]
id: ENVO:01000993
name: manufacturing process
namespace: ENVO
def: "A planned process during which raw or recycled materials are transformed into products for use or sale using labour and machines, tools, chemical and biological processing, or formulation." [https://en.wikipedia.org/wiki/Manufacturing]
comment: The term may refer to a range of human activity, from handicraft to high tech, but is most commonly applied to industrial production, in which raw materials are transformed into finished goods on a large scale. {xref="https://en.wikipedia.org/wiki/Manufacturing"}

[Term]
id: ENVO:01001164
name: geodiversity
namespace: ENVO
def: "A quality which inheres in a astronomical body or astronomical body part by virtue of the variation in its material composition, participation in geological processes, and the variation in is land- and hydroforms." [https://en.wikipedia.org/wiki/Geodiversity]
comment: Materials which are usually assessed when appraising geodiversity include minerals, rocks, sediments, fossils, soils and water. Landforms factored into geodiversity metrics typically include folds, faults, and other expressions of morphology or relations between units of earth material. Natural processes that are included in measures of geodiversity are those which either maintain or change materials or geoforms, including tectonics, sediment transport, and pedogenesis. Geodiversity does not usually factor in anthropogenic entities. {xref=""}

[Term]
id: ENVO:01001884
name: surface landform
namespace: ENVO
def: "A landform which occurs on the surface of an astronomical body." []
comment: The usage of "surface" here aligns with that of planetary surface: in contact with the atmosphere or space. The extent of the "surface" can vary. For rocky planets like Earth, astrogeologists consider the crust as the surface.
synonym: "geographic feature" RELATED []
is_a: ENVO:01001886 ! landform
property_value: http://purl.org/dc/elements/1.1/creator https://orcid.org/0000-0002-4366-3088
property_value: http://purl.org/dc/elements/1.1/date 2021-05-15T09:16:23Z xsd:dateTime

[Term]
id: ENVO:01001886
name: landform
namespace: ENVO
def: "A solid astronomical body part which has been formed from and is composed primarily of the matter of that astronomical body." [https://en.wikipedia.org/wiki/Landform]
comment: Landforms may be natural or anthropogenic. This term has often has loose usage when referencing entities which are either subterranean or submerged below water bodies. In some cases, oceans themselves are considered landforms. Here, we have provided subclasses to resolve this ambiguity, but place oceans and other water bodies elsewhere.In later revisions, this hiearchy is likely to be reordered based on the formation processes of the entities within it.
is_a: ENVO:00000191 ! solid astronomical body part
property_value: http://purl.org/dc/elements/1.1/creator https://orcid.org/0000-0002-4366-3088
property_value: http://purl.org/dc/elements/1.1/date 2021-05-15T09:40:37Z xsd:dateTime

[Typedef]
id: adjacent_to
namespace: ENVO
xref: RO:0002220

[Typedef]
id: attached_to
namespace: ENVO
xref: RO:0002371

[Typedef]
id: bounding_layer_of
namespace: ENVO
xref: RO:0002007

[Typedef]
id: capable_of
namespace: ENVO
xref: RO:0002215

[Typedef]
id: causal_agent_in_process
namespace: ENVO
xref: RO:0002500

[Typedef]
id: causally_downstream_of_or_within
namespace: ENVO
xref: RO:0002427

[Typedef]
id: causally_upstream_of
namespace: ENVO
xref: RO:0002411

[Typedef]
id: causally_upstream_of_or_within
namespace: ENVO
xref: RO:0002418

[Typedef]
id: characteristic_of
namespace: ENVO
xref: RO:0000052

[Typedef]
id: characteristic_of_part_of
namespace: ENVO
xref: RO:0002314

[Typedef]
id: composed_primarily_of
namespace: ENVO
xref: RO:0002473

[Typedef]
id: concretizes
namespace: ENVO
xref: RO:0000059

[Typedef]
id: connected_to
namespace: ENVO
xref: RO:0002170

[Typedef]
id: connects
name: connects
namespace: ENVO
xref: RO:0002176

[Typedef]
id: contained_in
namespace: ENVO
xref: RO:0001018

[Typedef]
id: contains
namespace: ENVO
xref: RO:0001019

[Typedef]
id: contains_process
namespace: ENVO
xref: BFO:0000067

[Typedef]
id: continuous_with
namespace: ENVO
xref: RO:0002150

[Typedef]
id: derives_from
namespace: ENVO
xref: RO:0001000
is_a: derives_from_part_of ! derives from part of

[Typedef]
id: derives_from_part_of
name: derives from part of
namespace: ENVO
def: "A relation between two distinct material entities, the new entity and the old entity, in which the new entity begins to exist through the separation or transformation of a part of the old entity, and the new entity inherits a significant portion of the matter belonging to that part of the old entity." []
xref: ENVO:01003004

[Typedef]
id: derives_into
namespace: ENVO
xref: RO:0001001

[Typedef]
id: determined_by
namespace: ENVO
xref: RO:0002507

[Typedef]
id: determined_by_part_of
namespace: ENVO
xref: RO:0002509

[Typedef]
id: disconnected_from
name: disconnected_from
namespace: ENVO
def: "A is disconnected_from B if they have no parts in common." [https://orcid.org/0000-0002-6601-2165]
synonym: "non_overlapping_with" EXACT []
expand_assertion_to: "Class: <http://www.w3.org/2002/07/owl#Nothing> EquivalentTo: (BFO_0000050 some ?X) and (BFO_0000050 some ?Y)" []
is_metadata_tag: true
is_class_level: true

[Typedef]
id: distributary_of
namespace: ENVO
xref: RO:0002377

[Typedef]
id: during_which_ends
namespace: ENVO
xref: RO:0002084

[Typedef]
id: during_which_starts
namespace: ENVO
xref: RO:0002088

[Typedef]
id: ends
namespace: ENVO
xref: RO:0002229

[Typedef]
id: formed_as_result_of
namespace: ENVO
xref: RO:0002354

[Typedef]
id: generates
name: generates
namespace: ENVO
def: "A relation between a process and a disposition such that the existence of the disposition is caused by the execution of the process." []
xref: ENVO:2000036
property_value: IAO:0000116 "Consider ceding to RO" xsd:string
created_by: https://orcid.org/0000-0002-6601-2165
creation_date: 2018-11-03T20:58:13Z

[Typedef]
id: has_characteristic
namespace: ENVO
xref: RO:0000053

[Typedef]
id: has_component
namespace: ENVO
xref: RO:0002180

[Typedef]
id: has_condition
name: has_condition
namespace: ENVO
comment: Experimental relation used in EnvO. A condition defines a restricted range of a given quality or combination of qualities. If an environment class, E, has_condition C, then all qualities listed in C are restricted to the ranges defined in C in E. This is not intended as a logical conditional.
xref: has_condition
is_inverse_functional: true
creation_date: 2013-05-08T07:33:05Z

[Typedef]
id: has_disposition
namespace: ENVO
xref: RO:0000091

[Typedef]
id: has_end_location
namespace: ENVO
xref: RO:0002232

[Typedef]
id: has_function
namespace: ENVO
xref: RO:0000085

[Typedef]
id: has_habitat
name: has habitat
namespace: ENVO
xref: RO:0002303

[Typedef]
id: has_increased_levels_of
namespace: ENVO
xref: has_increased_levels_of

[Typedef]
id: has_input
namespace: ENVO
xref: RO:0002233

[Typedef]
id: has_member
namespace: ENVO
xref: RO:0002351

[Typedef]
id: has_output
namespace: ENVO
xref: RO:0002234

[Typedef]
id: has_part
namespace: ENVO
xref: BFO:0000051

[Typedef]
id: has_part_that_occurs_in
namespace: ENVO
xref: RO:0002479

[Typedef]
id: has_participant
namespace: ENVO
xref: RO:0000057

[Typedef]
id: has_quality
namespace: ENVO
xref: RO:0000086

[Typedef]
id: has_role
namespace: ENVO
xref: RO:0000087

[Typedef]
id: input_of
namespace: ENVO
xref: RO:0002352

[Typedef]
id: involved_in
namespace: ENVO
xref: RO:0002331

[Typedef]
id: involved_in_negative_regulation_of
namespace: ENVO
xref: RO:0002430

[Typedef]
id: located_in
namespace: ENVO
xref: RO:0001025

[Typedef]
id: location_of
namespace: ENVO
xref: RO:0001015

[Typedef]
id: member_of
namespace: ENVO
xref: RO:0002350

[Typedef]
id: negatively_regulates
namespace: ENVO
xref: RO:0002212

[Typedef]
id: obsolete_determined_by
name: obsolete determined by
namespace: ENVO
xref: ENVO:2100001
is_obsolete: true

[Typedef]
id: obsolete_determined_by_part_of
name: obsolete determined by part of
namespace: ENVO
xref: ENVO:2100007
is_obsolete: true

[Typedef]
id: obsolete_has_active_participant
namespace: ENVO
xref: RO:0002218

[Typedef]
id: occurs_in
namespace: ENVO
xref: BFO:0000066

[Typedef]
id: output_of
namespace: ENVO
xref: RO:0002353

[Typedef]
id: overlaps
namespace: ENVO
xref: RO:0002131

[Typedef]
id: part_of
namespace: ENVO
xref: BFO:0000050

[Typedef]
id: partially_overlaps
namespace: ENVO
xref: RO:0002151

[Typedef]
id: partially_surrounded_by
name: partially_surrounded_by
namespace: ENVO
def: "x partially_surrounded_by y if and only if (1) x is adjacent to y and for the region r that is adjacent to x, r partially overlaps y (2) the shared boundary between x and y occupies  a non-trivial proportion of the outermost boundary of x" []
comment: Definition modified from 'surrounded by'.
xref: ENVO:01001307
property_value: IAO:0000112 "A duck swimming in a pond is partially surrounded by air and partially surrounded by water." xsd:string

[Typedef]
id: participates_in
namespace: ENVO
xref: RO:0000056

[Typedef]
id: preceded_by
namespace: ENVO
xref: BFO:0000062

[Typedef]
id: precedes
namespace: ENVO
xref: BFO:0000063

[Typedef]
id: process_has_causal_agent
namespace: ENVO
xref: RO:0002608

[Typedef]
id: realized_in
namespace: ENVO
xref: BFO:0000054

[Typedef]
id: realizes
namespace: ENVO
xref: BFO:0000055

[Typedef]
id: regulates_(processual)
name: regulates (processual)
namespace: ENVO
xref: RO:0002211

[Typedef]
id: results_in_expansion_of
name: results in expansion of
namespace: ENVO
def: "A process, p, results in the expansion of a material entity, m, if the spatial extent of m is increased as a result of participating in p." []
xref: ENVO:02500016
property_value: IAO:0000112 "Afforestation results in the expansion of a forest." xsd:string

[Typedef]
id: results_in_formation_of
namespace: ENVO
xref: RO:0002297

[Typedef]
id: results_in_proliferation_of
name: results in proliferation of
namespace: ENVO
comment: To be ceded to RO
xref: ENVO:02500020

[Typedef]
id: results_in_transformation_into
name: results in transformation into
namespace: ENVO
xref: ENVO:02500006

[Typedef]
id: starts_during
namespace: ENVO
xref: RO:0002091

[Typedef]
id: surrounded_by
name: surrounded by
namespace: ENVO
xref: RO:0002219

[Typedef]
id: towards
namespace: ENVO
xref: RO:0002503

[Typedef]
id: tributary_of
namespace: ENVO
xref: RO:0002376

