format-version: 1.2
data-version: envo/releases/2020-06-22/subsets/envoAstro.owl
subsetdef: disposition_slim "Disposition slim"
subsetdef: environmental_hazards "environmental_hazards"
subsetdef: EnvO-Lite-GSC "EnvO-Lite-GSC"
subsetdef: envoAstro "envoAstro"
subsetdef: envoAtmo "envoAtmo"
subsetdef: envoCesab "envoCesab"
subsetdef: envoCmecs "envoCmecs"
subsetdef: envoEmpo "envoEmpo"
subsetdef: envoEOVs "envoEOVs"
subsetdef: envoMarine "envoMarine"
subsetdef: envoMeo "envoMeo"
subsetdef: envoNceas "envoNceas"
subsetdef: envoOmics "envoOmics"
subsetdef: envoPolar "envoPolar"
subsetdef: mpath_slim "Pathology slim"
subsetdef: nlcd2011 "nlcd2011"
subsetdef: relational_slim "Relational slim: types of quality that require an additional entity in order to exist"
subsetdef: ro-eco "ro-eco"
subsetdef: scalar_slim "Scalar slim"
subsetdef: value_slim "Value slim"
subsetdef: wwfBiome "wwfBiome"
synonymtypedef: PLURAL "plurals"
ontology: envo/subsets/envoAstro
property_value: owl:versionInfo "2020-06-22" xsd:string

[Term]
id: ENVO:00000070
name: human construction
namespace: ENVO
def: "A construction that has been assembled by deliberate human effort." [MA:ma]
synonym: "constructed feature" EXACT []
relationship: output_of ENVO:01000996 ! human-directed construction process
relationship: part_of ENVO:01000983 ! technosphere
property_value: IAO:0000116 "\"constructed\" should probably be made something like a quality and this class obsoleted or filled only by inference" xsd:string

[Term]
id: ENVO:00000191
name: solid astronomical body part
namespace: ENVO
def: "A part of an astronomical body which is primarily composed of a continuous volume of solid material, shaped by one or more environmental processes." [https://en.wikipedia.org/wiki/Landform]
synonym: "geological feature" RELATED [ADL:FTT]
synonym: "physiographic feature" RELATED []
xref: EcoLexicon:landform
xref: EcoLexicon:landforms
xref: FTT:754
xref: FTT:96
xref: SWEETRealm:Landform
xref: TGN:21400
xref: TGN:21401
is_a: ENVO:01000813 ! astronomical body part
intersection_of: ENVO:01000813 ! astronomical body part
intersection_of: composed_primarily_of ENVO:01000814 ! solid environmental material

[Term]
id: ENVO:00001995
name: rock
namespace: ENVO
def: "A rock is a naturally occurring solid aggregate of one or more minerals or mineraloids." [https://en.wikipedia.org/wiki/Rock_(geology), MA:ma]
comment: From https://en.wikipedia.org/wiki/ [A mineral] is different from a rock, which can be an aggregate of minerals or non-minerals and does not have a specific chemical composition. The exact definition of a mineral is under debate, especially with respect to the requirement a valid species be abiogenic, and to a lesser extent with regards to it having an ordered atomic structure.
xref: EcoLexicon:rock
xref: FTT:1010
xref: FTT:145
xref: Geonames:T.RK
xref: Geonames:T.RKS
xref: https://en.wikipedia.org/wiki/Rock
xref: SWEETRealm:Rock
xref: TGN:21444
is_a: ENVO:01000814 ! solid environmental material
disjoint_from: ENVO:01000256 ! mineral material

[Term]
id: ENVO:00001998
name: soil
namespace: ENVO
def: "Soil is an environmental material which is primarily composed of minerals, varying proportions of sand, silt, and clay, organic material such as humus, gases, liquids, and a broad range of resident micro- and macroorganisms." [https://en.wikipedia.org/wiki/Soil]
comment: 'In engineering terms, soil is referred to as regolith, or loose rock material that lies above the 'solid geology'. Soil is commonly referred to as "earth" or "dirt"; technically, the term "dirt" should be restricted to displaced soil.' https://en.wikipedia.org/wiki/Soil\n\n" The upper limit of soil is the boundary between soil and air, shallow water, live plants, or plant materials that have not begun to decompose. Areas are not considered to have soil if the surface is permanently covered by water too deep (typically more than 2.5 meters) for the growth of rooted plants.\n\nThe lower boundary that separates soil from the nonsoil underneath is most difficult to define. Soil consists of horizons near the Earth's surface that, in contrast to the underlying parent material, have been altered by the interactions of climate, relief, and living organisms over time. Commonly, soil grades at its lower boundary to hard rock or to earthy materials virtually devoid of animals, roots, or other marks of biological activity. For purposes of classification, the lower boundary of soil is arbitrarily set at 200 cm."  Soil taxonomy, 2nd Ed., quoted in http://www.nrcs.usda.gov/wps/portal/nrcs/detail/soils/edu/?cid=nrcs142p2_054280
subset: EnvO-Lite-GSC
synonym: "regolith" BROAD []
xref: https://en.wikipedia.org/wiki/Soil
xref: LTER:535
xref: SPIRE:Soil
xref: SWEETRealm:Soil
is_a: ENVO:00010483 ! environmental material
relationship: has_part ENVO:00002982 ! clay
relationship: has_part ENVO:01000016 ! silt
relationship: has_part ENVO:01000017 ! sand
relationship: has_part ENVO:01000155 ! organic material
relationship: has_part ENVO:01000256 ! mineral material
relationship: part_of ENVO:01000820 ! pedosphere
property_value: IAO:0000116 "The various 'has part' and 'has quality' relations may not hold true for all soils; however, I have yet to find counter examples. Require input from a pedologist or similar. [pbuttigieg]" xsd:string

[Term]
id: ENVO:00002006
name: liquid water
namespace: ENVO
def: "An environmental material primarily composed of dihydrogen oxide in its liquid form." [MA:ma]
synonym: "water" BROAD []
xref: EcoLexicon:water
xref: https://en.wikipedia.org/wiki/Water
xref: LTER:617
is_a: ENVO:01000815 ! liquid environmental material

[Term]
id: ENVO:00002982
name: clay
namespace: ENVO
def: "A group of hydrous aluminium phyllosilicate (phyllosilicates being a subgroup of silicate minerals) minerals (see clay minerals), that are typically less than 2 micrometres in diameter. Clay consists of a variety of phyllosilicate minerals rich in silicon and aluminium oxides and hydroxides which include variable amounts of structural water." [https://en.wikipedia.org/wiki/Clay]
xref: EcoLexicon:clay
xref: https://en.wikipedia.org/wiki/Clay
xref: SWEETRealm:Clay
is_a: ENVO:00010483 ! environmental material
disjoint_from: ENVO:01000016 ! silt

[Term]
id: ENVO:00003074
name: manufactured product
namespace: ENVO
def: "A material entity that has been processed by humans or their technology in any way, including intermediate products as well as final products." [] {comment="https://en.wikipedia.org/wiki/Manufactured_product"}
synonym: "manufactured good" EXACT []
relationship: output_of ENVO:01000993 ! manufacturing process

[Term]
id: ENVO:00010483
name: environmental material
namespace: ENVO
def: "A portion of environmental material is a fiat object part which forms the medium or part of the medium of an environmental system." [DOI:10.1186/2041-1480-4-43, MA:ma, ORCID:0000-0002-4366-3088, URL:http\://ontology.buffalo.edu/smith/articles/niches.html]
comment: Everything under this parent must be a mass noun. All subclasses are to be understood as being composed primarily of the named entity, rather than restricted to that entity. For example, "ENVO:water" is to be understood as "environmental material composed primarly of some CHEBI:water". This class is currently being aligned to the Basic Formal Ontology. Following this alignment, its definition and the definitions of its subclasses will be revised.
synonym: "portion of environmental material" EXACT []

[Term]
id: ENVO:01000016
name: silt
namespace: ENVO
def: "Silt is granular material of a size somewhere between sand and clay whose mineral origin is quartz and feldspar." [https://en.wikipedia.org/wiki/Silt]
comment: https://en.wikipedia.org/wiki/ In the Udden-Wentworth scale (due to Krumbein), silt particles range between 0.0039 to 0.0625 mm, larger than clay but smaller than sand particles. ISO 14688 grades silts between 0.002 mm and 0.063 mm. In actuality, silt is chemically distinct from clay, and unlike clay, grains of silt are approximately the same size in all dimensions; furthermore, their size ranges overlap. Clays are formed from thin plate-shaped particles held together by electrostatic forces, so present a cohesion. According to the U.S. Department of Agriculture Soil Texture Classification system, the sand-silt distinction is made at the 0.05 mm particle size. The USDA system has been adopted by the Food and Agriculture Organization (FAO). In the Unified Soil Classification System (USCS) and the AASHTO Soil Classification system, the sand-silt distinction is made at the 0.075 mm particle size (i.e., material passing the #200 sieve). Silts and clays are distinguished mechanically by their plasticity.
xref: EcoLexicon:silt
xref: https://en.wikipedia.org/wiki/Silt
xref: SWEETRealm:Silt
is_a: ENVO:00010483 ! environmental material
disjoint_from: ENVO:01000017 ! sand

[Term]
id: ENVO:01000017
name: sand
namespace: ENVO
def: "A naturally occurring granular material composed of finely divided rock and mineral particles." [https://en.wikipedia.org/wiki/Sand]
xref: EcoLexicon:sand
xref: https://en.wikipedia.org/wiki/Sand
xref: LTER:484
xref: SWEETRealm:Sand
is_a: ENVO:00010483 ! environmental material
relationship: derives_from ENVO:00001995 ! rock

[Term]
id: ENVO:01000155
name: organic material
namespace: ENVO
def: "Environmental material derived from living organisms and composed primarily of one or more biomacromolecules." [ISBN:978-0-618-45504-1, ORCID:0000-0002-4366-3088]
synonym: "biomass" EXACT []
xref: EcoLexicon:organic_material
is_a: ENVO:00010483 ! environmental material
created_by: ORCID:0000-0002-4366-3088
creation_date: 2010-03-20T08:40:04Z

[Term]
id: ENVO:01000256
name: mineral material
namespace: ENVO
def: "A mineral material is an environmental material which is primarily composed of some substance that is naturally occurring, solid and stable at room temperature, representable by a chemical formula, usually abiogenic, and that has an ordered atomic structure." [https://en.wikipedia.org/wiki/Mineral]
xref: LTER:341
is_a: ENVO:00010483 ! environmental material
property_value: IAO:0000116 "Look for \"mineral\" in a chemical or geochemical ontology to formalise the composed primarily of link.\nFrom https://en.wikipedia.org/wiki/ [A mineral] is different from a rock, which can be an aggregate of minerals or non-minerals and does not have a specific chemical composition. The exact definition of a mineral is under debate, especially with respect to the requirement a valid species be abiogenic, and to a lesser extent with regards to it having an ordered atomic structure." xsd:string
created_by: ORCID:0000-0002-4366-3088
creation_date: 2013-10-05T12:37:41Z

[Term]
id: ENVO:01000267
name: atmosphere
namespace: ENVO
def: "An atmosphere is a layer of gases surrounding a material body of sufficient mass that is held in place by the gravity of the body." [https://en.wikipedia.org/wiki/Atmosphere, https://en.wikipedia.org/wiki/Physical_geography]
xref: LTER:48
is_a: ENVO:01001678 ! fluid layer
relationship: adjacent_to ENVO:01000799 ! astronomical body
created_by: ORCID:0000-0002-4366-3088
creation_date: 2013-10-10T08:14:50Z

[Term]
id: ENVO:01000277
name: water ice
namespace: ENVO
def: "Ice is water frozen into a solid state. It can appear transparent or opaque bluish-white color, depending on the presence of impurities or air inclusions. The addition of other materials such as soil may further alter its appearance." [https://en.wikipedia.org/wiki/Ice]
subset: envoPolar
synonym: "ice" RELATED [http://www.eionet.europa.eu/gemet/concept/4131]
xref: LTER:262
is_a: ENVO:01001125 ! ice
relationship: composed_primarily_of ENVO:00002006 ! liquid water
created_by: ORCID:0000-0002-4366-3088
creation_date: 2013-10-13T12:01:28Z

[Term]
id: ENVO:01000281
name: layer
namespace: ENVO
def: "A layer is a quantity of some material which is spatially continuous, has comparable thickness, and usually covers some surface." [Wiktionary:layer]
comment: Preliminary definition.
subset: envoPolar
created_by: ORCID:0000-0002-4366-3088
creation_date: 2013-10-15T16:42:02Z

[Term]
id: ENVO:01000637
name: outer space
namespace: ENVO
def: "Outer space is a hard vacuum containing a low density of particles, predominantly a plasma of hydrogen and helium as well as electromagnetic radiation, magnetic fields, neutrinos, dust and cosmic rays that exists between celestial bodies." [https://en.wikipedia.org/wiki/Outer_space]
subset: envoAstro
synonym: "space" BROAD []
is_a: ENVO:00010483 ! environmental material

[Term]
id: ENVO:01000638
name: planetary crust
namespace: ENVO
def: "A planetary crust is the outermost solid shell of a rocky planet or natural satellite, which is chemically distinct from the underlying mantle." [https://en.wikipedia.org/wiki/Crust_(geology)]
comment: This class is meant to be applicable accross planets. Earth's crust would be an instance.
synonym: "crust" BROAD []
is_a: ENVO:01000639 ! planetary structural layer

[Term]
id: ENVO:01000639
name: planetary structural layer
namespace: ENVO
def: "A planetary structural layer is laminar part of a terrestrial planet or other rocky body large enough to have differentiation by density. Planetary layers have differing physicochemical properties and composition." []
is_a: ENVO:01000281 ! layer
relationship: part_of ENVO:01000800 ! planet
property_value: IAO:0000116 "Label should be improved to match definition." xsd:string

[Term]
id: ENVO:01000646
name: lithosphere
namespace: ENVO
def: "A lithosphere is the outermost shell of a terrestrial-type planet or natural satellite that is defined by its rigid mechanical properties." [https://en.wikipedia.org/wiki/Lithosphere]
comment: Earth's lithosphere includes the crust and uppermost mantle.
is_a: ENVO:01000639 ! planetary structural layer
relationship: composed_primarily_of ENVO:01000814 ! solid environmental material
relationship: has_part ENVO:01000638 ! planetary crust

[Term]
id: ENVO:01000797
name: gaseous environmental material
namespace: ENVO
def: "A material entity which is composed of one or more chemical entities and has neither independent shape nor volume but tends to expand indefinitely." [http://www.merriam-webster.com/dictionary/gas]
synonym: "gas" NARROW []
is_a: ENVO:02000140 ! fluid environmental material
property_value: IAO:0000116 "This class is to be populated by inference." xsd:string

[Term]
id: ENVO:01000798
name: plasma
namespace: ENVO
def: "A material entity which is composed of a volume of unbound positive and negative particles in roughly equal numbers, conducts electricity, and possesses internal magnetic fields." [http://www.merriam-webster.com/dictionary/plasma, https://en.wikipedia.org/wiki/Plasma_%28physics%29]
is_a: ENVO:02000140 ! fluid environmental material
property_value: IAO:0000116 "An NTR for `quality of a plasma` has been posted on the PATO tracker: https://github.com/pato-ontology/pato/issues/88" xsd:string

[Term]
id: ENVO:01000799
name: astronomical body
namespace: ENVO
def: "An object which is naturally occuring, bound together by gravitational or electromagnetic forces, and surrounded by space." [https://en.wikipedia.org/wiki/Astronomical_object]
comment: Astronomical bodies are usually cohesive, thus the use of the term 'object' sensu BFO 'object'.
subset: envoAstro
synonym: "celestial body" RELATED []
is_a: ENVO:01000804 ! astronomical object

[Term]
id: ENVO:01000800
name: planet
namespace: ENVO
def: "A planet is an astronomical body orbiting a star or stellar remnant that is massive enough to be rounded by its own gravity, is not massive enough to cause thermonuclear fusion, and has cleared its neighbouring region of planetesimals." [http://solarsystem.nasa.gov/planets/whatisaplanet, https://en.wikipedia.org/wiki/Planet]
comment: Considerable debate on the definition of planet exists.
subset: envoAstro
subset: envoPolar
is_a: ENVO:01000799 ! astronomical body

[Term]
id: ENVO:01000801
name: star
namespace: ENVO
def: "An astronomical object which is composed primarily of luminous plasma held in a spherical form by gravitational forces." [https://en.wikipedia.org/wiki/Star]
subset: envoAstro
subset: envoPolar
is_a: ENVO:01000799 ! astronomical body
relationship: composed_primarily_of ENVO:01000798 ! plasma
property_value: IAO:0000116 "Add qualities such as spherical. Request NTRs if not available in PATO." xsd:string

[Term]
id: ENVO:01000802
name: planetary moon
namespace: ENVO
def: "An astronomical body which orbits a planet of comparatively greater mass." [http://solarsystem.nasa.gov/planets/solarsystem/sats, https://en.wikipedia.org/wiki/Natural_satellite]
comment: At times, a moon is equated to a natural satellite, however, the latter class includes a broader range of entities. Here, we currently separate moons from other satellites. We can create a logical definition of satellite using an orbital process class.
subset: envoAstro
synonym: "moon" BROAD []
synonym: "natural satellite" RELATED []
is_a: ENVO:01000799 ! astronomical body

[Term]
id: ENVO:01000803
name: asteroid
namespace: ENVO
comment: This class is hard to define and is sometimes treated as equivalent to 'minor planet'.
subset: envoAstro
is_a: ENVO:01000809 ! minor planet

[Term]
id: ENVO:01000804
name: astronomical object
namespace: ENVO
def: "An object which is composed of one or more gravitationally bound structures that are associated with a position in space." [https://en.wikipedia.org/wiki/Astronomical_object]
comment: If there is only one astronomical body involved, this class is equivalent to ENVO:01000799. This may be problematic with reasoning, but it seems to be true to the rather fuzzy definitions found thus far.
subset: envoAstro
synonym: "celestial object" RELATED []
relationship: has_part ENVO:01000799 {minCardinality="1"} ! astronomical body
relationship: has_quality ENVO:01001164 ! geodiversity
relationship: surrounded_by ENVO:01000637 ! outer space

[Term]
id: ENVO:01000805
name: globular star cluster
namespace: ENVO
def: "A group of gravitationally bound stars." [https://en.wikipedia.org/wiki/Star_cluster]
comment: There is a need to account for open star clusters which are not gravitationally bound. This would need a superclass other than 'astronomical object', as currently defined.
subset: envoAstro
is_a: ENVO:01000804 ! astronomical object

[Term]
id: ENVO:01000806
name: nebula
namespace: ENVO
def: "An interstellar cloud of dust, hydrogen, helium and other ionized gases" [https://en.wikipedia.org/wiki/Nebula]
subset: envoAstro
is_a: ENVO:01000804 ! astronomical object

[Term]
id: ENVO:01000807
name: galaxy
namespace: ENVO
def: "A galaxy is a gravitationally bound system of stars, stellar remnants, interstellar gas, dust, and dark matter." [https://en.wikipedia.org/wiki/Galaxy]
subset: envoAstro
is_a: ENVO:01000804 ! astronomical object

[Term]
id: ENVO:01000808
name: dwarf planet
namespace: ENVO
def: "An astronomical body which is in direct orbit of a star and is massive enough for its own gravity to compress it into a shape preserved by hydrostatic equilibrium (usually a spheroid), but which shares its orbit with other bodies, such as asteroids or comets." [http://solarsystem.nasa.gov/planets/Dwarf, https://en.wikipedia.org/wiki/Dwarf_planet]
comment: Considerable debate on this definition exists.
subset: envoAstro
is_a: ENVO:01000809 ! minor planet

[Term]
id: ENVO:01000809
name: minor planet
namespace: ENVO
def: "A minor planet is an astronomical object in direct orbit around the Sun that is neither a planet nor exclusively classified as a comet. Minor planets can be dwarf planets, asteroids, trojans, centaurs, Kuiper belt objects, and other trans-Neptunian objects." [https://en.wikipedia.org/wiki/Minor_planet]
comment: "Before 2006, the IAU had officially used the term minor planet. During its 2006 meeting, the IAU reclassified minor planets and comets into dwarf planets and small Solar System bodies (SSSB). Objects are called dwarf planets if their self-gravity is sufficient to achieve hydrostatic equilibrium and form an ellipsoidal shape. All other minor planets and comets are called small Solar System bodies. The IAU stated that the term minor planet may still be used, but the term small Solar System body will be preferred. However, for purposes of numbering and naming, the traditional distinction between minor planet and comet is still used." {xref="https://en.wikipedia.org/wiki/Minor_planet"}
subset: envoAstro
is_a: ENVO:01000799 ! astronomical body
property_value: IAO:0000116 "This definition is in need of revision - it relies on negation and seems to straddle class and instance level. The definitional space here is contested and quite inhomogeneous." xsd:string

[Term]
id: ENVO:01000813
name: astronomical body part
namespace: ENVO
def: "A material part of an astronomical body." []
subset: envoAstro
subset: envoPolar
relationship: part_of ENVO:01000799 ! astronomical body

[Term]
id: ENVO:01000814
name: solid environmental material
namespace: ENVO
def: "An environmental material which is in a solid state." []
comment: This is a defined class: its subclasses will not be asserted, but filled by inference.
is_a: ENVO:00010483 ! environmental material

[Term]
id: ENVO:01000815
name: liquid environmental material
namespace: ENVO
def: "An environmental material which is in a liquid state." []
comment: This is a defined class: most of its subclasses will not be asserted, but filled by inference.
subset: envoPolar
is_a: ENVO:02000140 ! fluid environmental material

[Term]
id: ENVO:01000817
name: biosphere
namespace: ENVO
def: "A biosphere is a part of an astronomical body which includes, as parts, all the living entities within the gravitational sphere of influence of that body, as well as the non-living and dead entities with which they interact." [http://www.biology-online.org/dictionary/Biosphere, https://en.wikipedia.org/wiki/Biosphere]
comment: The gravitational sphere of influence referenced in this class' definition is the Hill sphere: a region in which an object dominates the attraction of satellites despite gravitational perturbations.
subset: envoAstro
subset: envoPolar
is_a: ENVO:01001784 ! compound astronomical body part
property_value: IAO:0000116 "Whether this class should be grouped with classes such as \"hydrosphere\" and \"cryosphere\" requires some discussion." xsd:string

[Term]
id: ENVO:01000818
name: cryosphere
namespace: ENVO
def: "A cryosphere is that part of a planet which is primarily composed of water is in solid form." [https://en.wikipedia.org/wiki/Cryosphere]
comment: This is a very broad and, in practice, poorly defined term. Please consider using or requesting a more specific class.
subset: envoAstro
subset: envoPolar
is_a: ENVO:00000191 ! solid astronomical body part
relationship: composed_primarily_of ENVO:01000277 ! water ice

[Term]
id: ENVO:01000819
name: hydrosphere
namespace: ENVO
def: "An astronomical body part which is composed of the combined mass of water found on, under, and over the surface of a planet." [https://en.wikipedia.org/wiki/Hydrosphere]
comment: This is a very broad and, in practice, poorly defined term. Please consider using or requesting a more specific class.
subset: envoAstro
subset: envoPolar
is_a: ENVO:01001477 ! liquid astronomical body part
relationship: composed_primarily_of ENVO:00002006 ! liquid water

[Term]
id: ENVO:01000820
name: pedosphere
namespace: ENVO
def: "An astronomical body part which is composed of soil, subject to soil formation processes, and found on the surface of a lithosphere." [https://en.wikipedia.org/wiki/Pedosphere]
comment: This is a very broad and, in practice, poorly defined term. Please consider using or requesting a more specific class.
subset: envoAstro
is_a: ENVO:01001784 ! compound astronomical body part
relationship: composed_primarily_of ENVO:00001998 ! soil
relationship: overlaps ENVO:01000267 ! atmosphere
relationship: overlaps ENVO:01000646 ! lithosphere
relationship: overlaps ENVO:01000817 ! biosphere
relationship: overlaps ENVO:01000819 ! hydrosphere

[Term]
id: ENVO:01000821
name: photosphere
namespace: ENVO
def: "An astronomical body part which is composed of those parts of a star, distal from the star's core, from which light is radiated into space." [https://en.wikipedia.org/wiki/Photosphere]
subset: envoAstro
is_a: ENVO:01000813 ! astronomical body part
relationship: part_of ENVO:01000801 ! star

[Term]
id: ENVO:01000958
name: terrestrial planet
namespace: ENVO
def: "A planet that is composed primarily of silicate rocks or metals." [https://en.wikipedia.org/wiki/Terrestrial_planet]
subset: envoAstro
synonym: "Earth-like planet" RELATED []
synonym: "rocky planet" EXACT []
synonym: "telluric planet" EXACT []
is_a: ENVO:01000800 ! planet

[Term]
id: ENVO:01000983
name: technosphere
namespace: ENVO
def: "A part of an astronomical body which includes, as parts, all the entities which have been constructed or manufactured by humans or their technology and which are within the gravitational sphere of influence of that body." [http://dx.doi.org/10.1177/2053019616677743, http://www.yourdictionary.com/technosphere, https://www.sciencedaily.com/releases/2016/11/161130085021.htm]
comment: The gravitational sphere of influence referenced in this class' definition is the Hill sphere: a region in which an object dominates the attraction of satellites despite gravitational perturbations.
subset: envoAstro
is_a: ENVO:01000813 ! astronomical body part
relationship: has_part ENVO:00000070 ! human construction
relationship: has_part ENVO:00003074 ! manufactured product
relationship: overlaps ENVO:01000817 ! biosphere

[Term]
id: ENVO:01000993
name: manufacturing process
namespace: ENVO
def: "A planned process during which raw or recycled materials are transformed into products for use or sale using labour and machines, tools, chemical and biological processing, or formulation." [https://en.wikipedia.org/wiki/Manufacturing]
comment: The term may refer to a range of human activity, from handicraft to high tech, but is most commonly applied to industrial production, in which raw materials are transformed into finished goods on a large scale. {xref="https://en.wikipedia.org/wiki/Manufacturing"}

[Term]
id: ENVO:01000996
name: human-directed construction process
namespace: ENVO
def: "An process during which natural or manufactured materials and products are processed and arranged by humans or their technology into structures." []
relationship: has_part ENVO:03000010 ! material transport process
relationship: has_part ENVO:03000043 ! material transformation process
property_value: IAO:0000116 "The nature of \"structures\" must be further specified." xsd:string

[Term]
id: ENVO:01001023
name: radiation
namespace: ENVO
def: "A process during which energy is emitted or transmitted in the form of waves or particles through space or a material medium." [https://en.wikipedia.org/wiki/Radiation]
subset: environmental_hazards
subset: envoAstro
is_a: ENVO:01001852 ! energy transfer process
relationship: has_participant ENVO:00010483 ! environmental material
property_value: IAO:0000116 "Requires addition of waves for full axiomatisation. This should be linked to \"subatomic particle\" with an \"or\". Note that ENVO represents space as an environmental material (a hard vacuum with sparse material inclusions)." xsd:string

[Term]
id: ENVO:01001024
name: particle radiation
namespace: ENVO
def: "A radiation process during which energy is transmitted or emitted by means of fast-moving subatomic particles." [https://en.wikipedia.org/wiki/Particle_radiation]
subset: environmental_hazards
subset: envoAstro
is_a: ENVO:01001023 ! radiation

[Term]
id: ENVO:01001025
name: particle beam radiation
namespace: ENVO
def: "A particle radiation process during which subatomic particles move in the same direction." [https://en.wikipedia.org/wiki/Particle_radiation]
subset: environmental_hazards
subset: envoAstro
is_a: ENVO:01001024 ! particle radiation

[Term]
id: ENVO:01001026
name: electromagnetic radiation
namespace: ENVO
def: "A radiation process during which waves (or their quanta, photons) of the electromagnetic field propagate (radiate) through space carrying electromagnetic energy." [https://en.wikipedia.org/wiki/Electromagnetic_radiation]
comment: Note that this class is concerned only with active radiative processes: static electric and magnetic fields are not inlcuded. All electromagnetic radiation carries radiant energy.
subset: environmental_hazards
subset: envoAstro
synonym: "EM radiation" EXACT []
is_a: ENVO:01001023 ! radiation

[Term]
id: ENVO:01001027
name: acoustic radiation
namespace: ENVO
def: "A radiation process during which mechanical waves generated by oscillations radiate through an environmental material." [https://en.wikipedia.org/wiki/Acoustics] {comment="https://en.wikipedia.org/wiki/Vibration", comment="https://en.wikipedia.org/wiki/Mechanical_wave"}
comment: The mechanical waves generated by this process are also referred to as pressure waves.
subset: envoAstro
is_a: ENVO:01001023 ! radiation

[Term]
id: ENVO:01001068
name: meteoroid
namespace: ENVO
def: "An astronomical body which is composed of rocky or metallic materials and is considerably smaller than asteroids." [https://en.wikipedia.org/wiki/Meteoroid]
subset: envoAstro
is_a: ENVO:01000799 ! astronomical body

[Term]
id: ENVO:01001122
name: gas planet
namespace: ENVO
def: "A planet which is primarily composed of hydrogen and helium." [http://solarsystem.nasa.gov/planets/whatisaplanet, https://en.wikipedia.org/wiki/List_of_planet_types, https://en.wikipedia.org/wiki/Planet]
comment: Gas giants are composed of about 90% hydrogen and helium. Jupiter and Saturn are examples of gas giants.
subset: envoAstro
is_a: ENVO:01000800 ! planet
relationship: composed_primarily_of ENVO:01001155 ! astrogeological gas

[Term]
id: ENVO:01001123
name: dwarf gas planet
namespace: ENVO
def: "A gas planet which 1) is considerably smaller than a gas giant and 2) has a rocky core around which a thick envelope primarily composed of hydrogen, helium, and smaller proportions of volatiles." [http://solarsystem.nasa.gov/planets/whatisaplanet, https://en.wikipedia.org/wiki/Gas_dwarf, https://en.wikipedia.org/wiki/List_of_planet_types, https://en.wikipedia.org/wiki/Planet]
comment: The physical make-up of gas dwarfs limit their size, which gravitate towards a total radius between 1.7 and 3.9 Earth-radii. {xref="https://en.wikipedia.org/wiki/Gas_dwarf"}
subset: envoAstro
is_a: ENVO:01001122 ! gas planet

[Term]
id: ENVO:01001124
name: giant gas planet
namespace: ENVO
def: "A gas planet which has mass and size comparable to Jupiter and Saturn." [http://solarsystem.nasa.gov/planets/whatisaplanet, https://en.wikipedia.org/wiki/Gas_giant, https://en.wikipedia.org/wiki/List_of_planet_types, https://en.wikipedia.org/wiki/Planet]
subset: envoAstro
synonym: "gas giant" EXACT []
is_a: ENVO:01001122 ! gas planet
property_value: IAO:0000116 "The definition should be revised to avoid relativisation to instances." xsd:string

[Term]
id: ENVO:01001125
name: ice
namespace: ENVO
def: "An ice is an environmental material which is either frozen or which is maintained in a solid state by gravitational forces or pressure." []
comment: Note that ice may be formed at very high temperatures, due to gravitational effects and/or pressure.
is_a: ENVO:00010483 ! environmental material

[Term]
id: ENVO:01001126
name: astrogeological ice
namespace: ENVO
def: "An astrogeological volatile which is composed primarily of chemical compounds with freezing points above an approximate threshold of 100 Kelvin." [https://en.wikipedia.org/wiki/Ice_giant]
comment: This is a term native to the fields of planetary science and astrophysics.  Water, ammonia, and methane are considered "ices" with freezing points of 273 K, 195 K, and 91 K, respectively.
subset: envoAstro
synonym: "ice" RELATED []
is_a: ENVO:01001154 ! volatile astrogeological material

[Term]
id: ENVO:01001127
name: ice giant
namespace: ENVO
def: "A giant planet which is primarily composed of elements heavier than hydrogen and helium, volatile chemical compounds with freezing points above about 100 Kelvin." [http://solarsystem.nasa.gov/planets/whatisaplanet, https://en.wikipedia.org/wiki/Ice_giant, https://en.wikipedia.org/wiki/List_of_planet_types, https://en.wikipedia.org/wiki/Planet]
comment: Uranus and Neptune are considered ice giants, a separate class relative to the gas giants, Jupiter and Saturn. Ice giants consist of only about 20% hydrogen and helium in mass.  A large portion of the mass in an ice giant was incorporated by the capture of ice (as defined in planetary science) or as gas trapped in water ice.
subset: envoAstro
is_a: ENVO:01000800 ! planet
intersection_of: ENVO:01000800 ! planet
intersection_of: composed_primarily_of ENVO:01001126 ! astrogeological ice

[Term]
id: ENVO:01001128
name: mini-Neptune
namespace: ENVO
def: "A gas planet which has an atmosphere composed of hydrogen and helium  - probably with deep layers of ice, rock or liquid oceans (made of water, ammonia, a mixture of both, or heavier volatiles) - and a small core made of low-density volatiles." [https://en.wikipedia.org/wiki/Gas_dwarf, https://en.wikipedia.org/wiki/Mini-Neptune]
comment: These planets have a mass up to 10 Earth masses, notably smaller than Uranus or Neptune, which are about 14.5 and 17 Earth masses, respectively.
subset: envoAstro
synonym: "transitional planet" RELATED []
is_a: ENVO:01001122 ! gas planet

[Term]
id: ENVO:01001129
name: super-Jupiter
namespace: ENVO
def: "An astronomical object which is more massive than the planet Jupiter." [https://en.wikipedia.org/wiki/Super-Jupiter]
comment: Due to their immense size, super-Jupiter class objects straddle the space between planets and other objects such as brown dwarfs. While they may be more massive than Jupiter, super-Jupiters tend to be the same approximate size, with increasing density as their mass increases up to about 80 Jupiter masses.
subset: envoAstro
is_a: ENVO:01000799 ! astronomical body

[Term]
id: ENVO:01001130
name: gravitational motion
namespace: ENVO
def: "A process during which one or more entities move along geodesics in a region of spacetime that has been sufficiently curved towards an entity with sufficient mass and/or energy." [https://en.wikipedia.org/wiki/Gravity]
subset: envoAstro
is_a: ENVO:02500000 ! environmental system process

[Term]
id: ENVO:01001131
name: hot Jupiter
namespace: ENVO
def: "A giant gas planet which has a jovian-scale mass (0.36–11.8 Jupiter masses), a short orbital period (1.3–111 Earth days), and which is close to the star it orbits, resulting in extreme and exotic atmospheric properties." []
comment: It is assumed that the mass of a hot Jupiter cannot be greater than approximately 13.6 Jupiter masses, beyond which the planet would start burning deuterium and become a brown dwarf. {xref="https://en.wikipedia.org/wiki/Hot_Jupiter"}
subset: envoAstro
synonym: "epistellar jovian" EXACT []
synonym: "pegasean planet" EXACT []
synonym: "pegasid" EXACT []
synonym: "roaster planet" EXACT []
is_a: ENVO:01001124 ! giant gas planet
property_value: IAO:0000116 "" xsd:string

[Term]
id: ENVO:01001132
name: hot Neptune
namespace: ENVO
def: "A gas planet which has a mass similar to that of Neptune or Uranus and which closely orbits its star (normally at a distance less than 1 Astronomical Unit)." [https://en.wikipedia.org/wiki/Hot_Neptune]
subset: envoAstro
synonym: "hoptune" EXACT []
is_a: ENVO:01001122 ! gas planet
property_value: IAO:0000116 "Whether this should be classified as a gas planet or an ice giant must be explored." xsd:string

[Term]
id: ENVO:01001133
name: mega-Earth
namespace: ENVO
def: "A terrestrial exoplanet which is at least ten times the mass of Earth." [https://en.wikipedia.org/wiki/Mega-Earth]
subset: envoAstro
is_a: ENVO:01000958 ! terrestrial planet

[Term]
id: ENVO:01001134
name: super-Earth
namespace: ENVO
def: "A terrestrial planet which has a mass higher than Earth's, but substantially below the masses of Uranus and Neptune (15 and 17 Earth masses, respectively)." [https://en.wikipedia.org/wiki/Super-Earth]
comment: The upper bound of a super-Earth's mass is generally agreed on as 10 Earth masses. In general, super-Earths are defined exclusively by their masses, and the term does not imply temperatures, compositions, orbital properties, habitability, or environments.
subset: envoAstro
is_a: ENVO:01000958 ! terrestrial planet

[Term]
id: ENVO:01001135
name: desert planet
namespace: ENVO
def: "A terrestrial planet which has a surface dominated by hot deserts." []
comment: This class of planet is still mostly theoretical.
subset: envoAstro
synonym: "dry planet" EXACT []
is_a: ENVO:01000958 ! terrestrial planet

[Term]
id: ENVO:01001136
name: ocean planet
namespace: ENVO
def: "A planet which has a surface layer that nearly completely or completely covered by water, and which has a substantial portion of its mass composed of water." [https://en.wikipedia.org/wiki/Ocean_planet]
comment: While this planetary form is still mostly theoretical, strong candidates exist such as the extrasolar planet GJ 1214 b and ocean planet candidate Kepler-22b.
subset: envoAstro
synonym: "aquaplanet" EXACT []
synonym: "panthalassic planet" EXACT []
synonym: "water world" EXACT []
is_a: ENVO:01000800 ! planet
property_value: IAO:0000116 "An axiom to express that the planet has a 'substantial' proportion of its mass in the form of water wound enhance this class." xsd:string

[Term]
id: ENVO:01001137
name: ice planet
namespace: ENVO
def: "A planet which has a surface layer that nearly completely or completely covered by ice, and which has a substantial portion of its mass composed of ice." [https://en.wikipedia.org/wiki/Ice_planet]
comment: While this planetary form is still mostly theoretical, strong candidates exist such as OGLE-2005-BLG-390Lb, OGLE-2013-BLG-0341L b and MOA-2007-BLG-192Lb. Pluto was considered an ice planet until its reclassification in 2006 CE.  Surface temperatures of ice planets would have to be below 260 K (−13°C) if composed primarily of water, below 180 K (−93°C) if primarily composed of CO2 and ammonia, and below 80 K (−193°C) if composed primarily of methane. {xref="https://en.wikipedia.org/wiki/Ice_planet"}
subset: envoAstro
synonym: "cryoplanet" EXACT []
is_a: ENVO:01000800 ! planet

[Term]
id: ENVO:01001138
name: carbon dioxide ice
namespace: ENVO
def: "Ice which is primarily composed of carbon dioxide." [https://en.wikipedia.org/wiki/Ice]
subset: envoAstro
synonym: "dry ice" RELATED []
is_a: ENVO:01001125 ! ice

[Term]
id: ENVO:01001139
name: methane ice
namespace: ENVO
def: "Ice which is primarily composed of methane." [https://en.wikipedia.org/wiki/Ice]
subset: envoAstro
is_a: ENVO:01001125 ! ice

[Term]
id: ENVO:01001140
name: ammonia ice
namespace: ENVO
def: "Ice which is primarily composed of ammonia." [https://en.wikipedia.org/wiki/Ice]
subset: envoAstro
is_a: ENVO:01001125 ! ice

[Term]
id: ENVO:01001141
name: carbon monoxide ice
namespace: ENVO
def: "Ice which is primarily composed of carbon monoxide." [https://en.wikipedia.org/wiki/Ice]
subset: envoAstro
is_a: ENVO:01001125 ! ice

[Term]
id: ENVO:01001142
name: iron planet
namespace: ENVO
def: "A planet which in primarily composed of an iron-rich core with little to no mantle" [https://en.wikipedia.org/wiki/Iron_planet]
comment: Mercury is the largest iron planet in the Solar System, the other terrestrial planets being composed of silicate rocks. Some extrasolar planet candidates that may be composed mainly of iron are KOI-1843 b,[5] Kepler-70b and Kepler-10b. {xref="https://en.wikipedia.org/wiki/Iron_planet"}
subset: envoAstro
synonym: "cannonball planet" EXACT []
is_a: ENVO:01000958 ! terrestrial planet

[Term]
id: ENVO:01001143
name: lava planet
namespace: ENVO
def: "A planet which has a surface layer that nearly completely or completely covered by lava, and which has a substantial portion of its mass composed of lava." [https://en.wikipedia.org/wiki/Lava_planet]
comment: This class of planets is still mostly theoretical, however, lava planets are thought plausible shortly after a terrestrial planet is formed, soon after a terrestrial planet has suffered a large collision event, or if a terrestrial planet is orbiting very close to its star, causing intense irradiation and tidal forces.  Likely lava exoplanets include COROT-7b, Kepler-10b, Alpha Centauri Bb, and Kepler-78b. {xref="https://en.wikipedia.org/wiki/Lava_planet"}
subset: envoAstro
is_a: ENVO:01000800 ! planet

[Term]
id: ENVO:01001144
name: sub-Earth
namespace: ENVO
def: "A terrestrial planet which has a mass smaller than Earth's, such that 1) it lacks a magnetic field strong enough to shield its atmosphere from erosion by stellar wind and 2) it has comparatively short periods of geological activity unless it is subject to gravitational tidal forces from a much more massive object." [https://en.wikipedia.org/wiki/Sub-Earth]
comment: The first sub-Earths were discovered by the Kepler Orbiting Observatory space telescope on 2012-01-10, orbiting the star Kepler-42. As of June 2014, Kepler has 45 confirmed planets that are smaller than Earth, with 17 of them being smaller than 0.8 Earth radii. In addition, there are over 310 planet candidates with an estimated radius of less than 1 Earth radius, with 135 of them being smaller than 0.8 Earth radii. {xref="https://en.wikipedia.org/wiki/Sub-Earth"}
subset: envoAstro
is_a: ENVO:01000958 ! terrestrial planet

[Term]
id: ENVO:01001145
name: chthonian planet
namespace: ENVO
def: "A planet which is formed as a result of a gas giant's hydrogen and helium atmosphere, as well as its outer layers, being stripped away by a stellar wind through photoevaporation and hydrodynamic escape." [https://en.wikipedia.org/wiki/Chthonian_planet]
comment: This class is largely theoretical, however, some likely candidates exist. HD 209458 b and Gliese 436b are examples of a gas giants that are in the process of having their atmospheres stripped away. COROT-7b is the first exoplanet found that might be chthonian. {xref="https://en.wikipedia.org/wiki/Chthonian_planet"}
subset: envoAstro
synonym: "cthonian planet" EXACT []
is_a: ENVO:01000800 ! planet
property_value: IAO:0000116 "" xsd:string

[Term]
id: ENVO:01001146
name: photoevaporation
namespace: ENVO
def: "A process during which energetic radiation ionises gas and causes it to disperse away from the ionising source." [arXiv:1604.05220, https://en.wikipedia.org/wiki/Chthonian_planet#cite_note-4, https://en.wikipedia.org/wiki/Photoevaporation]
comment: This process is responsible for the stripping away of gases from the atmosphere of planets and related bodies by acceleration on interaction with high energy photons and other electromagnetic radiation.
subset: envoAstro
is_a: ENVO:03000010 ! material transport process
relationship: has_part ENVO:01001026 ! electromagnetic radiation
relationship: has_participant ENVO:01000797 ! gaseous environmental material

[Term]
id: ENVO:01001147
name: helium planet
namespace: ENVO
def: "A gas planet which has an atmosphere composed primarily of helium." [https://en.wikipedia.org/wiki/Helium_planet]
comment: A helium planet might form via hydrogen evaporation from a gaseous planet orbiting close to a star. Low-mass white dwarfs may transition into objects which are essentially helium planets by hydrogen depletion through mass transfer to a massive object such as a neutron star.  Gliese 436 b is a candidate helium planet. {xref="https://en.wikipedia.org/wiki/Helium_planet"}
subset: envoAstro
is_a: ENVO:01001122 ! gas planet
property_value: IAO:0000116 "The placement of this class assumes that some traces of hydrogen are left in the atmosphere. If this is not the case, the axiom on gas planet must be updated." xsd:string

[Term]
id: ENVO:01001148
name: planetesimal
namespace: ENVO
def: "An astronomical body which 1) is held together by its own gravity, 2)  can attract other, similar bodies through mutual gravitational influence, and 3) has orbital dynamics that are not significantly affected by gas drag." [https://en.wikipedia.org/wiki/Planetesimal]
comment: In the Solar nebula, planetesimals are usually larger than approximately 1 kilometer. {xref="https://en.wikipedia.org/wiki/Planetesimal"}
subset: envoAstro
is_a: ENVO:01000799 ! astronomical body

[Term]
id: ENVO:01001149
name: protoplanet
namespace: ENVO
def: "An astronomical object that forms within a protoplanetary disc when planetesimals and other solid debris aggregate and, due to gravitational forces,  fuse and initiate internal melting to produce a differentiated interior." [https://en.wikipedia.org/wiki/Protoplanet]
comment: Protoplanets are thought to form out of kilometer-sized planetesimals that gravitationally perturb each other's orbits and collide, gradually coalescing into the dominant planets. The exact sequence of events which lead to planetary formation from protoplanets is not fully understood. {xref="https://en.wikipedia.org/wiki/Protoplanet"}
subset: envoAstro
synonym: "planetary embryo" EXACT []
is_a: ENVO:01000799 ! astronomical body
property_value: IAO:0000116 "State that this is derived from a collection of planetesimals." xsd:string

[Term]
id: ENVO:01001150
name: protoplanetary disk
namespace: ENVO
def: "An astronomical object which is composed of dense gas and dust rotating around a young newly formed star, a T Tauri star, or a Herbig Ae/Be star in a disk-shaped configuration." [https://en.wikipedia.org/wiki/Protoplanetary_disk]
subset: envoAstro
is_a: ENVO:01000804 ! astronomical object
relationship: has_part ENVO:01000799 {minCardinality="1"} ! astronomical body
relationship: surrounded_by ENVO:01000637 ! outer space

[Term]
id: ENVO:01001151
name: proplyd
namespace: ENVO
def: "A protoplanetary disk which is externally illuminated and undergoing photoevaporation." [https://en.wikipedia.org/wiki/Proplyd, https://en.wikipedia.org/wiki/Protoplanetary_disk]
subset: envoAstro
synonym: "ionized protoplanetary disk" EXACT []
is_a: ENVO:01001150 ! protoplanetary disk
relationship: has_part ENVO:01000799 {minCardinality="1"} ! astronomical body
relationship: surrounded_by ENVO:01000637 ! outer space

[Term]
id: ENVO:01001152
name: mesoplanet
namespace: ENVO
def: "A planet which is smaller than Mercury but larger than Ceres." [https://en.wikipedia.org/wiki/Mesoplanet]
subset: envoAstro
is_a: ENVO:01000800 ! planet

[Term]
id: ENVO:01001153
name: circumbinary planet
namespace: ENVO
def: "A planet which orbits two stars." [https://en.wikipedia.org/wiki/Circumbinary_planet]
comment: Because of the short orbits of some binary stars, the only way for planets to form is by forming outside the orbit of the two stars. {xref="https://en.wikipedia.org/wiki/Circumbinary_planet"}
subset: envoAstro
is_a: ENVO:01000800 ! planet

[Term]
id: ENVO:01001154
name: volatile astrogeological material
namespace: ENVO
def: "A material which is composed primarily of chemical elements and compounds with relatively low boiling points, equilibrium condensation temperatures below 1300 Kelvin, and which are part of the crust or atmosphere of a moon or planet." [https://en.wikipedia.org/wiki/Volatiles]
comment: Examples include nitrogen, water, carbon dioxide, ammonia, hydrogen, methane and sulfur dioxide. In astrogeology, these compounds, in their solid state, often comprise large proportions of the crusts of moons and dwarf planets. {xref="https://en.wikipedia.org/wiki/Volatiles"}
subset: envoAstro
synonym: "volatile" RELATED []
is_a: ENVO:00010483 ! environmental material
property_value: IAO:0000116 "Add and axiomatise with moon and lunar crust" xsd:string

[Term]
id: ENVO:01001155
name: astrogeological gas
namespace: ENVO
def: "An astrogeological volatile which is composed primarily of chemical compounds with boiling points around those of hydrogen and helium." [https://en.wikipedia.org/wiki/Volatiles]
comment: This is a term native to the fields of planetary science and astrophysics.  Hydrogen has a boiling point of 20.271 Kelvin and a melting point of 13.99 Kelvin. Helium has a boiling point of 4.222 Kelvin and a melting point of 0.95 Kelvin.
subset: envoAstro
synonym: "gas" RELATED []
is_a: ENVO:01001154 ! volatile astrogeological material

[Term]
id: ENVO:01001156
name: refractory astrogeological material
namespace: ENVO
def: "A material which is composed primarily of chemical elements and compounds which have equilibrium condensation temperatures above approximately 1300 Kelvin and which are part of the crust or atmosphere of a moon or planet." [https://en.wikipedia.org/wiki/Refractory_(planetary_science)]
comment: The refractory group includes elements and compounds like metals and silicates (commonly termed rocks) which make up the bulk of the mass of the terrestrial planets and asteroids in the inner belt. {xref="https://en.wikipedia.org/wiki/Refractory_(planetary_science)"}
subset: envoAstro
synonym: "refractory material" RELATED []
is_a: ENVO:00010483 ! environmental material
property_value: IAO:0000116 "Add and axiomatise with moon and lunar crust" xsd:string

[Term]
id: ENVO:01001157
name: atmospheric escape
namespace: ENVO
def: "A process during which gases that constitute a planetary atmosphere escape that planet's gravitational field and move away into outer space." [https://en.wikipedia.org/wiki/Atmospheric_escape]
subset: envoAstro
is_a: ENVO:03000010 ! material transport process
relationship: has_part ENVO:01001026 ! electromagnetic radiation
relationship: has_participant ENVO:01000797 ! gaseous environmental material

[Term]
id: ENVO:01001158
name: hydrodynamic escape
namespace: ENVO
def: "An atmospheric escape process during which atoms that are parts of a planetary atmosphere escape into outer space through numerous collisions with lighter atoms in that atmosphere." [https://en.wikipedia.org/wiki/Atmospheric_escape]
subset: envoAstro
is_a: ENVO:01001157 ! atmospheric escape
relationship: has_part ENVO:01001026 ! electromagnetic radiation
relationship: has_participant ENVO:01000797 ! gaseous environmental material

[Term]
id: ENVO:01001164
name: geodiversity
namespace: ENVO
def: "A quality which inheres in a astronomical body or astronomical body part by virtue of the variation in its material composition, participation in geological processes, and the variation in is land- and hydroforms." [https://en.wikipedia.org/wiki/Geodiversity]
comment: Materials which are usually assessed when appraising geodiversity include minerals, rocks, sediments, fossils, soils and water. Landforms factored into geodiversity metrics typically include folds, faults, and other expressions of morphology or relations between units of earth material. Natural processes that are included in measures of geodiversity are those which either maintain or change materials or geoforms, including tectonics, sediment transport, and pedogenesis. Geodiversity does not usually factor in anthropogenic entities. {xref=""}

[Term]
id: ENVO:01001211
name: stellar radiation
namespace: ENVO
def: "An electromagnetic radiation process during which electromagnetic waves or their quanta are emitted from a star." [https://en.wikipedia.org/wiki/Electromagnetic_radiation, https://en.wikipedia.org/wiki/Solar_irradiance]
subset: environmental_hazards
subset: envoAstro
synonym: "solar radiation" NARROW [NCIT:C44445]
xref: NCIT:C44445
is_a: ENVO:01001026 ! electromagnetic radiation
intersection_of: ENVO:01001026 ! electromagnetic radiation
intersection_of: process_has_causal_agent ENVO:01000801 ! star

[Term]
id: ENVO:01001212
name: microwave stellar radiation
namespace: ENVO
def: "A stellar radiation process during which electromagnetic waves or their quanta are emitted from a star at wavelengths and frequencies which travel exclusively in a line-of-sight fashion and which may produce molecular rotation and torsion on contact with matter." [https://en.wikipedia.org/wiki/Microwave, https://www.iso.org/obp/ui/#iso\:std\:iso\:21348]
comment: This definition focuses on the properties of microwaves rather than their wavelength or frequency limits. Considerable ambiguity exists around the wavelength and frequency thresholds of microwaves. The ISO 21348 definition bounds these waves at 1 mm and 15 mm, with frequencies between 100 GHz and 0.225 GHz.
subset: envoAstro
synonym: "microwave radiation" EXACT []
synonym: "microwave solar radiation" NARROW []
property_value: IAO:0000114 IAO:0000428

[Term]
id: ENVO:01001213
name: radio wave stellar radiation
namespace: ENVO
def: "A stellar radiation process during which electromagnetic waves or their quanta are emitted from a star at wavelengths ranging from millimetre to kilometer scales." [https://en.wikipedia.org/wiki/Radio_wave, https://www.iso.org/obp/ui/#iso\:std\:iso\:21348]
comment: As with microwaves, considerable variation exists in the delimitation of frequency and wavelength thresholds for radiowaves. The ISO 21348 standard allows a wavelength range of 0.10 mm to 100 m and a frequency range of 300 GHz to 3 MHz. However, much lower thresholds also exist.
subset: envoAstro
synonym: "radio wave radiation" EXACT []
synonym: "radio wave solar radiation" NARROW []
property_value: IAO:0000114 IAO:0000428

[Term]
id: ENVO:01001214
name: infrared stellar radiation
namespace: ENVO
def: "A stellar radiation process during which electromagnetic waves or their quanta are emitted from a star when molecules change their rotational-vibrational movements, usually at wavelengths between 760 nm and 1 mm." [https://en.wikipedia.org/wiki/Infrared, https://www.iso.org/obp/ui/#iso\:std\:iso\:21348]
subset: envoAstro
synonym: "infra-red stellar radiation" EXACT []
synonym: "infrared radiation" BROAD []
synonym: "infrared solar radiation" NARROW []
synonym: "IR stellar radiation" RELATED []

[Term]
id: ENVO:01001215
name: visible spectrum stellar radiation
namespace: ENVO
def: "A stellar radiation process during which electromagnetic waves or their quanta are emitted from a star at wavelengths between 380 nm and 760 nm." [https://www.iso.org/obp/ui/#iso\:std\:iso\:21348]
subset: envoAstro
synonym: "optical stellar radiation" EXACT []
synonym: "visible spectrum solar radiation" NARROW []

[Term]
id: ENVO:01001216
name: ultraviolet stellar radiation
namespace: ENVO
def: "A stellar radiation process during which electromagnetic waves or their quanta are emitted from a star at wavelengths between 10 nm and 400 nm." [https://en.wikipedia.org/wiki/Ultraviolet, https://www.iso.org/obp/ui/#iso\:std\:iso\:21348]
subset: environmental_hazards
subset: envoAstro
synonym: "ultraviolet solar radiation" NARROW []
xref: NCIT:C17231
property_value: IAO:0000116 "To be expanded to account for subtypes." xsd:string

[Term]
id: ENVO:01001217
name: X-ray stellar radiation
namespace: ENVO
def: "A stellar radiation process during which penetrating electromagnetic radiation is emitted by high-energy electrons as they fall into a lower state of energy." [https://en.wikipedia.org/wiki/X-ray]
comment: Ambiguity exists in the definition of x-rays and their differentiation from gamma rays. Photons with sufficient energy to be classified as x-rays may be emitted by other processes than electrons falling to lower energy states. Most x-rays have wavelengths ranging from 0.01 to 10 nanometers, corresponding to frequencies in the range of 30 petahertz to 30 exahertz and energies in the range of 100 eV to 100 keV. {xref="https://en.wikipedia.org/wiki/X-ray#Energy_ranges"}
subset: environmental_hazards
subset: envoAstro
synonym: "x ray stellar radiation" EXACT []
synonym: "X-ray radiation" EXACT []
synonym: "X-ray solar radiation" NARROW []
synonym: "X-ray stellar radiation" EXACT []
property_value: IAO:0000114 IAO:0000428

[Term]
id: ENVO:01001218
name: gamma-ray stellar radiation
namespace: ENVO
def: "A stellar radiation process during which penetrating electromagnetic radiation is emitted from the radioactive decay (gamma decay) of atomic nuclei." [https://en.wikipedia.org/wiki/Gamma_ray]
comment: Ambiguity exists in the definition of gamma rays. As a rule of thumb, gamma rays have energies above 100 keV, frequencies above 10 exahertz, and wavelengths less than 10 picometers. However, regardless of the energy released, electromagnetic radiation from radioactive decay of atomic nuclei is referred to as "gamma rays". In astronomy, however, gamma rays are defined by their energy, and no production process needs to be specified. {xref="https://en.wikipedia.org/wiki/Gamma_ray"}
subset: environmental_hazards
subset: envoAstro
synonym: "gamma-ray solar radiation" NARROW []
property_value: IAO:0000114 IAO:0000428

[Term]
id: ENVO:01001219
name: ionizing stellar radiation
namespace: ENVO
def: "A stellar radiation process during which electromagnetic waves or their quanta are emitted from a star with sufficient energy to disrupt molecular bonds or alter the electron number of atoms." [https://en.wikipedia.org/wiki/Electromagnetic_radiation, https://en.wikipedia.org/wiki/Solar_irradiance]
subset: envoAstro
synonym: "ionising solar radiation" NARROW []
synonym: "ionising stellar radiation" EXACT []

[Term]
id: ENVO:01001477
name: liquid astronomical body part
namespace: ENVO
def: "A part of an astronomical body which is primarily composed of a continuous volume of liquid material, shaped by one or more environmental processes." [https://en.wikipedia.org/wiki/Landform]
is_a: ENVO:01001479 ! fluid astronomical body part
intersection_of: ENVO:01001479 ! fluid astronomical body part
intersection_of: composed_primarily_of ENVO:01000815 ! liquid environmental material
created_by: http://orcid.org/0000-0002-4366-3088

[Term]
id: ENVO:01001479
name: fluid astronomical body part
namespace: ENVO
def: "A part of an astronomical body which is primarily composed of a continuous volume of liquid or gaseous material, shaped by one or more environmental processes." [https://en.wikipedia.org/wiki/Landform]
is_a: ENVO:01000813 ! astronomical body part
created_by: http://orcid.org/0000-0002-4366-3088
creation_date: 2018-10-04T13:59:22Z

[Term]
id: ENVO:01001501
name: radiation from a manufactured product
namespace: ENVO
def: "An electromagnetic radiation process during which electromagnetic waves or their quanta are emitted from a manufactured product." [https://en.wikipedia.org/wiki/Electromagnetic_radiation, https://en.wikipedia.org/wiki/Solar_irradiance]
subset: environmental_hazards
subset: envoAstro
synonym: "anthropogenic radiation" BROAD []
synonym: "artificial radiation" EXACT []
is_a: ENVO:01001026 ! electromagnetic radiation
intersection_of: ENVO:01001026 ! electromagnetic radiation
intersection_of: process_has_causal_agent ENVO:00003074 ! manufactured product
created_by: http://orcid.org/0000-0002-4366-3088
creation_date: 2019-01-09T09:07:24Z

[Term]
id: ENVO:01001678
name: fluid layer
namespace: ENVO
def: "A layer which is composed primarily of some fluid." []
is_a: ENVO:01000281 ! layer
property_value: http://purl.org/dc/elements/1.1/creator http://orcid.org/0000-0002-4366-3088
property_value: http://purl.org/dc/elements/1.1/date 2019-07-22T17:35:08Z xsd:dateTime

[Term]
id: ENVO:01001784
name: compound astronomical body part
namespace: ENVO
def: "A part of an astronomical body which is primarily composed of a continuous medium bearing liquid, gaseous, and solid material in varying quantities." [https://en.wikipedia.org/wiki/Landform]
is_a: ENVO:01000813 ! astronomical body part
property_value: http://purl.org/dc/elements/1.1/creator http://orcid.org/0000-0002-4366-3088
property_value: http://purl.org/dc/elements/1.1/date 2019-10-17T08:36:00Z xsd:dateTime

[Term]
id: ENVO:01001852
name: energy transfer process
namespace: ENVO
def: "A process during which one entity loses energy to another entity." []
is_a: ENVO:02500000 ! environmental system process
property_value: http://purl.org/dc/elements/1.1/creator http://orcid.org/0000-0002-4366-3088
property_value: http://purl.org/dc/elements/1.1/date 2020-02-13T13:34:28Z xsd:dateTime

[Term]
id: ENVO:02000140
name: fluid environmental material
namespace: ENVO
def: "A liquid or a gas." [https://github.com/EnvironmentOntology/envo/issues/940]
synonym: "fluid" NARROW []
is_a: ENVO:00010483 ! environmental material
union_of: ENVO:01000797 ! gaseous environmental material
union_of: ENVO:01000798 ! plasma
union_of: ENVO:01000815 ! liquid environmental material

[Term]
id: ENVO:02500000
name: environmental system process
namespace: ENVO
def: "A process in which includes the components of an environmental system as participants." []
comment: This is a convenience class for organisation and should not be used for annotation.

[Term]
id: ENVO:03000010
name: material transport process
namespace: ENVO
def: "A process during which material is displaced from its original location and transported either to a new location or back to the original location." []
comment: Experimental class for structural purposes not recommended for annotation.
subset: envoPolar
is_a: ENVO:02500000 ! environmental system process
property_value: IAO:0000117 http://orcid.org/0000-0002-3410-4655 xsd:string
property_value: IAO:0000117 http://orcid.org/0000-0002-4366-3088

[Term]
id: ENVO:03000043
name: material transformation process
namespace: ENVO
def: "A process during which a portion of some environmental material is converted into a different material or a collection of materials." []
comment: Experimental class for structural purposes not recommended for annotation. A material transformation process only refers to ENVO:environmental material classes (e.g. bulk and typically impure substances), rather than transformations converting a specific chemical into another.
subset: envoPolar
is_a: ENVO:02500000 ! environmental system process
relationship: has_input ENVO:00010483 ! environmental material
relationship: has_output ENVO:00010483 ! environmental material
property_value: IAO:0000116 "A different material transformation process class (or similarly named class) pertaining to the conversion of a specific chemical into another belongs in CHEBI and or REX ontologies." xsd:string
property_value: IAO:0000117 http://orcid.org/0000-0002-3410-4655 xsd:string
property_value: IAO:0000117 http://orcid.org/0000-0002-4366-3088

[Term]
id: ENVO:03000096
name: season
namespace: ENVO
def: "A one-dimensional temporal region which is delimited by the occurrence of processes which serve as its delimiters." []
subset: envoAstro
subset: envoPolar
property_value: IAO:0000116 "Season could be implemented as a subclass of one-dimensional temporal region, however, this will need further thought and discussion with BFO editors." xsd:string
property_value: IAO:0000117 http://orcid.org/0000-0002-3410-4655 xsd:string
property_value: IAO:0000117 http://orcid.org/0000-0002-4366-3088

[Typedef]
id: adjacent_to
namespace: ENVO
xref: RO:0002220
is_functional: true

[Typedef]
id: attached_to
namespace: ENVO
xref: RO:0002371

[Typedef]
id: bearer_of
namespace: ENVO
xref: RO:0000053

[Typedef]
id: bounding_layer_of
namespace: ENVO
xref: RO:0002007

[Typedef]
id: capable_of
namespace: ENVO
xref: RO:0002215

[Typedef]
id: causal_agent_in_process
namespace: ENVO
xref: RO:0002500

[Typedef]
id: causally_downstream_of_or_within
namespace: ENVO
xref: RO:0002427

[Typedef]
id: causally_upstream_of
namespace: ENVO
xref: RO:0002411

[Typedef]
id: causally_upstream_of_or_within
namespace: ENVO
xref: RO:0002418

[Typedef]
id: composed_primarily_of
namespace: ENVO
xref: RO:0002473

[Typedef]
id: concretizes
namespace: ENVO
xref: RO:0000059

[Typedef]
id: connected_to
namespace: ENVO
xref: RO:0002170

[Typedef]
id: connects
name: connects
namespace: ENVO
xref: RO:0002176

[Typedef]
id: contained_in
namespace: ENVO
xref: RO:0001018

[Typedef]
id: contains
namespace: ENVO
xref: RO:0001019

[Typedef]
id: contains_process
namespace: ENVO
xref: BFO:0000067

[Typedef]
id: continuous_with
namespace: ENVO
xref: RO:0002150

[Typedef]
id: derives_from
namespace: ENVO
xref: RO:0001000

[Typedef]
id: derives_into
namespace: ENVO
xref: RO:0001001

[Typedef]
id: determined_by
namespace: ENVO
xref: RO:0002507

[Typedef]
id: determined_by_part_of
namespace: ENVO
xref: RO:0002509

[Typedef]
id: disconnected_from
name: disconnected_from
namespace: ENVO
def: "A is disconnected_from B if they have no parts in common." [SO:cjm]
synonym: "non_overlapping_with" EXACT []
expand_assertion_to: "Class: <http://www.w3.org/2002/07/owl#Nothing> EquivalentTo: (BFO_0000050 some ?X) and (BFO_0000050 some ?Y)" []
is_metadata_tag: true
is_class_level: true

[Typedef]
id: distributary_of
namespace: ENVO
xref: RO:0002377

[Typedef]
id: during_which_ends
namespace: ENVO
xref: RO:0002084

[Typedef]
id: during_which_starts
namespace: ENVO
xref: RO:0002088

[Typedef]
id: ends
namespace: ENVO
xref: RO:0002229

[Typedef]
id: formed_as_result_of
namespace: ENVO
xref: RO:0002354

[Typedef]
id: generates
name: generates
namespace: ENVO
def: "A relation between a process and a disposition such that the existence of the disposition is caused by the execution of the process." []
xref: ENVO:2000036
property_value: IAO:0000116 "Consider ceding to RO" xsd:string
created_by: cjm
creation_date: 2018-11-03T20:58:13Z

[Typedef]
id: has_condition
name: has_condition
namespace: ENVO
comment: Experimental relation used in EnvO. A condition defines a restricted range of a given quality or combination of qualities. If an environment class, E, has_condition C, then all qualities listed in C are restricted to the ranges defined in C in E. This is not intended as a logical conditional.
xref: has_condition
is_inverse_functional: true
creation_date: 2013-05-08T07:33:05Z

[Typedef]
id: has_disposition
namespace: ENVO
xref: RO:0000091

[Typedef]
id: has_end_location
namespace: ENVO
xref: RO:0002232

[Typedef]
id: has_function
namespace: ENVO
xref: RO:0000085

[Typedef]
id: has_habitat
name: has habitat
namespace: ENVO
xref: RO:0002303

[Typedef]
id: has_increased_levels_of
namespace: ENVO
xref: has_increased_levels_of

[Typedef]
id: has_input
namespace: ENVO
xref: RO:0002233

[Typedef]
id: has_member
namespace: ENVO
xref: RO:0002351

[Typedef]
id: has_output
namespace: ENVO
xref: RO:0002234

[Typedef]
id: has_part
namespace: ENVO
xref: BFO:0000051

[Typedef]
id: has_part_that_occurs_in
namespace: ENVO
xref: RO:0002479

[Typedef]
id: has_participant
namespace: ENVO
xref: RO:0000057

[Typedef]
id: has_quality
namespace: ENVO
xref: RO:0000086

[Typedef]
id: has_role
namespace: ENVO
xref: RO:0000087

[Typedef]
id: inheres_in
namespace: ENVO
xref: RO:0000052

[Typedef]
id: input_of
namespace: ENVO
xref: RO:0002352

[Typedef]
id: involved_in_negative_regulation_of
namespace: ENVO
xref: RO:0002430

[Typedef]
id: located_in
namespace: ENVO
xref: RO:0001025

[Typedef]
id: location_of
namespace: ENVO
xref: RO:0001015

[Typedef]
id: member_of
namespace: ENVO
xref: RO:0002350

[Typedef]
id: negatively_regulates
namespace: ENVO
xref: RO:0002212

[Typedef]
id: obsolete_determined_by
name: obsolete determined by
namespace: ENVO
xref: ENVO:2100001
is_obsolete: true

[Typedef]
id: obsolete_determined_by_part_of
name: obsolete determined by part of
namespace: ENVO
xref: ENVO:2100007
is_obsolete: true

[Typedef]
id: obsolete_has_active_participant
namespace: ENVO
xref: RO:0002218

[Typedef]
id: occurs_in
namespace: ENVO
xref: BFO:0000066

[Typedef]
id: output_of
namespace: ENVO
xref: RO:0002353

[Typedef]
id: overlaps
namespace: ENVO
xref: RO:0002131

[Typedef]
id: part_of
namespace: ENVO
xref: BFO:0000050

[Typedef]
id: partially_overlaps
namespace: ENVO
xref: RO:0002151

[Typedef]
id: partially_surrounded_by
name: partially_surrounded_by
namespace: ENVO
def: "x partially_surrounded_by y if and only if (1) x is adjacent to y and for the region r that is adjacent to x, r partially overlaps y (2) the shared boundary between x and y occupies  a non-trivial proportion of the outermost boundary of x" []
comment: Definition modified from 'surrounded by'.
xref: ENVO:01001307
property_value: IAO:0000112 "A duck swimming in a pond is partially surrounded by air and partially surrounded by water." xsd:string

[Typedef]
id: participates_in
namespace: ENVO
xref: RO:0000056

[Typedef]
id: preceded_by
namespace: ENVO
xref: BFO:0000062

[Typedef]
id: precedes
namespace: ENVO
xref: BFO:0000063

[Typedef]
id: process_has_causal_agent
namespace: ENVO
xref: RO:0002608

[Typedef]
id: realized_in
namespace: ENVO
xref: BFO:0000054

[Typedef]
id: realizes
namespace: ENVO
xref: BFO:0000055

[Typedef]
id: regulates_(processual)
name: regulates (processual)
namespace: ENVO
xref: RO:0002211

[Typedef]
id: results_in_expansion_of
name: results in expansion of
namespace: ENVO
def: "A process, p, results in the expansion of a material entity, m, if the spatial extent of m is increased as a result of participating in p." []
xref: ENVO:02500016
property_value: IAO:0000112 "Afforestation results in the expansion of a forest." xsd:string

[Typedef]
id: results_in_formation_of
namespace: ENVO
xref: RO:0002297

[Typedef]
id: results_in_proliferation_of
name: results in proliferation of
namespace: ENVO
comment: To be ceded to RO
xref: ENVO:02500020

[Typedef]
id: results_in_transformation_into
name: results in transformation into
namespace: ENVO
xref: ENVO:02500006

[Typedef]
id: starts_during
namespace: ENVO
xref: RO:0002091

[Typedef]
id: surrounded_by
name: surrounded by
namespace: ENVO
xref: RO:0002219

[Typedef]
id: towards
namespace: ENVO
xref: RO:0002503

[Typedef]
id: tributary_of
namespace: ENVO
xref: RO:0002376

